<?xml version="1.0"?>
<rdf:RDF xmlns="https://w3id.org/reno#"
     xml:base="https://w3id.org/reno"
     xmlns:owl="http://www.w3.org/2002/07/owl#"
     xmlns:rdf="http://www.w3.org/1999/02/22-rdf-syntax-ns#"
     xmlns:xml="http://www.w3.org/XML/1998/namespace"
     xmlns:xsd="http://www.w3.org/2001/XMLSchema#"
     xmlns:rdfs="http://www.w3.org/2000/01/rdf-schema#"
     xmlns:reno="https://w3id.org/reno#"
     xmlns:vann="http://purl.org/vocab/vann/"
     xmlns:terms="http://purl.org/dc/terms/"
     xmlns:schema="https://schema.org/"
     xmlns:Process="http://www.daml.org/services/owl-s/1.1/Process.owl#">
    <owl:Ontology rdf:about="https://w3id.org/reno#">
        <terms:abstract xml:lang="nl">Deze ontologie werd ontwikkeld als onderdeel van het RE-ENNOVATE project. Het doel is om concepten vast te leggen, die relevant zijn bij het ontwerpend van energetische renovatie suggesties.</terms:abstract>
        <terms:abstract xml:lang="en">This ontology was developed as part of the RE-ENNOVATE project. It aims to capture concepts that are relevant when designing energy renovation suggestions.</terms:abstract>
        <terms:creator>Emma Nuyts</terms:creator>
        <terms:creator>Femke Ongenae</terms:creator>
        <terms:creator>Mathias De Brouwer</terms:creator>
        <terms:license>https://creativecommons.org/licenses/by/4.0/</terms:license>
        <terms:modified rdf:datatype="http://www.w3.org/2001/XMLSchema#date">2025-03-06</terms:modified>
        <terms:title xml:lang="nl">Renovatie en ENergie Optimalisatie (RENO)</terms:title>
        <terms:title xml:lang="en">Renovation and ENergy Optimization (RENO)</terms:title>
        <vann:preferredNamespacePrefix>reno</vann:preferredNamespacePrefix>
        <vann:preferredNamespaceUri>https://w3id.org/reno#</vann:preferredNamespaceUri>
        <owl:versionInfo>0.0.1</owl:versionInfo>
    </owl:Ontology>
    


    <!-- 
    ///////////////////////////////////////////////////////////////////////////////////////
    //
    // Annotation properties
    //
    ///////////////////////////////////////////////////////////////////////////////////////
     -->


    


    <!-- http://purl.org/dc/terms/abstract -->


    <owl:AnnotationProperty rdf:about="http://purl.org/dc/terms/abstract"/>
    


    <!-- http://purl.org/dc/terms/contributor -->


    <owl:AnnotationProperty rdf:about="http://purl.org/dc/terms/contributor"/>
    


    <!-- http://purl.org/dc/terms/creator -->


    <owl:AnnotationProperty rdf:about="http://purl.org/dc/terms/creator"/>
    


    <!-- http://purl.org/dc/terms/license -->


    <owl:AnnotationProperty rdf:about="http://purl.org/dc/terms/license"/>
    


    <!-- http://purl.org/dc/terms/modified -->


    <owl:AnnotationProperty rdf:about="http://purl.org/dc/terms/modified"/>
    


    <!-- http://purl.org/dc/terms/title -->


    <owl:AnnotationProperty rdf:about="http://purl.org/dc/terms/title"/>
    


    <!-- http://purl.org/vocab/vann/preferredNamespacePrefix -->


    <owl:AnnotationProperty rdf:about="http://purl.org/vocab/vann/preferredNamespacePrefix"/>
    


    <!-- http://purl.org/vocab/vann/preferredNamespaceUri -->


    <owl:AnnotationProperty rdf:about="http://purl.org/vocab/vann/preferredNamespaceUri"/>
    


    <!-- https://schema.org/domainIncludes -->


    <owl:AnnotationProperty rdf:about="https://schema.org/domainIncludes">
        <rdfs:comment>Relates a property to a class that is (one of) the type(s) the property is expected to be used on.</rdfs:comment>
        <rdfs:label>domainIncludes</rdfs:label>
        <schema:domainIncludes rdf:resource="https://schema.org/Property"/>
        <schema:rangeIncludes rdf:resource="https://schema.org/Class"/>
    </owl:AnnotationProperty>
    


    <!-- https://schema.org/rangeIncludes -->


    <owl:AnnotationProperty rdf:about="https://schema.org/rangeIncludes">
        <rdfs:comment>Relates a property to a class that constitutes (one of) the expected type(s) for values of the property.</rdfs:comment>
        <rdfs:label>rangeIncludes</rdfs:label>
        <schema:domainIncludes rdf:resource="https://schema.org/Property"/>
        <schema:rangeIncludes rdf:resource="https://schema.org/Class"/>
    </owl:AnnotationProperty>
    


    <!-- 
    ///////////////////////////////////////////////////////////////////////////////////////
    //
    // Datatypes
    //
    ///////////////////////////////////////////////////////////////////////////////////////
     -->


    


    <!-- http://www.w3.org/2001/XMLSchema#date -->


    <rdfs:Datatype rdf:about="http://www.w3.org/2001/XMLSchema#date"/>
    


    <!-- http://www.w3.org/2001/XMLSchema#gYear -->


    <rdfs:Datatype rdf:about="http://www.w3.org/2001/XMLSchema#gYear"/>
    


    <!-- http://www.w3.org/2001/XMLSchema#time -->


    <rdfs:Datatype rdf:about="http://www.w3.org/2001/XMLSchema#time"/>
    


    <!-- 
    ///////////////////////////////////////////////////////////////////////////////////////
    //
    // Object Properties
    //
    ///////////////////////////////////////////////////////////////////////////////////////
     -->


    


    <!-- http://bimerr.iot.linkeddata.es/def/material-properties#hasMaterial -->


    <owl:ObjectProperty rdf:about="http://bimerr.iot.linkeddata.es/def/material-properties#hasMaterial">
        <rdfs:range rdf:resource="http://bimerr.iot.linkeddata.es/def/material-properties#Material"/>
        <rdfs:comment>Relation between a construction component (Layer, profile, constituent) and the materials that define them.</rdfs:comment>
    </owl:ObjectProperty>
    


    <!-- http://bimerr.iot.linkeddata.es/def/material-properties#hasMaterialLayer -->


    <owl:ObjectProperty rdf:about="http://bimerr.iot.linkeddata.es/def/material-properties#hasMaterialLayer">
        <rdfs:domain rdf:resource="http://bimerr.iot.linkeddata.es/def/material-properties#MaterialLayerSet"/>
        <rdfs:range rdf:resource="http://bimerr.iot.linkeddata.es/def/material-properties#MaterialLayer"/>
        <rdfs:comment>A relation between a layer set and the specific material layers.</rdfs:comment>
    </owl:ObjectProperty>
    


    <!-- http://bimerr.iot.linkeddata.es/def/material-properties#hasMaterialLayerSet -->


    <owl:ObjectProperty rdf:about="http://bimerr.iot.linkeddata.es/def/material-properties#hasMaterialLayerSet">
        <rdfs:range rdf:resource="http://bimerr.iot.linkeddata.es/def/material-properties#MaterialLayerSet"/>
        <rdfs:comment>Relation between an element and its construction based in material layers.</rdfs:comment>
    </owl:ObjectProperty>
    


    <!-- http://www.daml.org/services/owl-s/1.1/Process.owl#composedOf -->


    <owl:ObjectProperty rdf:about="http://www.daml.org/services/owl-s/1.1/Process.owl#composedOf">
        <rdfs:domain rdf:resource="http://www.daml.org/services/owl-s/1.1/Process.owl#CompositeProcess"/>
        <rdfs:range rdf:resource="http://www.daml.org/services/owl-s/1.1/Process.owl#ControlConstruct"/>
    </owl:ObjectProperty>
    


    <!-- http://www.daml.org/services/owl-s/1.1/Process.owl#hasPrecondition -->


    <owl:ObjectProperty rdf:about="http://www.daml.org/services/owl-s/1.1/Process.owl#hasPrecondition">
        <rdfs:domain rdf:resource="http://www.daml.org/services/owl-s/1.1/Process.owl#Process"/>
        <rdfs:range rdf:resource="http://www.daml.org/services/owl-s/1.1/generic/Expression.owl#Condition"/>
    </owl:ObjectProperty>
    


    <!-- http://www.daml.org/services/owl-s/1.1/Process.owl#hasResult -->


    <owl:ObjectProperty rdf:about="http://www.daml.org/services/owl-s/1.1/Process.owl#hasResult">
        <rdfs:domain rdf:resource="http://www.daml.org/services/owl-s/1.1/Process.owl#Process"/>
        <rdfs:range rdf:resource="http://www.daml.org/services/owl-s/1.1/Process.owl#Result"/>
        <rdfs:label>hasResult</rdfs:label>
    </owl:ObjectProperty>
    


    <!-- http://www.daml.org/services/owl-s/1.1/Process.owl#process -->


    <owl:ObjectProperty rdf:about="http://www.daml.org/services/owl-s/1.1/Process.owl#process">
        <rdfs:domain rdf:resource="http://www.daml.org/services/owl-s/1.1/Process.owl#Perform"/>
        <rdfs:range rdf:resource="http://www.daml.org/services/owl-s/1.1/Process.owl#Process"/>
    </owl:ObjectProperty>
    


    <!-- https://saref.etsi.org/core/accomplishes -->


    <owl:ObjectProperty rdf:about="https://saref.etsi.org/core/accomplishes">
        <owl:inverseOf rdf:resource="https://saref.etsi.org/core/isAccomplishedBy"/>
        <rdfs:range rdf:resource="https://saref.etsi.org/core/Task"/>
        <rdfs:comment>Links a certain entity (e.g., a device) to the task it accomplishes.</rdfs:comment>
    </owl:ObjectProperty>
    


    <!-- https://saref.etsi.org/core/consumes -->


    <owl:ObjectProperty rdf:about="https://saref.etsi.org/core/consumes">
        <owl:inverseOf rdf:resource="https://saref.etsi.org/core/isConsumedBy"/>
        <rdfs:comment>Links a feature kind, feature of interest, or device, to the commodity it consumes</rdfs:comment>
    </owl:ObjectProperty>
    


    <!-- https://saref.etsi.org/core/isAccomplishedBy -->


    <owl:ObjectProperty rdf:about="https://saref.etsi.org/core/isAccomplishedBy">
        <rdfs:comment>A relationship identifying an entity (e.g., a device) that can accomplish a task.</rdfs:comment>
    </owl:ObjectProperty>
    


    <!-- https://saref.etsi.org/core/isConsumedBy -->


    <owl:ObjectProperty rdf:about="https://saref.etsi.org/core/isConsumedBy">
        <rdfs:comment>Links a commodity to the feature kind, feature of interest, or device, that consumes it</rdfs:comment>
    </owl:ObjectProperty>
    


    <!-- https://w3id.org/bot#adjacentElement -->


    <owl:ObjectProperty rdf:about="https://w3id.org/bot#adjacentElement">
        <rdfs:subPropertyOf rdf:resource="https://w3id.org/bot#hasElement"/>
        <owl:propertyDisjointWith rdf:resource="https://w3id.org/bot#intersectingElement"/>
        <rdfs:comment xml:lang="nl">Relatie tussen een zone en zijn aangrenzende gebouwelementen. Het gebouwelement begrenst de zone.</rdfs:comment>
        <rdfs:comment xml:lang="en">Relation between a zone and its adjacent building elements, bounding the zone.</rdfs:comment>
        <rdfs:label xml:lang="nl">aangrenzend element</rdfs:label>
        <rdfs:label xml:lang="en">adjacent element</rdfs:label>
    </owl:ObjectProperty>
    


    <!-- https://w3id.org/bot#adjacentZone -->


    <owl:ObjectProperty rdf:about="https://w3id.org/bot#adjacentZone">
        <rdf:type rdf:resource="http://www.w3.org/2002/07/owl#SymmetricProperty"/>
        <rdfs:domain rdf:resource="https://w3id.org/bot#Zone"/>
        <rdfs:range rdf:resource="https://w3id.org/bot#Zone"/>
        <owl:propertyDisjointWith rdf:resource="https://w3id.org/bot#intersectsZone"/>
        <rdfs:comment xml:lang="nl">Relatie tussen twee zones die een interface delen, maar niet doorsnijdend zijn</rdfs:comment>
        <rdfs:comment xml:lang="en">Relationship between two zones that share a common interface, but do not intersect.</rdfs:comment>
        <rdfs:label xml:lang="nl">aangrenzende zone</rdfs:label>
        <rdfs:label xml:lang="en">adjacent zone</rdfs:label>
        <schema:domainIncludes rdf:resource="https://w3id.org/bot#Building"/>
        <schema:domainIncludes rdf:resource="https://w3id.org/bot#Site"/>
        <schema:domainIncludes rdf:resource="https://w3id.org/bot#Space"/>
        <schema:domainIncludes rdf:resource="https://w3id.org/bot#Storey"/>
        <schema:rangeIncludes rdf:resource="https://w3id.org/bot#Building"/>
        <schema:rangeIncludes rdf:resource="https://w3id.org/bot#Site"/>
        <schema:rangeIncludes rdf:resource="https://w3id.org/bot#Space"/>
        <schema:rangeIncludes rdf:resource="https://w3id.org/bot#Storey"/>
    </owl:ObjectProperty>
    


    <!-- https://w3id.org/bot#containsElement -->


    <owl:ObjectProperty rdf:about="https://w3id.org/bot#containsElement">
        <rdfs:subPropertyOf rdf:resource="https://w3id.org/bot#hasElement"/>
        <owl:propertyChainAxiom rdf:parseType="Collection">
            <rdf:Description rdf:about="https://w3id.org/bot#containsZone"/>
            <rdf:Description rdf:about="https://w3id.org/bot#containsElement"/>
        </owl:propertyChainAxiom>
        <rdfs:comment xml:lang="nl">Relatie tussen zone en een gebouwelement bevat in die zone.</rdfs:comment>
        <rdfs:comment xml:lang="en">Relation to a building element contained in a zone.</rdfs:comment>
        <rdfs:label xml:lang="nl">bevat element</rdfs:label>
        <rdfs:label xml:lang="en">contains element</rdfs:label>
    </owl:ObjectProperty>
    


    <!-- https://w3id.org/bot#containsZone -->


    <owl:ObjectProperty rdf:about="https://w3id.org/bot#containsZone">
        <rdf:type rdf:resource="http://www.w3.org/2002/07/owl#TransitiveProperty"/>
        <rdfs:domain rdf:resource="https://w3id.org/bot#Zone"/>
        <rdfs:range rdf:resource="https://w3id.org/bot#Zone"/>
        <rdfs:comment xml:lang="nl">Relatie tussen subzones van een hoofd zone. Een ruimtezone kan bijvoorbeeld worden bevat door een verdiepingszone, die wederom bevat wordt door een gebouwzone. bot:containsZone is een transitieve eigenschap, wat betekent dat in het vorige voorbeeld de ruimtezone ook bevat wordt door de gebouwzone.</rdfs:comment>
        <rdfs:comment xml:lang="en">Relationship to the subzones of a major zone. A space zone could for instance be contained in a storey zone which is further contained in a building zone. bot:containsZone is a transitive property. This implies that in the previous example a bot:containsZone relationship holds between the space zone and the building zone.</rdfs:comment>
        <rdfs:label xml:lang="nl">bevat zone</rdfs:label>
        <rdfs:label xml:lang="en">contains zone</rdfs:label>
        <schema:domainIncludes rdf:resource="https://w3id.org/bot#Building"/>
        <schema:domainIncludes rdf:resource="https://w3id.org/bot#Site"/>
        <schema:domainIncludes rdf:resource="https://w3id.org/bot#Space"/>
        <schema:domainIncludes rdf:resource="https://w3id.org/bot#Storey"/>
        <schema:rangeIncludes rdf:resource="https://w3id.org/bot#Building"/>
        <schema:rangeIncludes rdf:resource="https://w3id.org/bot#Site"/>
        <schema:rangeIncludes rdf:resource="https://w3id.org/bot#Space"/>
        <schema:rangeIncludes rdf:resource="https://w3id.org/bot#Storey"/>
    </owl:ObjectProperty>
    


    <!-- https://w3id.org/bot#hasBuilding -->


    <owl:ObjectProperty rdf:about="https://w3id.org/bot#hasBuilding">
        <rdfs:subPropertyOf rdf:resource="https://w3id.org/bot#containsZone"/>
        <rdfs:domain rdf:resource="https://w3id.org/bot#Zone"/>
        <rdfs:range rdf:resource="https://w3id.org/bot#Building"/>
        <rdfs:comment xml:lang="nl">Relatie tot gebouwen die zich in een zone bevinden. De typische domeinen van bot:hasBuilding zijn instanties van bot:Site</rdfs:comment>
        <rdfs:comment xml:lang="en">Relation to buildings contained in a zone. The typical domains of bot:hasBuilding are instances of bot:Site.</rdfs:comment>
        <rdfs:label xml:lang="en">has building</rdfs:label>
        <rdfs:label xml:lang="nl">heeft gebouw</rdfs:label>
        <schema:domainIncludes rdf:resource="https://w3id.org/bot#Site"/>
    </owl:ObjectProperty>
    


    <!-- https://w3id.org/bot#hasElement -->


    <owl:ObjectProperty rdf:about="https://w3id.org/bot#hasElement">
        <rdfs:domain rdf:resource="https://w3id.org/bot#Zone"/>
        <rdfs:range rdf:resource="https://w3id.org/bot#Element"/>
        <owl:propertyChainAxiom rdf:parseType="Collection">
            <rdf:Description rdf:about="https://w3id.org/bot#containsZone"/>
            <rdf:Description rdf:about="https://w3id.org/bot#hasElement"/>
        </owl:propertyChainAxiom>
        <rdfs:comment xml:lang="en">Links a Zone to an Element that is either contained in, adjacent to or intersecting with the Zone. The intended use of this relationship is not to be stated explicitly, but to be inferred from its sub-properties. It will, for example, allow one to query for all the doors of a building given that they have an adjacency to spaces of the building.</rdfs:comment>
        <rdfs:comment xml:lang="nl">Verbindt een bot:Zone instantie met een bot:Element instantie die er ofwel door bevat wordt, aangrenzend aan is of snijdend mee is. Het is aangeraden om deze relatie niet expliciet te maken, maar af te leiden uit het gebruik van zijn sub relaties. Deze relatie maakt het bijvoorbeeld mogelijk om alle deuren van een gebouw op te vragen als die aangrenzend gedefinieerd zijn aan de ruimtes van het gebouw.</rdfs:comment>
        <rdfs:label xml:lang="en">has element</rdfs:label>
        <rdfs:label xml:lang="nl">heeft element</rdfs:label>
    </owl:ObjectProperty>
    


    <!-- https://w3id.org/bot#hasSpace -->


    <owl:ObjectProperty rdf:about="https://w3id.org/bot#hasSpace">
        <rdfs:subPropertyOf rdf:resource="https://w3id.org/bot#containsZone"/>
        <rdfs:domain rdf:resource="https://w3id.org/bot#Zone"/>
        <rdfs:range rdf:resource="https://w3id.org/bot#Space"/>
        <rdfs:comment xml:lang="nl">Relatie tot ruimtes die zich in een zone bevinden. De typische domeinen van bot:hasSpace zijn instanties van bot:Storey of bot:Building.</rdfs:comment>
        <rdfs:comment xml:lang="en">Relation to spaces contained in a zone. The typical domains of bot:hasSpace are instances of bot:Storey or bot:Building.</rdfs:comment>
        <rdfs:label xml:lang="en">has space</rdfs:label>
        <rdfs:label xml:lang="nl">heeft ruimte</rdfs:label>
        <schema:domainIncludes rdf:resource="https://w3id.org/bot#Storey"/>
    </owl:ObjectProperty>
    


    <!-- https://w3id.org/bot#hasStorey -->


    <owl:ObjectProperty rdf:about="https://w3id.org/bot#hasStorey">
        <rdfs:subPropertyOf rdf:resource="https://w3id.org/bot#containsZone"/>
        <rdfs:domain rdf:resource="https://w3id.org/bot#Zone"/>
        <rdfs:range rdf:resource="https://w3id.org/bot#Storey"/>
        <rdfs:comment xml:lang="nl">Relatie tot de verdiepingen die zich in een zone bevinden. De typische domeinen van bot:hasStorey zijn instanties van bot:Building.</rdfs:comment>
        <rdfs:comment xml:lang="en">Relation to storeys contained in a zone. The typical domains of bot:hasStorey are instances of bot:Building.</rdfs:comment>
        <rdfs:label xml:lang="en">has storey</rdfs:label>
        <rdfs:label xml:lang="nl">heeft verdieping</rdfs:label>
        <schema:domainIncludes rdf:resource="https://w3id.org/bot#Building"/>
    </owl:ObjectProperty>
    


    <!-- https://w3id.org/bot#hasSubElement -->


    <owl:ObjectProperty rdf:about="https://w3id.org/bot#hasSubElement">
        <rdfs:domain rdf:resource="https://w3id.org/bot#Element"/>
        <rdfs:range rdf:resource="https://w3id.org/bot#Element"/>
        <rdfs:comment xml:lang="nl">Relatie tussen twee gebouwelementen, ofwel één element dat een andere element bevat (bv. een muur die een raam bevat) of een subcompositie van een gebouwelement in kleinere delen (bv. een luchtbehandelingskast die een ventilator bevat).</rdfs:comment>
        <rdfs:comment xml:lang="en">Relation between two building elements, either one element hosting another (e.g. a wall hosts a window) or a subcomposition of a building element into smaller parts (e.g. an air handling unit has as a part a fan).</rdfs:comment>
        <rdfs:label xml:lang="en">has sub-element</rdfs:label>
        <rdfs:label xml:lang="nl">heeft subelement</rdfs:label>
    </owl:ObjectProperty>
    


    <!-- https://w3id.org/bot#intersectingElement -->


    <owl:ObjectProperty rdf:about="https://w3id.org/bot#intersectingElement">
        <rdfs:subPropertyOf rdf:resource="https://w3id.org/bot#hasElement"/>
        <rdfs:comment xml:lang="nl">Relatie tussen een zone en een gebouwelement die de zone doorsnijdt.</rdfs:comment>
        <rdfs:comment xml:lang="en">Relation between a Zone and a building Element that intersects it.</rdfs:comment>
        <rdfs:label xml:lang="nl">doorsnijdend element</rdfs:label>
        <rdfs:label xml:lang="en">intersecting element</rdfs:label>
    </owl:ObjectProperty>
    


    <!-- https://w3id.org/bot#intersectsZone -->


    <owl:ObjectProperty rdf:about="https://w3id.org/bot#intersectsZone">
        <rdf:type rdf:resource="http://www.w3.org/2002/07/owl#SymmetricProperty"/>
        <rdfs:domain rdf:resource="https://w3id.org/bot#Zone"/>
        <rdfs:range rdf:resource="https://w3id.org/bot#Zone"/>
        <rdfs:comment xml:lang="nl">Een relatie tussen twee zones waarvan de driedimensionale omvang doorsnijdend is. Bijvoorbeeld een traphal die verschillende verdiepingen doorsnijdt.</rdfs:comment>
        <rdfs:comment xml:lang="en">Relationship between two zones whose 3D extent intersect. For example, a stairwell intersects different storeys.</rdfs:comment>
        <rdfs:label xml:lang="en">intersects zone</rdfs:label>
        <rdfs:label xml:lang="nl">snijdt door zone</rdfs:label>
        <schema:domainIncludes rdf:resource="https://w3id.org/bot#Building"/>
        <schema:domainIncludes rdf:resource="https://w3id.org/bot#Site"/>
        <schema:domainIncludes rdf:resource="https://w3id.org/bot#Space"/>
        <schema:domainIncludes rdf:resource="https://w3id.org/bot#Storey"/>
        <schema:rangeIncludes rdf:resource="https://w3id.org/bot#Building"/>
        <schema:rangeIncludes rdf:resource="https://w3id.org/bot#Site"/>
        <schema:rangeIncludes rdf:resource="https://w3id.org/bot#Space"/>
        <schema:rangeIncludes rdf:resource="https://w3id.org/bot#Storey"/>
    </owl:ObjectProperty>
    


    <!-- https://w3id.org/reno#changedDuring -->


    <owl:ObjectProperty rdf:about="https://w3id.org/reno#changedDuring">
        <rdf:type rdf:resource="http://www.w3.org/2002/07/owl#FunctionalProperty"/>
        <rdfs:range rdf:resource="https://w3id.org/reno#RenovationIntervention"/>
        <rdfs:comment xml:lang="nl">De relatie tussen een bouwcomponent (set materiaallagen, raamkader...) en de renovatie interventie waarbij het veranderde.</rdfs:comment>
        <rdfs:comment xml:lang="en">The relationship between a building component (material layer set, windowframe...) and the renovation intervention during which it changed.</rdfs:comment>
        <rdfs:label xml:lang="en">changed during</rdfs:label>
        <rdfs:label xml:lang="nl">veranderd tijdens</rdfs:label>
    </owl:ObjectProperty>
    


    <!-- https://w3id.org/reno#changedInto -->


    <owl:ObjectProperty rdf:about="https://w3id.org/reno#changedInto">
        <rdfs:comment xml:lang="nl">De relatie tussen een bouwdeel (set materiaallagen, raamkader...) en het bouwdeel waarin het veranderde.</rdfs:comment>
        <rdfs:comment xml:lang="en">The relationship between a building component (material layer set, windowframe...) and the building component it changed into.</rdfs:comment>
        <rdfs:label xml:lang="en">changed into</rdfs:label>
        <rdfs:label xml:lang="nl">veranderd in</rdfs:label>
    </owl:ObjectProperty>
    


    <!-- https://w3id.org/reno#commodityAccomplishes -->


    <owl:ObjectProperty rdf:about="https://w3id.org/reno#commodityAccomplishes">
        <rdfs:domain rdf:resource="https://saref.etsi.org/core/Commodity"/>
        <rdfs:range rdf:resource="https://saref.etsi.org/core/Task"/>
        <owl:propertyChainAxiom rdf:parseType="Collection">
            <rdf:Description rdf:about="https://saref.etsi.org/core/isConsumedBy"/>
            <rdf:Description rdf:about="https://saref.etsi.org/core/accomplishes"/>
        </owl:propertyChainAxiom>
        <rdfs:comment xml:lang="nl">De relatie tussen een drager en de taak die erdoor wordt verwezenlijkt.</rdfs:comment>
        <rdfs:comment xml:lang="en">The relationship between a commodity and the task it accomplishes.</rdfs:comment>
        <rdfs:label xml:lang="en">commodity accomplishes</rdfs:label>
        <rdfs:label xml:lang="nl">drager verwezenlijkt</rdfs:label>
    </owl:ObjectProperty>
    


    <!-- https://w3id.org/reno#hasAddress -->


    <owl:ObjectProperty rdf:about="https://w3id.org/reno#hasAddress">
        <rdfs:domain rdf:resource="https://w3id.org/reno#Resident"/>
        <rdfs:range rdf:resource="https://w3id.org/reno#Address"/>
        <owl:propertyChainAxiom rdf:parseType="Collection">
            <rdf:Description rdf:about="https://w3id.org/reno#isResidentOf"/>
            <rdf:Description rdf:about="https://w3id.org/reno#hasAddress"/>
        </owl:propertyChainAxiom>
        <rdfs:comment xml:lang="nl">De relatie tussen een persoon en het adres waarop ze wonen.</rdfs:comment>
        <rdfs:comment xml:lang="en">The relationship between a person and the address they reside at.</rdfs:comment>
        <rdfs:label xml:lang="en">has address</rdfs:label>
        <rdfs:label xml:lang="nl">heeft adres</rdfs:label>
    </owl:ObjectProperty>
    


    <!-- https://w3id.org/reno#hasAffectedElement -->


    <owl:ObjectProperty rdf:about="https://w3id.org/reno#hasAffectedElement">
        <rdfs:domain rdf:resource="https://w3id.org/reno#Tender"/>
        <rdfs:range rdf:resource="https://w3id.org/bot#Element"/>
        <rdfs:comment xml:lang="nl">De relatie tussen een offerte en de (bouw)elementen die erdoor worden beïnvloed.</rdfs:comment>
        <rdfs:comment xml:lang="en">The relationship between a tender and the (building) elements it affects.</rdfs:comment>
        <rdfs:label xml:lang="en">has affected element</rdfs:label>
        <rdfs:label xml:lang="nl">heeft invloed op element</rdfs:label>
    </owl:ObjectProperty>
    


    <!-- https://w3id.org/reno#hasCreator -->


    <owl:ObjectProperty rdf:about="https://w3id.org/reno#hasCreator">
        <rdf:type rdf:resource="http://www.w3.org/2002/07/owl#FunctionalProperty"/>
        <rdfs:domain rdf:resource="https://w3id.org/reno#EnergyPerformanceCertificate"/>
        <rdfs:range rdf:resource="https://w3id.org/reno#EnergyExpert"/>
        <rdfs:comment xml:lang="nl">De relatie tussen een energieprestatiecertificaat en de energiedeskundige die het opgesteld heeft.</rdfs:comment>
        <rdfs:comment xml:lang="en">The relationship between a energy performance certificate and the energy expert who created it.</rdfs:comment>
        <rdfs:label xml:lang="en">has creator</rdfs:label>
        <rdfs:label xml:lang="nl">heeft maker</rdfs:label>
    </owl:ObjectProperty>
    


    <!-- https://w3id.org/reno#hasDesiredSoundLevel -->


    <owl:ObjectProperty rdf:about="https://w3id.org/reno#hasDesiredSoundLevel">
        <rdfs:domain rdf:resource="https://w3id.org/bot#Space"/>
        <rdfs:range rdf:resource="https://w3id.org/reno#SoundLevel"/>
        <rdfs:comment xml:lang="nl">De relatie tussen een ruimte en zijn gewenst geluidsniveau.</rdfs:comment>
        <rdfs:comment xml:lang="en">The relationship between a space and its desired sound level.</rdfs:comment>
        <rdfs:label xml:lang="en">has desired sound level</rdfs:label>
        <rdfs:label xml:lang="nl">heeft gewenst geluidsniveau</rdfs:label>
    </owl:ObjectProperty>
    


    <!-- https://w3id.org/reno#hasEnergyPerformanceCertificate -->


    <owl:ObjectProperty rdf:about="https://w3id.org/reno#hasEnergyPerformanceCertificate">
        <rdfs:domain rdf:resource="https://w3id.org/bot#Zone"/>
        <rdfs:range rdf:resource="https://w3id.org/reno#EnergyPerformanceCertificate"/>
        <owl:propertyChainAxiom rdf:parseType="Collection">
            <rdf:Description rdf:about="https://w3id.org/bot#containsZone"/>
            <rdf:Description rdf:about="https://w3id.org/reno#hasEnergyPerformanceCertificate"/>
        </owl:propertyChainAxiom>
        <rdfs:comment xml:lang="nl">De relatie tussen een zone en het bijhorende energieprestatiecertificaat. Een zone kan de energieprestatiecertificaten van de subzones aggregeren.</rdfs:comment>
        <rdfs:comment xml:lang="en">The relationship between a zone and its energy performance certificate. A zone can aggregate the energy performance certificates of its subszones.</rdfs:comment>
        <rdfs:label xml:lang="en">has energy performance certificate</rdfs:label>
        <rdfs:label xml:lang="nl">heeft energieprestatiecertificaat</rdfs:label>
    </owl:ObjectProperty>
    


    <!-- https://w3id.org/reno#hasFrame -->


    <owl:ObjectProperty rdf:about="https://w3id.org/reno#hasFrame">
        <rdfs:domain rdf:resource="https://pi.pauwel.be/voc/buildingelement#Window"/>
        <rdfs:range rdf:resource="https://w3id.org/reno#WindowFrame"/>
        <rdfs:comment xml:lang="nl">De relatie tussen een raam en zijn kader.</rdfs:comment>
        <rdfs:comment xml:lang="en">The relationship between a window and its frame.</rdfs:comment>
        <rdfs:label xml:lang="en">has frame</rdfs:label>
        <rdfs:label xml:lang="nl">heeft kader</rdfs:label>
    </owl:ObjectProperty>
    


    <!-- https://w3id.org/reno#hasFrameMaterial -->


    <owl:ObjectProperty rdf:about="https://w3id.org/reno#hasFrameMaterial">
        <rdf:type rdf:resource="http://www.w3.org/2002/07/owl#FunctionalProperty"/>
        <rdfs:domain rdf:resource="https://w3id.org/reno#WindowFrame"/>
        <rdfs:range rdf:resource="https://w3id.org/reno#WindowFrameMaterial"/>
        <rdfs:comment xml:lang="nl">De relatie tussen een raamkader en het materiaal waaruit het vervaardigt is.</rdfs:comment>
        <rdfs:comment xml:lang="en">The relationship between a window frame and the material it is made of.</rdfs:comment>
        <rdfs:label xml:lang="en">frame material</rdfs:label>
        <rdfs:label xml:lang="nl">kader materiaal</rdfs:label>
    </owl:ObjectProperty>
    


    <!-- https://w3id.org/reno#hasGlazing -->


    <owl:ObjectProperty rdf:about="https://w3id.org/reno#hasGlazing">
        <rdfs:domain rdf:resource="https://pi.pauwel.be/voc/buildingelement#Window"/>
        <rdfs:range rdf:resource="https://w3id.org/reno#WindowGlazing"/>
        <rdfs:comment xml:lang="nl">De relatie tussen een raam en zijn beglazing.</rdfs:comment>
        <rdfs:comment xml:lang="en">The relationship between a window and its glazing.</rdfs:comment>
        <rdfs:label xml:lang="en">has glazing</rdfs:label>
        <rdfs:label xml:lang="nl">heeft beglazing</rdfs:label>
    </owl:ObjectProperty>
    


    <!-- https://w3id.org/reno#hasGlazingType -->


    <owl:ObjectProperty rdf:about="https://w3id.org/reno#hasGlazingType">
        <rdf:type rdf:resource="http://www.w3.org/2002/07/owl#FunctionalProperty"/>
        <rdfs:domain rdf:resource="https://w3id.org/reno#WindowGlazing"/>
        <rdfs:range rdf:resource="https://w3id.org/reno#WindowGlazingType"/>
        <rdfs:comment xml:lang="nl">De relatie tussen raambeglazing en het type.</rdfs:comment>
        <rdfs:comment xml:lang="en">The relationship between window glazing and its type.</rdfs:comment>
        <rdfs:label xml:lang="en">has glazing type</rdfs:label>
        <rdfs:label xml:lang="nl">heeft beglazingstype</rdfs:label>
    </owl:ObjectProperty>
    


    <!-- https://w3id.org/reno#hasHeatingPeriod -->


    <owl:ObjectProperty rdf:about="https://w3id.org/reno#hasHeatingPeriod">
        <rdfs:domain rdf:resource="https://w3id.org/bot#Space"/>
        <rdfs:range rdf:resource="https://w3id.org/reno#HeatingPeriod"/>
        <rdfs:comment xml:lang="nl">De relatie tussen een ruimte en zijn verwarmingsperiode.</rdfs:comment>
        <rdfs:comment xml:lang="en">The relationship between a space and its heating period.</rdfs:comment>
        <rdfs:label xml:lang="en">has heating period</rdfs:label>
        <rdfs:label xml:lang="nl">heeft verwarmingsperiode</rdfs:label>
    </owl:ObjectProperty>
    


    <!-- https://w3id.org/reno#hasInsulationGrade -->


    <owl:ObjectProperty rdf:about="https://w3id.org/reno#hasInsulationGrade">
        <rdf:type rdf:resource="http://www.w3.org/2002/07/owl#FunctionalProperty"/>
        <rdfs:domain rdf:resource="https://pi.pauwel.be/voc/buildingelement#BuildingElement"/>
        <rdfs:range rdf:resource="https://w3id.org/reno#InsulationGrade"/>
        <rdfs:comment xml:lang="nl">De relatie tussen een gebouwelement en de mate waarin het geïsoleerd is.</rdfs:comment>
        <rdfs:comment xml:lang="en">The relationship between a building element and its grade of insulation.</rdfs:comment>
        <rdfs:label xml:lang="en">has insulation grade</rdfs:label>
        <rdfs:label xml:lang="nl">heeft isolatiegraad</rdfs:label>
    </owl:ObjectProperty>
    


    <!-- https://w3id.org/reno#hasMotivation -->


    <owl:ObjectProperty rdf:about="https://w3id.org/reno#hasMotivation">
        <rdfs:domain rdf:resource="http://xmlns.com/foaf/spec/Person"/>
        <rdfs:range rdf:resource="https://w3id.org/reno#Motivation"/>
        <rdfs:comment xml:lang="nl">De relatie tussen een persoon en hun motivatie.</rdfs:comment>
        <rdfs:comment xml:lang="en">The relationship between a person and their motivation.</rdfs:comment>
        <rdfs:label xml:lang="en">has motivation</rdfs:label>
        <rdfs:label xml:lang="nl">heeft motivatie</rdfs:label>
    </owl:ObjectProperty>
    


    <!-- https://w3id.org/reno#hasOrientation -->


    <owl:ObjectProperty rdf:about="https://w3id.org/reno#hasOrientation">
        <rdf:type rdf:resource="http://www.w3.org/2002/07/owl#FunctionalProperty"/>
        <rdfs:domain rdf:resource="https://w3id.org/bot#Space"/>
        <rdfs:range rdf:resource="https://w3id.org/reno#Orientation"/>
        <rdfs:comment xml:lang="nl">De relatie tussen een ruimte en zijn oriëntatie.</rdfs:comment>
        <rdfs:comment xml:lang="en">The relationship between a space and the orientation it faces.</rdfs:comment>
        <rdfs:label xml:lang="en">orientation</rdfs:label>
        <rdfs:label xml:lang="nl">oriëntatie</rdfs:label>
    </owl:ObjectProperty>
    


    <!-- https://w3id.org/reno#hasOwner -->


    <owl:ObjectProperty rdf:about="https://w3id.org/reno#hasOwner">
        <rdfs:domain rdf:resource="https://w3id.org/bot#Zone"/>
        <rdfs:range rdf:resource="https://w3id.org/reno#Owner"/>
        <owl:propertyChainAxiom rdf:parseType="Collection">
            <rdf:Description rdf:about="https://w3id.org/bot#containsZone"/>
            <rdf:Description rdf:about="https://w3id.org/reno#hasOwner"/>
        </owl:propertyChainAxiom>
        <rdfs:comment xml:lang="nl">De relatie tussen een zone en de persoon die het bezit.</rdfs:comment>
        <rdfs:comment xml:lang="en">The relationship between a zone and the person that owns it.</rdfs:comment>
        <rdfs:label xml:lang="en">has owner</rdfs:label>
        <rdfs:label xml:lang="nl">heeft eigenaar</rdfs:label>
    </owl:ObjectProperty>
    


    <!-- https://w3id.org/reno#hasPlannedSpaceUsage -->


    <owl:ObjectProperty rdf:about="https://w3id.org/reno#hasPlannedSpaceUsage">
        <rdfs:domain rdf:resource="https://w3id.org/bot#Space"/>
        <rdfs:range rdf:resource="https://w3id.org/reno#SpaceUsage"/>
        <rdfs:comment xml:lang="nl">De relatie tussen een ruimte en zijn gepland type gebruik.</rdfs:comment>
        <rdfs:comment xml:lang="en">The relationship between a space and its planned type of usage.</rdfs:comment>
        <rdfs:label xml:lang="en">has planned space usage</rdfs:label>
        <rdfs:label xml:lang="nl">heeft gepland ruimtegebruik</rdfs:label>
    </owl:ObjectProperty>
    


    <!-- https://w3id.org/reno#hasPowerConnection -->


    <owl:ObjectProperty rdf:about="https://w3id.org/reno#hasPowerConnection">
        <rdf:type rdf:resource="http://www.w3.org/2002/07/owl#FunctionalProperty"/>
        <rdfs:domain rdf:resource="https://w3id.org/bot#Zone"/>
        <rdfs:range rdf:resource="https://w3id.org/reno#PowerConnection"/>
        <rdfs:comment xml:lang="nl">De relatie tussen een zone en zijn elektriciteitsaansluiting.</rdfs:comment>
        <rdfs:comment xml:lang="en">The relationship between a zone and its power connection.</rdfs:comment>
        <rdfs:label xml:lang="en">has power connection</rdfs:label>
        <rdfs:label xml:lang="nl">heeft elektriciteitsaansluiting</rdfs:label>
    </owl:ObjectProperty>
    


    <!-- https://w3id.org/reno#hasRenovation -->


    <owl:ObjectProperty rdf:about="https://w3id.org/reno#hasRenovation">
        <rdfs:domain rdf:resource="https://w3id.org/bot#Zone"/>
        <rdfs:range rdf:resource="https://w3id.org/reno#Renovation"/>
        <owl:propertyChainAxiom rdf:parseType="Collection">
            <rdf:Description rdf:about="https://w3id.org/bot#hasElement"/>
            <rdf:Description rdf:about="http://bimerr.iot.linkeddata.es/def/material-properties#hasMaterialLayerSet"/>
            <rdf:Description rdf:about="https://w3id.org/reno#changedDuring"/>
            <rdf:Description rdf:about="https://w3id.org/reno#isRenovationInterventionOf"/>
        </owl:propertyChainAxiom>
        <rdfs:comment xml:lang="nl">De relatie tussen een zone en de renovaties ervan. De renovaties kunnen in het verleden, momenteel of in de toekomst zijn.</rdfs:comment>
        <rdfs:comment xml:lang="en">The relationship between a zone and its renovations. The renovations can be in the past, ongoing, or in the future.</rdfs:comment>
        <rdfs:label xml:lang="en">has renovation</rdfs:label>
        <rdfs:label xml:lang="nl">heeft renovatie</rdfs:label>
    </owl:ObjectProperty>
    


    <!-- https://w3id.org/reno#hasRenovationIntervention -->


    <owl:ObjectProperty rdf:about="https://w3id.org/reno#hasRenovationIntervention">
        <rdfs:domain rdf:resource="https://w3id.org/reno#Renovation"/>
        <rdfs:range rdf:resource="https://w3id.org/reno#RenovationIntervention"/>
        <rdfs:comment xml:lang="nl">De relatie tussen een renovatie en de bijhorende renovatie interventie.</rdfs:comment>
        <rdfs:comment xml:lang="en">The relationship between a renovation and the corresponding renovation intervention.</rdfs:comment>
        <rdfs:label xml:lang="en">has renovation intervention</rdfs:label>
        <rdfs:label xml:lang="nl">heeft renovatie interventie</rdfs:label>
    </owl:ObjectProperty>
    


    <!-- https://w3id.org/reno#hasResident -->


    <owl:ObjectProperty rdf:about="https://w3id.org/reno#hasResident">
        <rdfs:domain rdf:resource="https://w3id.org/bot#Zone"/>
        <rdfs:range rdf:resource="https://w3id.org/reno#Resident"/>
        <owl:propertyChainAxiom rdf:parseType="Collection">
            <rdf:Description rdf:about="https://w3id.org/bot#containsZone"/>
            <rdf:Description rdf:about="https://w3id.org/reno#hasResident"/>
        </owl:propertyChainAxiom>
        <rdfs:comment xml:lang="nl">De relatie tussen een persoon en de zone waarin ze wonen. Een zone kan de bewoners van de subzones aggregeren.</rdfs:comment>
        <rdfs:comment xml:lang="en">The relationship between a person and the zone they reside in. A zone can aggregate the residents of its subszones.</rdfs:comment>
        <rdfs:label xml:lang="en">has resident</rdfs:label>
        <rdfs:label xml:lang="nl">heeft bewoner</rdfs:label>
    </owl:ObjectProperty>
    


    <!-- https://w3id.org/reno#hasSigned -->


    <owl:ObjectProperty rdf:about="https://w3id.org/reno#hasSigned">
        <rdfs:domain rdf:resource="http://xmlns.com/foaf/spec/Person"/>
        <rdfs:range rdf:resource="https://w3id.org/reno#Tender"/>
        <rdfs:comment xml:lang="nl">De relatie tussen een persoon en de offerte die door hen ondertekend is.</rdfs:comment>
        <rdfs:comment xml:lang="en">The relationship between a person and the tender they signed.</rdfs:comment>
        <rdfs:label xml:lang="en">has signed</rdfs:label>
        <rdfs:label xml:lang="nl">heeft ondertekend</rdfs:label>
    </owl:ObjectProperty>
    


    <!-- https://w3id.org/reno#hasSpaceUsage -->


    <owl:ObjectProperty rdf:about="https://w3id.org/reno#hasSpaceUsage">
        <rdfs:domain rdf:resource="https://w3id.org/bot#Space"/>
        <rdfs:range rdf:resource="https://w3id.org/reno#SpaceUsage"/>
        <rdfs:comment xml:lang="nl">De relatie tussen een ruimte en zijn type gebruik.</rdfs:comment>
        <rdfs:comment xml:lang="en">The relationship between a space and its type of usage.</rdfs:comment>
        <rdfs:label xml:lang="en">has space usage</rdfs:label>
        <rdfs:label xml:lang="nl">heeft ruimtegebruik</rdfs:label>
    </owl:ObjectProperty>
    


    <!-- https://w3id.org/reno#hasState -->


    <owl:ObjectProperty rdf:about="https://w3id.org/reno#hasState">
        <rdfs:domain rdf:resource="https://w3id.org/bot#Element"/>
        <rdfs:range rdf:resource="https://w3id.org/reno#State"/>
        <rdfs:comment xml:lang="nl">The relatie tussen een element en de staat van dat element.</rdfs:comment>
        <rdfs:comment xml:lang="en">The relationship between an element and the state of that element.</rdfs:comment>
        <rdfs:label xml:lang="en">has state</rdfs:label>
        <rdfs:label xml:lang="nl">heeft staat</rdfs:label>
    </owl:ObjectProperty>
    


    <!-- https://w3id.org/reno#isAddressOf -->


    <owl:ObjectProperty rdf:about="https://w3id.org/reno#isAddressOf">
        <owl:inverseOf rdf:resource="https://w3id.org/reno#hasAddress"/>
        <rdfs:comment xml:lang="nl">De relatie tussen een adres en de persoon die er woont.</rdfs:comment>
        <rdfs:comment xml:lang="en">The relationship between an address and the person who lives there.</rdfs:comment>
        <rdfs:label xml:lang="en">is address of</rdfs:label>
        <rdfs:label xml:lang="nl">is adres van</rdfs:label>
    </owl:ObjectProperty>
    


    <!-- https://w3id.org/reno#isAffectedBy -->


    <owl:ObjectProperty rdf:about="https://w3id.org/reno#isAffectedBy">
        <owl:inverseOf rdf:resource="https://w3id.org/reno#hasAffectedElement"/>
        <rdfs:comment xml:lang="nl">De relatie tussen een (bouw)element en de offerte waardoor het wordt beïnvloed.</rdfs:comment>
        <rdfs:comment xml:lang="en">The relationship between a (building) element and a tender by which it is affected.</rdfs:comment>
        <rdfs:label xml:lang="en">is affected by</rdfs:label>
        <rdfs:label xml:lang="nl">wordt beïnvloed door</rdfs:label>
    </owl:ObjectProperty>
    


    <!-- https://w3id.org/reno#isCreatorOf -->


    <owl:ObjectProperty rdf:about="https://w3id.org/reno#isCreatorOf">
        <owl:inverseOf rdf:resource="https://w3id.org/reno#hasCreator"/>
        <rdf:type rdf:resource="http://www.w3.org/2002/07/owl#InverseFunctionalProperty"/>
        <rdfs:comment xml:lang="nl">De relatie tussen een energiedeskundige en het energieprestatiecertificaat dat door hen werd opgesteld.</rdfs:comment>
        <rdfs:comment xml:lang="en">The relationship between an energy expert and the energy performance certificate they made.</rdfs:comment>
        <rdfs:label xml:lang="en">is creator of</rdfs:label>
        <rdfs:label xml:lang="nl">is maker van</rdfs:label>
    </owl:ObjectProperty>
    


    <!-- https://w3id.org/reno#isFrameOf -->


    <owl:ObjectProperty rdf:about="https://w3id.org/reno#isFrameOf">
        <owl:inverseOf rdf:resource="https://w3id.org/reno#hasFrame"/>
        <rdfs:comment xml:lang="nl">De relatie tussen een kader en het raam waartoe het behoort.</rdfs:comment>
        <rdfs:comment xml:lang="en">The relationship between a frame and the window it belongs to.</rdfs:comment>
        <rdfs:label xml:lang="en">is frame of</rdfs:label>
        <rdfs:label xml:lang="nl">is kader van</rdfs:label>
    </owl:ObjectProperty>
    


    <!-- https://w3id.org/reno#isGlazingOf -->


    <owl:ObjectProperty rdf:about="https://w3id.org/reno#isGlazingOf">
        <owl:inverseOf rdf:resource="https://w3id.org/reno#hasGlazing"/>
        <rdfs:comment xml:lang="nl">De relatie tussen een beglazing en het raam waartoe het behoort.</rdfs:comment>
        <rdfs:comment xml:lang="en">The relationship between a glazing and the window it belongs to.</rdfs:comment>
        <rdfs:label xml:lang="nl">is beglazing van</rdfs:label>
        <rdfs:label xml:lang="en">is glazing of</rdfs:label>
    </owl:ObjectProperty>
    


    <!-- https://w3id.org/reno#isHeatingPeriodOf -->


    <owl:ObjectProperty rdf:about="https://w3id.org/reno#isHeatingPeriodOf">
        <owl:inverseOf rdf:resource="https://w3id.org/reno#hasHeatingPeriod"/>
        <rdfs:comment xml:lang="nl">De relatie tussen een verwarmingsperiode en de bijhorende ruimte.</rdfs:comment>
        <rdfs:comment xml:lang="en">The relationship between a heating period and the space it belongs to.</rdfs:comment>
        <rdfs:label xml:lang="en">is heating period of</rdfs:label>
        <rdfs:label xml:lang="nl">is verwarmingsperiode van</rdfs:label>
    </owl:ObjectProperty>
    


    <!-- https://w3id.org/reno#isInsulationGradeOf -->


    <owl:ObjectProperty rdf:about="https://w3id.org/reno#isInsulationGradeOf">
        <owl:inverseOf rdf:resource="https://w3id.org/reno#hasInsulationGrade"/>
        <rdf:type rdf:resource="http://www.w3.org/2002/07/owl#InverseFunctionalProperty"/>
        <rdfs:comment xml:lang="nl">De relatie tussen een isolatiegraad en het bouwelement waartoe het behoort.</rdfs:comment>
        <rdfs:comment xml:lang="en">The relationship between a grade of insulation and the building element it belongs to.</rdfs:comment>
        <rdfs:label xml:lang="en">is insulation grade of</rdfs:label>
        <rdfs:label xml:lang="nl">is isolatiegraad van</rdfs:label>
    </owl:ObjectProperty>
    


    <!-- https://w3id.org/reno#isMotivationOf -->


    <owl:ObjectProperty rdf:about="https://w3id.org/reno#isMotivationOf">
        <owl:inverseOf rdf:resource="https://w3id.org/reno#hasMotivation"/>
        <rdfs:comment xml:lang="nl">De relatie tussen een motivatie en de bijhorende persoon.</rdfs:comment>
        <rdfs:comment xml:lang="en">The relationship between a motivation and the person it belongs to.</rdfs:comment>
        <rdfs:label xml:lang="nl">is motivatie van</rdfs:label>
        <rdfs:label xml:lang="en">is motivation of</rdfs:label>
    </owl:ObjectProperty>
    


    <!-- https://w3id.org/reno#isOwnerOf -->


    <owl:ObjectProperty rdf:about="https://w3id.org/reno#isOwnerOf">
        <owl:inverseOf rdf:resource="https://w3id.org/reno#hasOwner"/>
        <rdfs:comment xml:lang="nl">De relatie tussen een persoon en het gebouw dat ze bezitten.</rdfs:comment>
        <rdfs:comment xml:lang="en">The relationship between a person and the building they own.</rdfs:comment>
        <rdfs:label xml:lang="nl">is eigenaar van</rdfs:label>
        <rdfs:label xml:lang="en">is owner of</rdfs:label>
    </owl:ObjectProperty>
    


    <!-- https://w3id.org/reno#isRenovationInterventionOf -->


    <owl:ObjectProperty rdf:about="https://w3id.org/reno#isRenovationInterventionOf">
        <owl:inverseOf rdf:resource="https://w3id.org/reno#hasRenovationIntervention"/>
        <rdfs:comment xml:lang="nl">De relatie tussen een renovatie interventie en de renovatie waar die bij hoort.</rdfs:comment>
        <rdfs:comment xml:lang="en">The relationship between a renovation intervention and the renovation it belongs to.</rdfs:comment>
        <rdfs:label xml:lang="nl">is renovatie interventie van</rdfs:label>
        <rdfs:label xml:lang="en">is renovation intervention of</rdfs:label>
    </owl:ObjectProperty>
    


    <!-- https://w3id.org/reno#isResidentOf -->


    <owl:ObjectProperty rdf:about="https://w3id.org/reno#isResidentOf">
        <owl:inverseOf rdf:resource="https://w3id.org/reno#hasResident"/>
        <rdfs:comment xml:lang="nl">De relatie tussen een zone en de persoon die erin woont.</rdfs:comment>
        <rdfs:comment xml:lang="en">The relationship between a zone and the person that resides in it.</rdfs:comment>
        <rdfs:label xml:lang="nl">is bewoner van</rdfs:label>
        <rdfs:label xml:lang="en">is resident of</rdfs:label>
    </owl:ObjectProperty>
    


    <!-- https://w3id.org/reno#isSignedBy -->


    <owl:ObjectProperty rdf:about="https://w3id.org/reno#isSignedBy">
        <owl:inverseOf rdf:resource="https://w3id.org/reno#hasSigned"/>
        <rdfs:comment xml:lang="nl">De relatie tussen een offerte en de persoon die hem ondertekend heeft.</rdfs:comment>
        <rdfs:comment xml:lang="en">The relationship between a tender and the person who signed it.</rdfs:comment>
        <rdfs:label xml:lang="nl">is ondertekend door</rdfs:label>
        <rdfs:label xml:lang="en">is signed by</rdfs:label>
    </owl:ObjectProperty>
    


    <!-- https://w3id.org/reno#isStateOf -->


    <owl:ObjectProperty rdf:about="https://w3id.org/reno#isStateOf">
        <owl:inverseOf rdf:resource="https://w3id.org/reno#hasState"/>
        <rdfs:comment xml:lang="nl">De relatie tussen een toestand en het element waarmee het overeenkomt.</rdfs:comment>
        <rdfs:comment xml:lang="en">The relationship between a state and the element it corresponds to.</rdfs:comment>
        <rdfs:label xml:lang="nl">is staat van</rdfs:label>
        <rdfs:label xml:lang="en">is state of</rdfs:label>
    </owl:ObjectProperty>
    


    <!-- https://w3id.org/reno#wantsToExecute -->


    <owl:ObjectProperty rdf:about="https://w3id.org/reno#wantsToExecute">
        <rdfs:domain rdf:resource="https://w3id.org/reno#Owner"/>
        <rdfs:range rdf:resource="https://saref.etsi.org/core/Task"/>
        <rdfs:comment xml:lang="nl">De relatie tussen een gebouweigenaar en de (renovatie) taken die ze zelf willen uitvoeren.</rdfs:comment>
        <rdfs:comment xml:lang="en">The relationship between a building owner and the (renovation) tasks they want to execute themselves.</rdfs:comment>
        <rdfs:label xml:lang="en">wants to execute</rdfs:label>
        <rdfs:label xml:lang="nl">wilt uitvoeren</rdfs:label>
    </owl:ObjectProperty>
    


    <!-- 
    ///////////////////////////////////////////////////////////////////////////////////////
    //
    // Data properties
    //
    ///////////////////////////////////////////////////////////////////////////////////////
     -->


    


    <!-- http://bimerr.iot.linkeddata.es/def/material-properties#position -->


    <owl:DatatypeProperty rdf:about="http://bimerr.iot.linkeddata.es/def/material-properties#position">
        <rdfs:domain rdf:resource="http://bimerr.iot.linkeddata.es/def/material-properties#MaterialLayer"/>
        <rdfs:range rdf:resource="http://www.w3.org/2001/XMLSchema#integer"/>
        <rdfs:comment>Position of the layer</rdfs:comment>
    </owl:DatatypeProperty>
    


    <!-- http://bimerr.iot.linkeddata.es/def/material-properties#thickness -->


    <owl:DatatypeProperty rdf:about="http://bimerr.iot.linkeddata.es/def/material-properties#thickness">
        <rdfs:domain rdf:resource="http://bimerr.iot.linkeddata.es/def/material-properties#MaterialLayer"/>
        <rdfs:range rdf:resource="http://www.w3.org/2001/XMLSchema#integer"/>
        <rdfs:comment>Thickness of the layer</rdfs:comment>
    </owl:DatatypeProperty>
    


    <!-- http://xmlns.com/foaf/spec/age -->


    <owl:DatatypeProperty rdf:about="http://xmlns.com/foaf/spec/age">
        <rdfs:domain rdf:resource="http://xmlns.com/foaf/spec/Person"/>
        <rdfs:range rdf:resource="http://www.w3.org/2001/XMLSchema#integer"/>
        <rdfs:comment>The age property is a relationship between a Agent and an integer string representing their age in years. See also birthday.</rdfs:comment>
    </owl:DatatypeProperty>
    


    <!-- https://saref.etsi.org/saref4bldg/temperatureClassification -->


    <owl:DatatypeProperty rdf:about="https://saref.etsi.org/saref4bldg/temperatureClassification">
        <rdfs:domain rdf:resource="https://saref.etsi.org/saref4bldg/SpaceHeater"/>
        <rdfs:range rdf:resource="http://www.w3.org/2001/XMLSchema#string"/>
        <rdfs:comment>Enumeration defining the temperature classification of the space heater surface temperature. low temperature - surface temperature is relatively low, usually heated by hot water or electricity. high temperature - surface temperature is relatively high, usually heated by gas or steam.</rdfs:comment>
    </owl:DatatypeProperty>
    


    <!-- https://saref.etsi.org/saref4bldg/thermalEfficiency -->


    <owl:DatatypeProperty rdf:about="https://saref.etsi.org/saref4bldg/thermalEfficiency">
        <rdfs:domain rdf:resource="https://saref.etsi.org/saref4bldg/SpaceHeater"/>
        <rdfs:comment>Overall Thermal Efficiency is defined as gross energy output of the heat transfer device divided by the energy input.</rdfs:comment>
    </owl:DatatypeProperty>
    


    <!-- https://w3id.org/reno#containsAsbestos -->


    <owl:DatatypeProperty rdf:about="https://w3id.org/reno#containsAsbestos">
        <rdf:type rdf:resource="http://www.w3.org/2002/07/owl#FunctionalProperty"/>
        <rdfs:domain rdf:resource="http://bimerr.iot.linkeddata.es/def/material-properties#Material"/>
        <rdfs:range rdf:resource="http://www.w3.org/2001/XMLSchema#boolean"/>
        <rdfs:comment xml:lang="nl">Geeft aan of een materiaal asbest bevat of niet.</rdfs:comment>
        <rdfs:comment xml:lang="en">Indicates whether or not a material contains asbestos.</rdfs:comment>
        <rdfs:label xml:lang="nl">bevat asbest</rdfs:label>
        <rdfs:label xml:lang="en">contains asbestos</rdfs:label>
    </owl:DatatypeProperty>
    


    <!-- https://w3id.org/reno#hasCertificateNumber -->


    <owl:DatatypeProperty rdf:about="https://w3id.org/reno#hasCertificateNumber">
        <rdf:type rdf:resource="http://www.w3.org/2002/07/owl#FunctionalProperty"/>
        <rdfs:domain rdf:resource="https://w3id.org/reno#EnergyPerformanceCertificate"/>
        <rdfs:range rdf:resource="http://www.w3.org/2001/XMLSchema#string"/>
        <rdfs:comment xml:lang="en">Links the energy performance certificate to the corresponding certificate number.</rdfs:comment>
        <rdfs:comment xml:lang="nl">Linkt het energieprestatiecertificaat aan het bijhorende certificaat nummer.</rdfs:comment>
        <rdfs:label xml:lang="en">has certificate number</rdfs:label>
        <rdfs:label xml:lang="nl">heeft certificaat nummer</rdfs:label>
    </owl:DatatypeProperty>
    


    <!-- https://w3id.org/reno#hasCity -->


    <owl:DatatypeProperty rdf:about="https://w3id.org/reno#hasCity">
        <rdf:type rdf:resource="http://www.w3.org/2002/07/owl#FunctionalProperty"/>
        <rdfs:domain rdf:resource="https://w3id.org/reno#Address"/>
        <rdfs:range rdf:resource="http://www.w3.org/2001/XMLSchema#string"/>
        <rdfs:comment xml:lang="en">Links an address to the corresponding city.</rdfs:comment>
        <rdfs:comment xml:lang="nl">Linkt een adres aan de bijhorende stad.</rdfs:comment>
        <rdfs:label xml:lang="en">has city</rdfs:label>
        <rdfs:label xml:lang="nl">heeft stad</rdfs:label>
    </owl:DatatypeProperty>
    


    <!-- https://w3id.org/reno#hasConstructionYear -->


    <owl:DatatypeProperty rdf:about="https://w3id.org/reno#hasConstructionYear">
        <rdf:type rdf:resource="http://www.w3.org/2002/07/owl#FunctionalProperty"/>
        <rdfs:domain rdf:resource="https://w3id.org/bot#Building"/>
        <rdfs:range rdf:resource="http://www.w3.org/2001/XMLSchema#gYear"/>
        <rdfs:comment xml:lang="en">Links a building to the year it was constructed.</rdfs:comment>
        <rdfs:comment xml:lang="nl">Linkt een gebouw aan het jaar waarin het werd gebouwd.</rdfs:comment>
        <rdfs:label xml:lang="en">has construction year</rdfs:label>
        <rdfs:label xml:lang="nl">heeft constructiejaar</rdfs:label>
    </owl:DatatypeProperty>
    


    <!-- https://w3id.org/reno#hasCountry -->


    <owl:DatatypeProperty rdf:about="https://w3id.org/reno#hasCountry">
        <rdf:type rdf:resource="http://www.w3.org/2002/07/owl#FunctionalProperty"/>
        <rdfs:domain rdf:resource="https://w3id.org/reno#Address"/>
        <rdfs:range rdf:resource="http://www.w3.org/2001/XMLSchema#string"/>
        <rdfs:comment xml:lang="en">Links an address to the corresponding country.</rdfs:comment>
        <rdfs:comment xml:lang="nl">Linkt een adres aan de bijhorende land.</rdfs:comment>
        <rdfs:label xml:lang="en">has country</rdfs:label>
        <rdfs:label xml:lang="nl">heeft land</rdfs:label>
    </owl:DatatypeProperty>
    


    <!-- https://w3id.org/reno#hasCreationDate -->


    <owl:DatatypeProperty rdf:about="https://w3id.org/reno#hasCreationDate">
        <rdf:type rdf:resource="http://www.w3.org/2002/07/owl#FunctionalProperty"/>
        <rdfs:domain rdf:resource="https://w3id.org/reno#EnergyPerformanceCertificate"/>
        <rdfs:range rdf:resource="http://www.w3.org/2001/XMLSchema#date"/>
        <rdfs:comment xml:lang="en">Links the energy performance certificate to the date it was created.</rdfs:comment>
        <rdfs:comment xml:lang="nl">Linkt het energieprestatiecertificaat aan de dag waarop het opgesteld is.</rdfs:comment>
        <rdfs:label xml:lang="en">has creation date</rdfs:label>
        <rdfs:label xml:lang="nl">heeft creatie datum</rdfs:label>
    </owl:DatatypeProperty>
    


    <!-- https://w3id.org/reno#hasDesiredEPCLabel -->


    <owl:DatatypeProperty rdf:about="https://w3id.org/reno#hasDesiredEPCLabel">
        <rdfs:domain rdf:resource="https://w3id.org/reno#Owner"/>
        <rdfs:range>
            <rdfs:Datatype>
                <owl:oneOf>
                    <rdf:Description>
                        <rdf:type rdf:resource="http://www.w3.org/1999/02/22-rdf-syntax-ns#List"/>
                        <rdf:first>A</rdf:first>
                        <rdf:rest>
                            <rdf:Description>
                                <rdf:type rdf:resource="http://www.w3.org/1999/02/22-rdf-syntax-ns#List"/>
                                <rdf:first>A+</rdf:first>
                                <rdf:rest>
                                    <rdf:Description>
                                        <rdf:type rdf:resource="http://www.w3.org/1999/02/22-rdf-syntax-ns#List"/>
                                        <rdf:first>B</rdf:first>
                                        <rdf:rest>
                                            <rdf:Description>
                                                <rdf:type rdf:resource="http://www.w3.org/1999/02/22-rdf-syntax-ns#List"/>
                                                <rdf:first>C</rdf:first>
                                                <rdf:rest>
                                                    <rdf:Description>
                                                        <rdf:type rdf:resource="http://www.w3.org/1999/02/22-rdf-syntax-ns#List"/>
                                                        <rdf:first>D</rdf:first>
                                                        <rdf:rest>
                                                            <rdf:Description>
                                                                <rdf:type rdf:resource="http://www.w3.org/1999/02/22-rdf-syntax-ns#List"/>
                                                                <rdf:first>E</rdf:first>
                                                                <rdf:rest>
                                                                    <rdf:Description>
                                                                        <rdf:type rdf:resource="http://www.w3.org/1999/02/22-rdf-syntax-ns#List"/>
                                                                        <rdf:first>F</rdf:first>
                                                                        <rdf:rest rdf:resource="http://www.w3.org/1999/02/22-rdf-syntax-ns#nil"/>
                                                                    </rdf:Description>
                                                                </rdf:rest>
                                                            </rdf:Description>
                                                        </rdf:rest>
                                                    </rdf:Description>
                                                </rdf:rest>
                                            </rdf:Description>
                                        </rdf:rest>
                                    </rdf:Description>
                                </rdf:rest>
                            </rdf:Description>
                        </rdf:rest>
                    </rdf:Description>
                </owl:oneOf>
            </rdfs:Datatype>
        </rdfs:range>
        <rdfs:comment xml:lang="en">Links a person to the EPC label they desire for their property.</rdfs:comment>
        <rdfs:comment xml:lang="nl">Linkt een persoon aan het EPC label dat ze wensen voor hun eigendom.</rdfs:comment>
        <rdfs:label xml:lang="en">has desired EPC label</rdfs:label>
        <rdfs:label xml:lang="nl">heeft gewenst EPC label</rdfs:label>
    </owl:DatatypeProperty>
    


    <!-- https://w3id.org/reno#hasEndDate -->


    <owl:DatatypeProperty rdf:about="https://w3id.org/reno#hasEndDate">
        <rdf:type rdf:resource="http://www.w3.org/2002/07/owl#FunctionalProperty"/>
        <rdfs:domain rdf:resource="https://w3id.org/reno#Renovation"/>
        <rdfs:range rdf:resource="http://www.w3.org/2001/XMLSchema#date"/>
        <rdfs:comment xml:lang="en">Links a renovation to its end date.</rdfs:comment>
        <rdfs:comment xml:lang="nl">Linkt een renovatie aan zijn einddatum.</rdfs:comment>
        <rdfs:label xml:lang="en">has end date</rdfs:label>
        <rdfs:label xml:lang="nl">heeft einddatum</rdfs:label>
    </owl:DatatypeProperty>
    


    <!-- https://w3id.org/reno#hasEndTime -->


    <owl:DatatypeProperty rdf:about="https://w3id.org/reno#hasEndTime">
        <rdf:type rdf:resource="http://www.w3.org/2002/07/owl#FunctionalProperty"/>
        <rdfs:domain rdf:resource="https://w3id.org/reno#HeatingPeriod"/>
        <rdfs:range rdf:resource="http://www.w3.org/2001/XMLSchema#time"/>
        <rdfs:comment xml:lang="en">Links a heating period to its end time.</rdfs:comment>
        <rdfs:comment xml:lang="nl">Linkt een verwarmingsperiode aan zijn eindtijd.</rdfs:comment>
        <rdfs:label xml:lang="en">has end time</rdfs:label>
        <rdfs:label xml:lang="nl">heeft eindtijd</rdfs:label>
    </owl:DatatypeProperty>
    


    <!-- https://w3id.org/reno#hasEnergyScore -->


    <owl:DatatypeProperty rdf:about="https://w3id.org/reno#hasEnergyScore">
        <rdf:type rdf:resource="http://www.w3.org/2002/07/owl#FunctionalProperty"/>
        <rdfs:domain rdf:resource="https://w3id.org/reno#EnergyPerformanceCertificate"/>
        <rdfs:range rdf:resource="http://www.w3.org/2001/XMLSchema#decimal"/>
        <rdfs:comment xml:lang="en">Links the energy performance certificate to the corresponding score.</rdfs:comment>
        <rdfs:comment xml:lang="nl">Linkt het energieprestatiecertificaat aan de bijhorende score</rdfs:comment>
        <rdfs:label xml:lang="en">has energy score</rdfs:label>
        <rdfs:label xml:lang="nl">heeft energie score</rdfs:label>
    </owl:DatatypeProperty>
    


    <!-- https://w3id.org/reno#hasFrameThickness -->


    <owl:DatatypeProperty rdf:about="https://w3id.org/reno#hasFrameThickness">
        <rdf:type rdf:resource="http://www.w3.org/2002/07/owl#FunctionalProperty"/>
        <rdfs:domain rdf:resource="https://w3id.org/reno#WindowFrame"/>
        <rdfs:range rdf:resource="http://www.w3.org/2001/XMLSchema#decimal"/>
        <rdfs:comment xml:lang="en">Links the window frame to its thickness.</rdfs:comment>
        <rdfs:comment xml:lang="nl">Linkt een raamkader aan zijn dikte.</rdfs:comment>
        <rdfs:label xml:lang="en">has frame thickness</rdfs:label>
        <rdfs:label xml:lang="nl">heeft raamkader dikte</rdfs:label>
    </owl:DatatypeProperty>
    


    <!-- https://w3id.org/reno#hasHeatIssue -->


    <owl:DatatypeProperty rdf:about="https://w3id.org/reno#hasHeatIssue">
        <rdf:type rdf:resource="http://www.w3.org/2002/07/owl#FunctionalProperty"/>
        <rdfs:domain rdf:resource="https://w3id.org/bot#Space"/>
        <rdfs:range rdf:resource="http://www.w3.org/2001/XMLSchema#boolean"/>
        <rdfs:comment xml:lang="nl">Geeft aan of een ruimte een hitteprobleem heeft.</rdfs:comment>
        <rdfs:comment xml:lang="en">Indicates whether or not the space has a heat issue.</rdfs:comment>
        <rdfs:label xml:lang="en">has heat issue</rdfs:label>
        <rdfs:label xml:lang="nl">heeft hitteprobleem</rdfs:label>
    </owl:DatatypeProperty>
    


    <!-- https://w3id.org/reno#hasHistoricalProtection -->


    <owl:DatatypeProperty rdf:about="https://w3id.org/reno#hasHistoricalProtection">
        <rdfs:subPropertyOf rdf:resource="https://w3id.org/reno#hasProtection"/>
        <rdf:type rdf:resource="http://www.w3.org/2002/07/owl#FunctionalProperty"/>
        <rdfs:domain rdf:resource="https://pi.pauwel.be/voc/buildingelement#BuildingElement"/>
        <rdfs:range rdf:resource="http://www.w3.org/2001/XMLSchema#boolean"/>
        <rdfs:comment xml:lang="nl">Geeft aan of een gebouwelement historisch beschermd is of niet.</rdfs:comment>
        <rdfs:comment xml:lang="en">Indates whether a building element is historically protected or not.</rdfs:comment>
        <rdfs:label xml:lang="en">has historical protection</rdfs:label>
        <rdfs:label xml:lang="nl">heeft historische bescherming</rdfs:label>
    </owl:DatatypeProperty>
    


    <!-- https://w3id.org/reno#hasHouseNumber -->


    <owl:DatatypeProperty rdf:about="https://w3id.org/reno#hasHouseNumber">
        <rdf:type rdf:resource="http://www.w3.org/2002/07/owl#FunctionalProperty"/>
        <rdfs:domain rdf:resource="https://w3id.org/reno#Address"/>
        <rdfs:range rdf:resource="http://www.w3.org/2001/XMLSchema#string"/>
        <rdfs:comment xml:lang="en">Links an address to the corresponding house number.</rdfs:comment>
        <rdfs:comment xml:lang="nl">Linkt een adres aan de bijhorende huisnummer.</rdfs:comment>
        <rdfs:label xml:lang="en">has house number</rdfs:label>
        <rdfs:label xml:lang="nl">heeft huisnummer</rdfs:label>
    </owl:DatatypeProperty>
    


    <!-- https://w3id.org/reno#hasNetFloorArea -->


    <owl:DatatypeProperty rdf:about="https://w3id.org/reno#hasNetFloorArea">
        <rdf:type rdf:resource="http://www.w3.org/2002/07/owl#FunctionalProperty"/>
        <rdfs:domain rdf:resource="https://w3id.org/bot#Zone"/>
        <rdfs:range rdf:resource="http://www.w3.org/2001/XMLSchema#decimal"/>
        <rdfs:comment xml:lang="en">Links a zone to their net floor area.</rdfs:comment>
        <rdfs:comment xml:lang="nl">Linkt een zone aan zijn netto vloeroppervlakte.</rdfs:comment>
        <rdfs:label xml:lang="en">has net floor area</rdfs:label>
        <rdfs:label xml:lang="nl">heeft netto vloeroppervlakte</rdfs:label>
    </owl:DatatypeProperty>
    


    <!-- https://w3id.org/reno#hasNuisanceScore -->


    <owl:DatatypeProperty rdf:about="https://w3id.org/reno#hasNuisanceScore">
        <rdf:type rdf:resource="http://www.w3.org/2002/07/owl#FunctionalProperty"/>
        <rdfs:domain rdf:resource="https://w3id.org/reno#Owner"/>
        <rdfs:range>
            <rdfs:Datatype>
                <owl:oneOf>
                    <rdf:Description>
                        <rdf:type rdf:resource="http://www.w3.org/1999/02/22-rdf-syntax-ns#List"/>
                        <rdf:first rdf:datatype="http://www.w3.org/2001/XMLSchema#integer">1</rdf:first>
                        <rdf:rest>
                            <rdf:Description>
                                <rdf:type rdf:resource="http://www.w3.org/1999/02/22-rdf-syntax-ns#List"/>
                                <rdf:first rdf:datatype="http://www.w3.org/2001/XMLSchema#integer">10</rdf:first>
                                <rdf:rest>
                                    <rdf:Description>
                                        <rdf:type rdf:resource="http://www.w3.org/1999/02/22-rdf-syntax-ns#List"/>
                                        <rdf:first rdf:datatype="http://www.w3.org/2001/XMLSchema#integer">2</rdf:first>
                                        <rdf:rest>
                                            <rdf:Description>
                                                <rdf:type rdf:resource="http://www.w3.org/1999/02/22-rdf-syntax-ns#List"/>
                                                <rdf:first rdf:datatype="http://www.w3.org/2001/XMLSchema#integer">3</rdf:first>
                                                <rdf:rest>
                                                    <rdf:Description>
                                                        <rdf:type rdf:resource="http://www.w3.org/1999/02/22-rdf-syntax-ns#List"/>
                                                        <rdf:first rdf:datatype="http://www.w3.org/2001/XMLSchema#integer">4</rdf:first>
                                                        <rdf:rest>
                                                            <rdf:Description>
                                                                <rdf:type rdf:resource="http://www.w3.org/1999/02/22-rdf-syntax-ns#List"/>
                                                                <rdf:first rdf:datatype="http://www.w3.org/2001/XMLSchema#integer">5</rdf:first>
                                                                <rdf:rest>
                                                                    <rdf:Description>
                                                                        <rdf:type rdf:resource="http://www.w3.org/1999/02/22-rdf-syntax-ns#List"/>
                                                                        <rdf:first rdf:datatype="http://www.w3.org/2001/XMLSchema#integer">6</rdf:first>
                                                                        <rdf:rest>
                                                                            <rdf:Description>
                                                                                <rdf:type rdf:resource="http://www.w3.org/1999/02/22-rdf-syntax-ns#List"/>
                                                                                <rdf:first rdf:datatype="http://www.w3.org/2001/XMLSchema#integer">7</rdf:first>
                                                                                <rdf:rest>
                                                                                    <rdf:Description>
                                                                                        <rdf:type rdf:resource="http://www.w3.org/1999/02/22-rdf-syntax-ns#List"/>
                                                                                        <rdf:first rdf:datatype="http://www.w3.org/2001/XMLSchema#integer">8</rdf:first>
                                                                                        <rdf:rest>
                                                                                            <rdf:Description>
                                                                                                <rdf:type rdf:resource="http://www.w3.org/1999/02/22-rdf-syntax-ns#List"/>
                                                                                                <rdf:first rdf:datatype="http://www.w3.org/2001/XMLSchema#integer">9</rdf:first>
                                                                                                <rdf:rest rdf:resource="http://www.w3.org/1999/02/22-rdf-syntax-ns#nil"/>
                                                                                            </rdf:Description>
                                                                                        </rdf:rest>
                                                                                    </rdf:Description>
                                                                                </rdf:rest>
                                                                            </rdf:Description>
                                                                        </rdf:rest>
                                                                    </rdf:Description>
                                                                </rdf:rest>
                                                            </rdf:Description>
                                                        </rdf:rest>
                                                    </rdf:Description>
                                                </rdf:rest>
                                            </rdf:Description>
                                        </rdf:rest>
                                    </rdf:Description>
                                </rdf:rest>
                            </rdf:Description>
                        </rdf:rest>
                    </rdf:Description>
                </owl:oneOf>
            </rdfs:Datatype>
        </rdfs:range>
        <rdfs:comment xml:lang="en">Links a building owner to the amount of nuisance they are willing to tolerate during the renovations, on a scale of 1 to 10.</rdfs:comment>
        <rdfs:comment xml:lang="nl">Linkt een gebouweigenaar aan de hoeveelheid overlast die hij bereid is te tolereren tijdens de renovatie, op een schaal van 1 tot 10.</rdfs:comment>
        <rdfs:label xml:lang="en">has nuisance score</rdfs:label>
        <rdfs:label xml:lang="nl">heeft overlastscore</rdfs:label>
    </owl:DatatypeProperty>
    


    <!-- https://w3id.org/reno#hasPostalCode -->


    <owl:DatatypeProperty rdf:about="https://w3id.org/reno#hasPostalCode">
        <rdf:type rdf:resource="http://www.w3.org/2002/07/owl#FunctionalProperty"/>
        <rdfs:domain rdf:resource="https://w3id.org/reno#Address"/>
        <rdfs:range rdf:resource="http://www.w3.org/2001/XMLSchema#string"/>
        <rdfs:comment xml:lang="en">Links an address to the corresponding postal code.</rdfs:comment>
        <rdfs:comment xml:lang="nl">Linkt een adres aan de bijhorende postcode.</rdfs:comment>
        <rdfs:label xml:lang="en">has postal code</rdfs:label>
        <rdfs:label xml:lang="nl">heeft postcode</rdfs:label>
    </owl:DatatypeProperty>
    


    <!-- https://w3id.org/reno#hasPotentialForPV -->


    <owl:DatatypeProperty rdf:about="https://w3id.org/reno#hasPotentialForPV">
        <rdf:type rdf:resource="http://www.w3.org/2002/07/owl#FunctionalProperty"/>
        <rdfs:domain rdf:resource="https://w3id.org/bot#Zone"/>
        <rdfs:range rdf:resource="http://www.w3.org/2001/XMLSchema#boolean"/>
        <rdfs:comment xml:lang="nl">Geeft aan of een zone potentieel heeft om PV-panelen te installeren.</rdfs:comment>
        <rdfs:comment xml:lang="en">Indicates whether or not a zone has potential to install PV-panels.</rdfs:comment>
        <rdfs:label xml:lang="en">has potential for PV</rdfs:label>
        <rdfs:label xml:lang="nl">heeft potentieel voor PV</rdfs:label>
    </owl:DatatypeProperty>
    


    <!-- https://w3id.org/reno#hasProtection -->


    <owl:DatatypeProperty rdf:about="https://w3id.org/reno#hasProtection">
        <rdf:type rdf:resource="http://www.w3.org/2002/07/owl#FunctionalProperty"/>
        <rdfs:domain rdf:resource="https://pi.pauwel.be/voc/buildingelement#BuildingElement"/>
        <rdfs:range rdf:resource="http://www.w3.org/2001/XMLSchema#boolean"/>
        <rdfs:comment xml:lang="nl">Geeft aan of een gebouwelement beschermd is door iets (bijv. historische bescherming) of iemand (bijv. de eigenaar).</rdfs:comment>
        <rdfs:comment xml:lang="en">Indicates whether or not a building element is protected by something (e.g. historical protection) or someone (e.g. the owner).</rdfs:comment>
        <rdfs:label xml:lang="en">has protection</rdfs:label>
        <rdfs:label xml:lang="nl">heeft bescherming</rdfs:label>
    </owl:DatatypeProperty>
    


    <!-- https://w3id.org/reno#hasRenovationBudget -->


    <owl:DatatypeProperty rdf:about="https://w3id.org/reno#hasRenovationBudget">
        <rdf:type rdf:resource="http://www.w3.org/2002/07/owl#FunctionalProperty"/>
        <rdfs:domain rdf:resource="https://w3id.org/reno#Owner"/>
        <rdfs:range rdf:resource="http://www.w3.org/2001/XMLSchema#decimal"/>
        <rdfs:comment xml:lang="en">Links a building owner to their renovation budget.</rdfs:comment>
        <rdfs:comment xml:lang="nl">Linkt een gebouweigenaar aan hun renovatiebudget.</rdfs:comment>
        <rdfs:label xml:lang="en">has renovation budget</rdfs:label>
        <rdfs:label xml:lang="nl">heeft renovatiebudget</rdfs:label>
    </owl:DatatypeProperty>
    


    <!-- https://w3id.org/reno#hasRenovationCost -->


    <owl:DatatypeProperty rdf:about="https://w3id.org/reno#hasRenovationCost">
        <rdf:type rdf:resource="http://www.w3.org/2002/07/owl#FunctionalProperty"/>
        <rdfs:domain rdf:resource="https://w3id.org/reno#Renovation"/>
        <rdfs:range rdf:resource="http://www.w3.org/2001/XMLSchema#decimal"/>
        <rdfs:comment xml:lang="en">Links a renovation to its (estimated) cost.</rdfs:comment>
        <rdfs:comment xml:lang="nl">Linkt een renovatie aan zijn (geraamde) kostprijs.</rdfs:comment>
        <rdfs:label xml:lang="en">has renovation cost</rdfs:label>
        <rdfs:label xml:lang="nl">heeft renovatiekost</rdfs:label>
    </owl:DatatypeProperty>
    


    <!-- https://w3id.org/reno#hasSignatureDate -->


    <owl:DatatypeProperty rdf:about="https://w3id.org/reno#hasSignatureDate">
        <rdfs:domain rdf:resource="https://w3id.org/reno#Tender"/>
        <rdfs:range rdf:resource="http://www.w3.org/2001/XMLSchema#date"/>
        <rdfs:comment xml:lang="nl">De relatie tussen een offerte en de datum waarop deze is geaccepteerd en/of ondertekend.</rdfs:comment>
        <rdfs:comment xml:lang="en">The relationship between a tender and the date it was accepted and/or signed.</rdfs:comment>
        <rdfs:label xml:lang="en">has signature date</rdfs:label>
        <rdfs:label xml:lang="nl">heeft handtekeningsdatum</rdfs:label>
    </owl:DatatypeProperty>
    


    <!-- https://w3id.org/reno#hasStartDate -->


    <owl:DatatypeProperty rdf:about="https://w3id.org/reno#hasStartDate">
        <rdf:type rdf:resource="http://www.w3.org/2002/07/owl#FunctionalProperty"/>
        <rdfs:domain rdf:resource="https://w3id.org/reno#Renovation"/>
        <rdfs:range rdf:resource="http://www.w3.org/2001/XMLSchema#date"/>
        <rdfs:comment xml:lang="en">Links a renovation to its start date. This date can also be in the future to identify a planned renovation.</rdfs:comment>
        <rdfs:comment xml:lang="nl">Linkt een renovatie aan zijn startdatum. Deze datum kan ook in de toekomst liggen om een geplande renovatie aan te duiden.</rdfs:comment>
        <rdfs:label xml:lang="en">has start date</rdfs:label>
        <rdfs:label xml:lang="nl">heeft startdatum</rdfs:label>
    </owl:DatatypeProperty>
    


    <!-- https://w3id.org/reno#hasStartTime -->


    <owl:DatatypeProperty rdf:about="https://w3id.org/reno#hasStartTime">
        <rdf:type rdf:resource="http://www.w3.org/2002/07/owl#FunctionalProperty"/>
        <rdfs:domain rdf:resource="https://w3id.org/reno#HeatingPeriod"/>
        <rdfs:range rdf:resource="http://www.w3.org/2001/XMLSchema#time"/>
        <rdfs:comment xml:lang="en">Links a heating period to its start time.</rdfs:comment>
        <rdfs:comment xml:lang="nl">Linkt een verwarmingsperiode aan zijn starttijd.</rdfs:comment>
        <rdfs:label xml:lang="en">has start time</rdfs:label>
        <rdfs:label xml:lang="nl">heeft starttijd</rdfs:label>
    </owl:DatatypeProperty>
    


    <!-- https://w3id.org/reno#hasStateDate -->


    <owl:DatatypeProperty rdf:about="https://w3id.org/reno#hasStateDate">
        <rdf:type rdf:resource="http://www.w3.org/2002/07/owl#FunctionalProperty"/>
        <rdfs:domain rdf:resource="https://w3id.org/reno#State"/>
        <rdfs:range rdf:resource="http://www.w3.org/2001/XMLSchema#date"/>
        <rdfs:comment xml:lang="en">Links a state to the date the state was observed.</rdfs:comment>
        <rdfs:comment xml:lang="nl">Linkt een staat aan de dag waarop het is waargenomen.</rdfs:comment>
        <rdfs:label xml:lang="en">has state date</rdfs:label>
        <rdfs:label xml:lang="nl">heeft staat datum</rdfs:label>
    </owl:DatatypeProperty>
    


    <!-- https://w3id.org/reno#hasStateValue -->


    <owl:DatatypeProperty rdf:about="https://w3id.org/reno#hasStateValue">
        <rdf:type rdf:resource="http://www.w3.org/2002/07/owl#FunctionalProperty"/>
        <rdfs:domain rdf:resource="https://w3id.org/reno#State"/>
        <rdfs:range>
            <rdfs:Datatype>
                <owl:oneOf>
                    <rdf:Description>
                        <rdf:type rdf:resource="http://www.w3.org/1999/02/22-rdf-syntax-ns#List"/>
                        <rdf:first rdf:datatype="http://www.w3.org/2001/XMLSchema#integer">1</rdf:first>
                        <rdf:rest>
                            <rdf:Description>
                                <rdf:type rdf:resource="http://www.w3.org/1999/02/22-rdf-syntax-ns#List"/>
                                <rdf:first rdf:datatype="http://www.w3.org/2001/XMLSchema#integer">10</rdf:first>
                                <rdf:rest>
                                    <rdf:Description>
                                        <rdf:type rdf:resource="http://www.w3.org/1999/02/22-rdf-syntax-ns#List"/>
                                        <rdf:first rdf:datatype="http://www.w3.org/2001/XMLSchema#integer">2</rdf:first>
                                        <rdf:rest>
                                            <rdf:Description>
                                                <rdf:type rdf:resource="http://www.w3.org/1999/02/22-rdf-syntax-ns#List"/>
                                                <rdf:first rdf:datatype="http://www.w3.org/2001/XMLSchema#integer">3</rdf:first>
                                                <rdf:rest>
                                                    <rdf:Description>
                                                        <rdf:type rdf:resource="http://www.w3.org/1999/02/22-rdf-syntax-ns#List"/>
                                                        <rdf:first rdf:datatype="http://www.w3.org/2001/XMLSchema#integer">4</rdf:first>
                                                        <rdf:rest>
                                                            <rdf:Description>
                                                                <rdf:type rdf:resource="http://www.w3.org/1999/02/22-rdf-syntax-ns#List"/>
                                                                <rdf:first rdf:datatype="http://www.w3.org/2001/XMLSchema#integer">5</rdf:first>
                                                                <rdf:rest>
                                                                    <rdf:Description>
                                                                        <rdf:type rdf:resource="http://www.w3.org/1999/02/22-rdf-syntax-ns#List"/>
                                                                        <rdf:first rdf:datatype="http://www.w3.org/2001/XMLSchema#integer">6</rdf:first>
                                                                        <rdf:rest>
                                                                            <rdf:Description>
                                                                                <rdf:type rdf:resource="http://www.w3.org/1999/02/22-rdf-syntax-ns#List"/>
                                                                                <rdf:first rdf:datatype="http://www.w3.org/2001/XMLSchema#integer">7</rdf:first>
                                                                                <rdf:rest>
                                                                                    <rdf:Description>
                                                                                        <rdf:type rdf:resource="http://www.w3.org/1999/02/22-rdf-syntax-ns#List"/>
                                                                                        <rdf:first rdf:datatype="http://www.w3.org/2001/XMLSchema#integer">8</rdf:first>
                                                                                        <rdf:rest>
                                                                                            <rdf:Description>
                                                                                                <rdf:type rdf:resource="http://www.w3.org/1999/02/22-rdf-syntax-ns#List"/>
                                                                                                <rdf:first rdf:datatype="http://www.w3.org/2001/XMLSchema#integer">9</rdf:first>
                                                                                                <rdf:rest rdf:resource="http://www.w3.org/1999/02/22-rdf-syntax-ns#nil"/>
                                                                                            </rdf:Description>
                                                                                        </rdf:rest>
                                                                                    </rdf:Description>
                                                                                </rdf:rest>
                                                                            </rdf:Description>
                                                                        </rdf:rest>
                                                                    </rdf:Description>
                                                                </rdf:rest>
                                                            </rdf:Description>
                                                        </rdf:rest>
                                                    </rdf:Description>
                                                </rdf:rest>
                                            </rdf:Description>
                                        </rdf:rest>
                                    </rdf:Description>
                                </rdf:rest>
                            </rdf:Description>
                        </rdf:rest>
                    </rdf:Description>
                </owl:oneOf>
            </rdfs:Datatype>
        </rdfs:range>
        <rdfs:comment xml:lang="en">Links a state to its corresponding value, on a scale of 1 to 10.</rdfs:comment>
        <rdfs:comment xml:lang="nl">Linkt een staat aan de bijhorende waarde, op een schaal van 1 tot 10.</rdfs:comment>
        <rdfs:label xml:lang="en">hase state value</rdfs:label>
        <rdfs:label xml:lang="nl">heeft staat waarde</rdfs:label>
    </owl:DatatypeProperty>
    


    <!-- https://w3id.org/reno#hasStreet -->


    <owl:DatatypeProperty rdf:about="https://w3id.org/reno#hasStreet">
        <rdf:type rdf:resource="http://www.w3.org/2002/07/owl#FunctionalProperty"/>
        <rdfs:domain rdf:resource="https://w3id.org/reno#Address"/>
        <rdfs:range rdf:resource="http://www.w3.org/2001/XMLSchema#string"/>
        <rdfs:comment xml:lang="en">Links an address to the corresponding street.</rdfs:comment>
        <rdfs:comment xml:lang="nl">Linkt een adres aan de bijhorende straat.</rdfs:comment>
        <rdfs:label xml:lang="en">has street</rdfs:label>
        <rdfs:label xml:lang="nl">heeft straat</rdfs:label>
    </owl:DatatypeProperty>
    


    <!-- https://w3id.org/reno#hasTemperatureSetPoint -->


    <owl:DatatypeProperty rdf:about="https://w3id.org/reno#hasTemperatureSetPoint">
        <rdf:type rdf:resource="http://www.w3.org/2002/07/owl#FunctionalProperty"/>
        <rdfs:domain rdf:resource="https://w3id.org/reno#HeatingPeriod"/>
        <rdfs:range rdf:resource="http://www.w3.org/2001/XMLSchema#decimal"/>
        <rdfs:comment xml:lang="en">Links a heating period to its temperature setpoint.</rdfs:comment>
        <rdfs:comment xml:lang="nl">Linkt een verwarmingsperiode aan zijn ingestelde temperatuur.</rdfs:comment>
        <rdfs:label xml:lang="en">has temperature setpoint</rdfs:label>
        <rdfs:label xml:lang="nl">heeft temperatuur instelpunt</rdfs:label>
    </owl:DatatypeProperty>
    


    <!-- https://w3id.org/reno#hasThermalBreak -->


    <owl:DatatypeProperty rdf:about="https://w3id.org/reno#hasThermalBreak">
        <rdf:type rdf:resource="http://www.w3.org/2002/07/owl#FunctionalProperty"/>
        <rdfs:domain rdf:resource="https://w3id.org/reno#WindowFrame"/>
        <rdfs:range rdf:resource="http://www.w3.org/2001/XMLSchema#boolean"/>
        <rdfs:comment xml:lang="nl">Geeft aan of een raamkader een thermische onderbreking heeft of niet.</rdfs:comment>
        <rdfs:comment xml:lang="en">Indicates whether a window frame has a thermal break or not.</rdfs:comment>
        <rdfs:label xml:lang="en">has thermal break</rdfs:label>
        <rdfs:label xml:lang="nl">heeft thermische onderbreking</rdfs:label>
    </owl:DatatypeProperty>
    


    <!-- https://w3id.org/reno#hasYearlyConsumption -->


    <owl:DatatypeProperty rdf:about="https://w3id.org/reno#hasYearlyConsumption">
        <rdfs:domain rdf:resource="https://saref.etsi.org/core/Commodity"/>
        <rdfs:range rdf:resource="http://www.w3.org/2001/XMLSchema#decimal"/>
        <rdfs:comment xml:lang="en">Links a commodity to its yearly consumption.</rdfs:comment>
        <rdfs:comment xml:lang="nl">Linkt een drager aan zijn jaarlijks verbruik.</rdfs:comment>
        <rdfs:label xml:lang="en">has yearly consumption</rdfs:label>
        <rdfs:label xml:lang="nl">heeft jaarlijks verbruik</rdfs:label>
    </owl:DatatypeProperty>
    


    <!-- https://w3id.org/reno#hasYearlyCost -->


    <owl:DatatypeProperty rdf:about="https://w3id.org/reno#hasYearlyCost">
        <rdfs:domain rdf:resource="https://saref.etsi.org/core/Commodity"/>
        <rdfs:range rdf:resource="http://www.w3.org/2001/XMLSchema#decimal"/>
        <rdfs:comment xml:lang="en">Links a commodity to its yearly cost.</rdfs:comment>
        <rdfs:comment xml:lang="nl">Linkt een drager aan zijn jaarlijkse kost.</rdfs:comment>
        <rdfs:label xml:lang="en">has yearly cost</rdfs:label>
        <rdfs:label xml:lang="nl">heeft jaarlijkste kost</rdfs:label>
    </owl:DatatypeProperty>
    


    <!-- https://w3id.org/reno#hasYearlyProduction -->


    <owl:DatatypeProperty rdf:about="https://w3id.org/reno#hasYearlyProduction">
        <rdfs:domain rdf:resource="https://saref.etsi.org/saref4bldg/SolarDevice"/>
        <rdfs:range rdf:resource="http://www.w3.org/2001/XMLSchema#decimal"/>
        <rdfs:comment xml:lang="en">Links a solar device to its yearly production.</rdfs:comment>
        <rdfs:comment xml:lang="nl">Linkt een zonne apparaat aan zijn jaarlijkse productie.</rdfs:comment>
        <rdfs:label xml:lang="en">has yearly production</rdfs:label>
        <rdfs:label xml:lang="nl">heeft jaarlijkse productie</rdfs:label>
    </owl:DatatypeProperty>
    


    <!-- https://w3id.org/reno#inFavourOfPVInGarden -->


    <owl:DatatypeProperty rdf:about="https://w3id.org/reno#inFavourOfPVInGarden">
        <rdf:type rdf:resource="http://www.w3.org/2002/07/owl#FunctionalProperty"/>
        <rdfs:domain rdf:resource="https://w3id.org/reno#Owner"/>
        <rdfs:range rdf:resource="http://www.w3.org/2001/XMLSchema#boolean"/>
        <rdfs:comment xml:lang="nl">Geeft aan of een gebouweigenaar voor de installatie van PV-panelen in de tuin is of niet.</rdfs:comment>
        <rdfs:comment xml:lang="en">Indicates whether or not a building owner is in favour of installing PV-panels in the garden.</rdfs:comment>
        <rdfs:label xml:lang="en">in favour of PV in garden</rdfs:label>
        <rdfs:label xml:lang="nl">voor PV in tuin</rdfs:label>
    </owl:DatatypeProperty>
    


    <!-- https://w3id.org/reno#inProtectedArea -->


    <owl:DatatypeProperty rdf:about="https://w3id.org/reno#inProtectedArea">
        <rdf:type rdf:resource="http://www.w3.org/2002/07/owl#FunctionalProperty"/>
        <rdfs:domain rdf:resource="https://w3id.org/bot#Site"/>
        <rdfs:range rdf:resource="http://www.w3.org/2001/XMLSchema#boolean"/>
        <rdfs:comment xml:lang="nl">Geeft aan of een terrein in een beschermde zone ligt of niet.</rdfs:comment>
        <rdfs:comment xml:lang="en">Indicates whether or not the site is located in a protected area or not.</rdfs:comment>
        <rdfs:label xml:lang="nl">in beschermde zone</rdfs:label>
        <rdfs:label xml:lang="en">in protected area</rdfs:label>
    </owl:DatatypeProperty>
    


    <!-- https://w3id.org/reno#isValidUntil -->


    <owl:DatatypeProperty rdf:about="https://w3id.org/reno#isValidUntil">
        <rdf:type rdf:resource="http://www.w3.org/2002/07/owl#FunctionalProperty"/>
        <rdfs:domain rdf:resource="https://w3id.org/reno#EnergyPerformanceCertificate"/>
        <rdfs:range rdf:resource="http://www.w3.org/2001/XMLSchema#date"/>
        <rdfs:comment xml:lang="en">Links the energy performance certificate to the date until which it is valid.</rdfs:comment>
        <rdfs:comment xml:lang="nl">Linkt het energieprestatiecertificaat aan de dag tot wanneer het geldig is.</rdfs:comment>
        <rdfs:label xml:lang="nl">is geldig tot</rdfs:label>
        <rdfs:label xml:lang="en">is valid until</rdfs:label>
    </owl:DatatypeProperty>
    


    <!-- https://w3id.org/reno#ownerSince -->


    <owl:DatatypeProperty rdf:about="https://w3id.org/reno#ownerSince">
        <rdfs:domain rdf:resource="https://w3id.org/reno#Owner"/>
        <rdfs:range rdf:resource="http://www.w3.org/2001/XMLSchema#gYear"/>
        <rdfs:comment xml:lang="en">Links a person to the year in which they became owner of the building.</rdfs:comment>
        <rdfs:comment xml:lang="nl">Linkt een persoon aan het jaar waarin ze eigenaar van het gebouw werden.</rdfs:comment>
        <rdfs:label xml:lang="nl">eigenaar sinds</rdfs:label>
        <rdfs:label xml:lang="en">owner since</rdfs:label>
    </owl:DatatypeProperty>
    


    <!-- https://w3id.org/reno#ownerUntil -->


    <owl:DatatypeProperty rdf:about="https://w3id.org/reno#ownerUntil">
        <rdfs:domain rdf:resource="https://w3id.org/reno#Owner"/>
        <rdfs:range rdf:resource="http://www.w3.org/2001/XMLSchema#gYear"/>
        <rdfs:comment xml:lang="en">Links a person to the year until which they owned the building</rdfs:comment>
        <rdfs:comment xml:lang="nl">Linkt een persoon aan het jaar tot wanneer ze eigenaar van het gebouw waren.</rdfs:comment>
        <rdfs:label xml:lang="nl">eigenaar tot</rdfs:label>
        <rdfs:label xml:lang="en">owner until</rdfs:label>
    </owl:DatatypeProperty>
    


    <!-- https://w3id.org/reno#potentialForHorizontalGeothermalCaptation -->


    <owl:DatatypeProperty rdf:about="https://w3id.org/reno#potentialForHorizontalGeothermalCaptation">
        <rdf:type rdf:resource="http://www.w3.org/2002/07/owl#FunctionalProperty"/>
        <rdfs:domain rdf:resource="https://w3id.org/bot#Site"/>
        <rdfs:range rdf:resource="http://www.w3.org/2001/XMLSchema#boolean"/>
        <rdfs:comment xml:lang="nl">Geeft aan of een terrein potentieel heeft om een horizontaal geothermisch captatienet te plaatsen.</rdfs:comment>
        <rdfs:comment xml:lang="en">Indicates whether or not a site has potential to place a horizontal geothermal captation.</rdfs:comment>
        <rdfs:label xml:lang="en">potential for horizontal geothermal captation</rdfs:label>
        <rdfs:label xml:lang="nl">potentieel voor horizontaal geothermisch captatienet</rdfs:label>
    </owl:DatatypeProperty>
    


    <!-- https://w3id.org/reno#potentialForVerticalGeothermalDrilling -->


    <owl:DatatypeProperty rdf:about="https://w3id.org/reno#potentialForVerticalGeothermalDrilling">
        <rdf:type rdf:resource="http://www.w3.org/2002/07/owl#FunctionalProperty"/>
        <rdfs:domain rdf:resource="https://w3id.org/bot#Site"/>
        <rdfs:range rdf:resource="http://www.w3.org/2001/XMLSchema#boolean"/>
        <rdfs:comment xml:lang="nl">Geeft aan of een terrein potentieel heeft om een verticale geothermisch boring uit te voeren.</rdfs:comment>
        <rdfs:comment xml:lang="en">Indicates whether or not a site has potential to perform a vertical geothermal drilling.</rdfs:comment>
        <rdfs:label xml:lang="en">potential for vertical geothermal drilling</rdfs:label>
        <rdfs:label xml:lang="nl">potentieel voor verticale geothermisch boring</rdfs:label>
    </owl:DatatypeProperty>
    


    <!-- https://w3id.org/reno#presenceOfHeatGrid -->


    <owl:DatatypeProperty rdf:about="https://w3id.org/reno#presenceOfHeatGrid">
        <rdf:type rdf:resource="http://www.w3.org/2002/07/owl#FunctionalProperty"/>
        <rdfs:domain rdf:resource="https://w3id.org/bot#Building"/>
        <rdfs:range rdf:resource="http://www.w3.org/2001/XMLSchema#boolean"/>
        <rdfs:comment xml:lang="nl">Geeft aan of er een warmtenet aanwezig is in de nabijheid van het gebouw.</rdfs:comment>
        <rdfs:comment xml:lang="en">Indicates whether or not there is a heat grid available near the building.</rdfs:comment>
        <rdfs:label xml:lang="nl">aanwezigheid van warmtenet</rdfs:label>
        <rdfs:label xml:lang="en">presence of heat grid</rdfs:label>
    </owl:DatatypeProperty>
    


    <!-- https://w3id.org/reno#residentSince -->


    <owl:DatatypeProperty rdf:about="https://w3id.org/reno#residentSince">
        <rdfs:domain rdf:resource="https://w3id.org/reno#Resident"/>
        <rdfs:range rdf:resource="http://www.w3.org/2001/XMLSchema#gYear"/>
        <rdfs:comment xml:lang="en">Links a person to the year in which they started inhabiting the building.</rdfs:comment>
        <rdfs:comment xml:lang="nl">Linkt een persoon aan het jaar waarin ze het gebouw zijn gaan bewonen.</rdfs:comment>
        <rdfs:label xml:lang="nl">bewoner sinds</rdfs:label>
        <rdfs:label xml:lang="en">resident since</rdfs:label>
    </owl:DatatypeProperty>
    


    <!-- https://w3id.org/reno#residentUntil -->


    <owl:DatatypeProperty rdf:about="https://w3id.org/reno#residentUntil">
        <rdfs:domain rdf:resource="https://w3id.org/reno#Resident"/>
        <rdfs:range rdf:resource="http://www.w3.org/2001/XMLSchema#gYear"/>
        <rdfs:comment xml:lang="en">Links a person to the year until which they inhabited the building.</rdfs:comment>
        <rdfs:comment xml:lang="nl">Linkt een persoon aan het jaar tot wanneer ze het gebouw bewoonden.</rdfs:comment>
        <rdfs:label xml:lang="nl">bewoner tot</rdfs:label>
        <rdfs:label xml:lang="en">resident until</rdfs:label>
    </owl:DatatypeProperty>
    


    <!-- https://w3id.org/reno#satisfiedWithRevenuePV -->


    <owl:DatatypeProperty rdf:about="https://w3id.org/reno#satisfiedWithRevenuePV">
        <rdf:type rdf:resource="http://www.w3.org/2002/07/owl#FunctionalProperty"/>
        <rdfs:domain rdf:resource="https://w3id.org/reno#Owner"/>
        <rdfs:range rdf:resource="http://www.w3.org/2001/XMLSchema#boolean"/>
        <rdfs:comment xml:lang="nl">Geeft aan of een gebouweigenaar tevreden is met de opbrengst van de geïnstalleerde PV-panelen of niet.</rdfs:comment>
        <rdfs:comment xml:lang="en">Indicates whether or not a building owner is satisfied with the revenue of the installed PV-panels or not.</rdfs:comment>
        <rdfs:label xml:lang="en">satisfied with revenue PV</rdfs:label>
        <rdfs:label xml:lang="nl">tevreden met opbrengst PV</rdfs:label>
    </owl:DatatypeProperty>
    


    <!-- 
    ///////////////////////////////////////////////////////////////////////////////////////
    //
    // Classes
    //
    ///////////////////////////////////////////////////////////////////////////////////////
     -->


    


    <!-- http://bimerr.iot.linkeddata.es/def/material-properties#Air -->


    <owl:Class rdf:about="http://bimerr.iot.linkeddata.es/def/material-properties#Air">
        <rdfs:subClassOf rdf:resource="http://bimerr.iot.linkeddata.es/def/material-properties#Material"/>
    </owl:Class>
    


    <!-- http://bimerr.iot.linkeddata.es/def/material-properties#BuildingBoard -->


    <owl:Class rdf:about="http://bimerr.iot.linkeddata.es/def/material-properties#BuildingBoard">
        <rdfs:subClassOf rdf:resource="http://bimerr.iot.linkeddata.es/def/material-properties#Material"/>
    </owl:Class>
    


    <!-- http://bimerr.iot.linkeddata.es/def/material-properties#Concrete -->


    <owl:Class rdf:about="http://bimerr.iot.linkeddata.es/def/material-properties#Concrete">
        <rdfs:subClassOf rdf:resource="http://bimerr.iot.linkeddata.es/def/material-properties#Material"/>
    </owl:Class>
    


    <!-- http://bimerr.iot.linkeddata.es/def/material-properties#ConstructiveSolidWood -->


    <owl:Class rdf:about="http://bimerr.iot.linkeddata.es/def/material-properties#ConstructiveSolidWood">
        <rdfs:subClassOf rdf:resource="http://bimerr.iot.linkeddata.es/def/material-properties#Material"/>
    </owl:Class>
    


    <!-- http://bimerr.iot.linkeddata.es/def/material-properties#FacadeCladding -->


    <owl:Class rdf:about="http://bimerr.iot.linkeddata.es/def/material-properties#FacadeCladding">
        <rdfs:subClassOf rdf:resource="http://bimerr.iot.linkeddata.es/def/material-properties#Material"/>
    </owl:Class>
    


    <!-- http://bimerr.iot.linkeddata.es/def/material-properties#FloorCoveringAndSkirtingBoard -->


    <owl:Class rdf:about="http://bimerr.iot.linkeddata.es/def/material-properties#FloorCoveringAndSkirtingBoard">
        <rdfs:subClassOf rdf:resource="http://bimerr.iot.linkeddata.es/def/material-properties#Material"/>
    </owl:Class>
    


    <!-- http://bimerr.iot.linkeddata.es/def/material-properties#InsulationMaterial -->


    <owl:Class rdf:about="http://bimerr.iot.linkeddata.es/def/material-properties#InsulationMaterial">
        <rdfs:subClassOf rdf:resource="http://bimerr.iot.linkeddata.es/def/material-properties#Material"/>
    </owl:Class>
    


    <!-- http://bimerr.iot.linkeddata.es/def/material-properties#Masonry -->


    <owl:Class rdf:about="http://bimerr.iot.linkeddata.es/def/material-properties#Masonry">
        <rdfs:subClassOf rdf:resource="http://bimerr.iot.linkeddata.es/def/material-properties#Material"/>
    </owl:Class>
    


    <!-- http://bimerr.iot.linkeddata.es/def/material-properties#Material -->


    <owl:Class rdf:about="http://bimerr.iot.linkeddata.es/def/material-properties#Material">
        <rdfs:comment>A homogeneous or inhomogeneous substance that can be used to form elements (physical products or their components). (Definition taken from IFC)</rdfs:comment>
    </owl:Class>
    


    <!-- http://bimerr.iot.linkeddata.es/def/material-properties#MaterialLayer -->


    <owl:Class rdf:about="http://bimerr.iot.linkeddata.es/def/material-properties#MaterialLayer">
        <rdfs:comment>A single and identifiable part of an element which is constructed of a number of layers (one or more).</rdfs:comment>
    </owl:Class>
    


    <!-- http://bimerr.iot.linkeddata.es/def/material-properties#MaterialLayerSet -->


    <owl:Class rdf:about="http://bimerr.iot.linkeddata.es/def/material-properties#MaterialLayerSet">
        <rdfs:comment>A designation by which materials of an element constructed of a number of material layers is known and through which the relative positioning of individual layers can be expressed.</rdfs:comment>
    </owl:Class>
    


    <!-- http://bimerr.iot.linkeddata.es/def/material-properties#NaturalStone -->


    <owl:Class rdf:about="http://bimerr.iot.linkeddata.es/def/material-properties#NaturalStone">
        <rdfs:subClassOf rdf:resource="http://bimerr.iot.linkeddata.es/def/material-properties#Material"/>
    </owl:Class>
    


    <!-- http://bimerr.iot.linkeddata.es/def/material-properties#PlasterAndMortar -->


    <owl:Class rdf:about="http://bimerr.iot.linkeddata.es/def/material-properties#PlasterAndMortar">
        <rdfs:subClassOf rdf:resource="http://bimerr.iot.linkeddata.es/def/material-properties#Material"/>
    </owl:Class>
    


    <!-- http://bimerr.iot.linkeddata.es/def/material-properties#RoofCovering -->


    <owl:Class rdf:about="http://bimerr.iot.linkeddata.es/def/material-properties#RoofCovering">
        <rdfs:subClassOf rdf:resource="http://bimerr.iot.linkeddata.es/def/material-properties#Material"/>
    </owl:Class>
    


    <!-- http://bimerr.iot.linkeddata.es/def/material-properties#Screed -->


    <owl:Class rdf:about="http://bimerr.iot.linkeddata.es/def/material-properties#Screed">
        <rdfs:subClassOf rdf:resource="http://bimerr.iot.linkeddata.es/def/material-properties#Material"/>
    </owl:Class>
    


    <!-- http://bimerr.iot.linkeddata.es/def/material-properties#WallPaintAndCovering -->


    <owl:Class rdf:about="http://bimerr.iot.linkeddata.es/def/material-properties#WallPaintAndCovering">
        <rdfs:subClassOf rdf:resource="http://bimerr.iot.linkeddata.es/def/material-properties#Material"/>
    </owl:Class>
    


    <!-- http://www.daml.org/services/owl-s/1.1/Process.owl#AtomicProcess -->


    <owl:Class rdf:about="http://www.daml.org/services/owl-s/1.1/Process.owl#AtomicProcess">
        <rdfs:subClassOf rdf:resource="http://www.daml.org/services/owl-s/1.1/Process.owl#Process"/>
    </owl:Class>
    


    <!-- http://www.daml.org/services/owl-s/1.1/Process.owl#CompositeProcess -->


    <owl:Class rdf:about="http://www.daml.org/services/owl-s/1.1/Process.owl#CompositeProcess">
        <owl:equivalentClass>
            <owl:Class>
                <owl:intersectionOf rdf:parseType="Collection">
                    <rdf:Description rdf:about="http://www.daml.org/services/owl-s/1.1/Process.owl#Process"/>
                    <owl:Restriction>
                        <owl:onProperty rdf:resource="http://www.daml.org/services/owl-s/1.1/Process.owl#composedOf"/>
                        <owl:cardinality rdf:datatype="http://www.w3.org/2001/XMLSchema#nonNegativeInteger">1</owl:cardinality>
                    </owl:Restriction>
                </owl:intersectionOf>
            </owl:Class>
        </owl:equivalentClass>
        <rdfs:subClassOf rdf:resource="http://www.daml.org/services/owl-s/1.1/Process.owl#Process"/>
        <rdfs:comment>A CompositeProcess can have at most one invocable property. Similarly for computedInput, computedOutput, computedEffect, and computedPrecondition.</rdfs:comment>
        <rdfs:comment>A CompositeProcess must have exactly 1 composedOf property.</rdfs:comment>
    </owl:Class>
    


    <!-- http://www.daml.org/services/owl-s/1.1/Process.owl#ControlConstruct -->


    <owl:Class rdf:about="http://www.daml.org/services/owl-s/1.1/Process.owl#ControlConstruct">
        <rdfs:comment>A ControlConstruct can have at most one instance of timeout.</rdfs:comment>
    </owl:Class>
    


    <!-- http://www.daml.org/services/owl-s/1.1/Process.owl#Perform -->


    <owl:Class rdf:about="http://www.daml.org/services/owl-s/1.1/Process.owl#Perform">
        <rdfs:subClassOf rdf:resource="http://www.daml.org/services/owl-s/1.1/Process.owl#ControlConstruct"/>
        <rdfs:subClassOf>
            <owl:Restriction>
                <owl:onProperty rdf:resource="http://www.daml.org/services/owl-s/1.1/Process.owl#process"/>
                <owl:cardinality rdf:datatype="http://www.w3.org/2001/XMLSchema#nonNegativeInteger">1</owl:cardinality>
            </owl:Restriction>
        </rdfs:subClassOf>
        <rdfs:comment>The PERFORM construct is how one references a process in a composite process. This is analogous to a function call in a program body. The inputs to the PERFORM are described using the hasDataFrom property.</rdfs:comment>
    </owl:Class>
    


    <!-- http://www.daml.org/services/owl-s/1.1/Process.owl#Process -->


    <owl:Class rdf:about="http://www.daml.org/services/owl-s/1.1/Process.owl#Process">
        <rdfs:comment>A Process can have at most one name, but names need not be unique.</rdfs:comment>
        <rdfs:comment>The most general class of processes</rdfs:comment>
    </owl:Class>
    


    <!-- http://www.daml.org/services/owl-s/1.1/Process.owl#Result -->


    <owl:Class rdf:about="http://www.daml.org/services/owl-s/1.1/Process.owl#Result">
        <rdfs:label>Result</rdfs:label>
    </owl:Class>
    


    <!-- http://www.daml.org/services/owl-s/1.1/Process.owl#Sequence -->


    <owl:Class rdf:about="http://www.daml.org/services/owl-s/1.1/Process.owl#Sequence">
        <rdfs:comment>Sequence is defined as having a list of component processes that specify the body. The Preconditions, parameters and effects of the sequence are not defined in the minimal version.  An obvious extension would be to define the effect of the sequence to be the union of the effect of the individual members, and the parameters of the sequence to be the union of the parameters of individual members. However, some implementations may decide to use the last event&apos;s effects as the effect of the sequence, etc.</rdfs:comment>
    </owl:Class>
    


    <!-- http://www.daml.org/services/owl-s/1.1/Process.owl#SimpleProcess -->


    <owl:Class rdf:about="http://www.daml.org/services/owl-s/1.1/Process.owl#SimpleProcess">
        <rdfs:subClassOf rdf:resource="http://www.daml.org/services/owl-s/1.1/Process.owl#Process"/>
    </owl:Class>
    


    <!-- http://www.daml.org/services/owl-s/1.1/generic/Expression.owl#Condition -->


    <owl:Class rdf:about="http://www.daml.org/services/owl-s/1.1/generic/Expression.owl#Condition"/>
    


    <!-- http://xmlns.com/foaf/spec/Agent -->


    <owl:Class rdf:about="http://xmlns.com/foaf/spec/Agent">
        <rdfs:comment>The Agent class is the class of agents; things that do stuff. A well known sub-class is Person, representing people. Other kinds of agents include Organization and Group. The Agent class is useful in a few places in FOAF where Person would have been overly specific. For example, the IM chat ID properties such as jabberID are typically associated with people, but sometimes belong to software bots.</rdfs:comment>
    </owl:Class>
    


    <!-- http://xmlns.com/foaf/spec/Person -->


    <owl:Class rdf:about="http://xmlns.com/foaf/spec/Person">
        <rdfs:subClassOf rdf:resource="http://xmlns.com/foaf/spec/Agent"/>
        <rdfs:comment>The Person class represents people. Something is a Person if it is a person. We don&apos;t nitpic about whether they&apos;re alive, dead, real, or imaginary. The Person class is a sub-class of the Agent class, since all people are considered &apos;agents&apos; in FOAF.</rdfs:comment>
    </owl:Class>
    


    <!-- https://pi.pauwel.be/voc/buildingelement#BuildingElement -->


    <owl:Class rdf:about="https://pi.pauwel.be/voc/buildingelement#BuildingElement">
        <rdfs:subClassOf rdf:resource="https://w3id.org/bot#Element"/>
        <rdfs:comment>Comprises all elements that are primarily part of the construction of a building, i.e., its structural and space separating system. Building elements are all physically existent and tangible things.</rdfs:comment>
    </owl:Class>
    


    <!-- https://pi.pauwel.be/voc/buildingelement#Floor -->


    <owl:Class rdf:about="https://pi.pauwel.be/voc/buildingelement#Floor">
        <rdfs:subClassOf rdf:resource="https://pi.pauwel.be/voc/buildingelement#Slab"/>
        <rdfs:comment>http://bsdd.buildingsmart.org/#concept/details/0jBALpJIv7vvlWkbd9HdCx</rdfs:comment>
    </owl:Class>
    


    <!-- https://pi.pauwel.be/voc/buildingelement#Roof -->


    <owl:Class rdf:about="https://pi.pauwel.be/voc/buildingelement#Roof">
        <rdfs:subClassOf rdf:resource="https://pi.pauwel.be/voc/buildingelement#BuildingElement"/>
        <rdfs:comment>A covering of the top part of a building. Protects the building against the effects of weather.</rdfs:comment>
    </owl:Class>
    


    <!-- https://pi.pauwel.be/voc/buildingelement#Roof-FLAT_ROOF -->


    <owl:Class rdf:about="https://pi.pauwel.be/voc/buildingelement#Roof-FLAT_ROOF">
        <rdfs:subClassOf rdf:resource="https://pi.pauwel.be/voc/buildingelement#Roof"/>
        <rdfs:comment>http://bsdd.buildingsmart.org/#concept/details/3IeKrtrMz2SQN7qpJt82e5</rdfs:comment>
    </owl:Class>
    


    <!-- https://pi.pauwel.be/voc/buildingelement#Roof-GABLE_ROOF -->


    <owl:Class rdf:about="https://pi.pauwel.be/voc/buildingelement#Roof-GABLE_ROOF">
        <rdfs:subClassOf rdf:resource="https://pi.pauwel.be/voc/buildingelement#Roof"/>
        <rdfs:comment>http://bsdd.buildingsmart.org/#concept/details/0gHJNRNhz6LOTHVbnW$nEj</rdfs:comment>
    </owl:Class>
    


    <!-- https://pi.pauwel.be/voc/buildingelement#Slab -->


    <owl:Class rdf:about="https://pi.pauwel.be/voc/buildingelement#Slab">
        <rdfs:subClassOf rdf:resource="https://pi.pauwel.be/voc/buildingelement#BuildingElement"/>
        <rdfs:comment>A component of the construction that normally encloses a space vertically. May provide the lower support (floor) or upper construction (roof slab) in any space in a building. Only the core or constructional part of this construction is considered to be a slab. The upper finish (flooring, roofing) and the lower finish (ceiling, suspended ceiling) are considered to be coverings.</rdfs:comment>
    </owl:Class>
    


    <!-- https://pi.pauwel.be/voc/buildingelement#Wall -->


    <owl:Class rdf:about="https://pi.pauwel.be/voc/buildingelement#Wall">
        <rdfs:subClassOf rdf:resource="https://pi.pauwel.be/voc/buildingelement#BuildingElement"/>
        <rdfs:comment>A vertical construction that bounds or subdivides spaces. Usually vertical, or nearly vertical, planar elements, often designed to bear structural loads. However not required to be load bearing.</rdfs:comment>
    </owl:Class>
    


    <!-- https://pi.pauwel.be/voc/buildingelement#Window -->


    <owl:Class rdf:about="https://pi.pauwel.be/voc/buildingelement#Window">
        <rdfs:subClassOf rdf:resource="https://pi.pauwel.be/voc/buildingelement#BuildingElement"/>
        <rdfs:comment>building component for closing an opening in a wall or pitched roof that will admit light and may provide ventilation</rdfs:comment>
    </owl:Class>
    


    <!-- https://saref.etsi.org/core/Commodity -->


    <owl:Class rdf:about="https://saref.etsi.org/core/Commodity">
        <rdfs:comment>A marketable item which may be supplied without qualitative differentiation.</rdfs:comment>
    </owl:Class>
    


    <!-- https://saref.etsi.org/core/Device -->


    <owl:Class rdf:about="https://saref.etsi.org/core/Device">
        <rdfs:subClassOf rdf:resource="https://w3id.org/bot#Element"/>
        <rdfs:comment>A tangible object designed to accomplish a particular task. In order to accomplish this task, the device performs one or more functions. An instance of saref:Device represents one specific real world entity.</rdfs:comment>
    </owl:Class>
    


    <!-- https://saref.etsi.org/core/EnergyCommodity -->


    <owl:Class rdf:about="https://saref.etsi.org/core/EnergyCommodity">
        <rdfs:subClassOf rdf:resource="https://saref.etsi.org/core/Commodity"/>
        <rdfs:comment>The class of energy commodities</rdfs:comment>
    </owl:Class>
    


    <!-- https://saref.etsi.org/core/NaturalResourceCommodity -->


    <owl:Class rdf:about="https://saref.etsi.org/core/NaturalResourceCommodity">
        <rdfs:subClassOf rdf:resource="https://saref.etsi.org/core/Commodity"/>
        <rdfs:comment>The class of natural resource commodities</rdfs:comment>
    </owl:Class>
    


    <!-- https://saref.etsi.org/core/Task -->


    <owl:Class rdf:about="https://saref.etsi.org/core/Task">
        <rdfs:comment>The goal for which a device is designed, from a user perspective.</rdfs:comment>
    </owl:Class>
    


    <!-- https://saref.etsi.org/saref4bldg/Boiler -->


    <owl:Class rdf:about="https://saref.etsi.org/saref4bldg/Boiler">
        <rdfs:subClassOf rdf:resource="https://saref.etsi.org/saref4bldg/EnergyConversionDevice"/>
        <rdfs:comment>A boiler is a closed, pressure-rated vessel in which water or other fluid is heated using an energy source such as natural gas, heating oil, or electricity. The fluid in the vessel is then circulated out of the boiler for use in various processes or heating applications.</rdfs:comment>
    </owl:Class>
    


    <!-- https://saref.etsi.org/saref4bldg/BuildingDevice -->


    <owl:Class rdf:about="https://saref.etsi.org/saref4bldg/BuildingDevice">
        <rdfs:subClassOf rdf:resource="https://saref.etsi.org/core/Device"/>
        <rdfs:subClassOf rdf:resource="https://saref.etsi.org/saref4bldg/BuildingObject"/>
        <rdfs:comment>A tangible object designed to accomplish a particular task in a building.</rdfs:comment>
    </owl:Class>
    


    <!-- https://saref.etsi.org/saref4bldg/BuildingObject -->


    <owl:Class rdf:about="https://saref.etsi.org/saref4bldg/BuildingObject">
        <rdfs:subClassOf rdf:resource="https://saref.etsi.org/saref4bldg/PhysicalObject"/>
        <rdfs:comment>An object in the building that can be controlled by devices, such as a door or a window that can be automatically opened or closed by an actuator. (Definition taken from SAREF 1.0)</rdfs:comment>
    </owl:Class>
    


    <!-- https://saref.etsi.org/saref4bldg/Chiller -->


    <owl:Class rdf:about="https://saref.etsi.org/saref4bldg/Chiller">
        <rdfs:subClassOf rdf:resource="https://saref.etsi.org/saref4bldg/EnergyConversionDevice"/>
        <rdfs:comment>A chiller is a device used to remove heat from a liquid via a vapor-compression or absorption refrigeration cycle to cool a fluid, typically water or a mixture of water and glycol. The chilled fluid is then used to cool and dehumidify air in a building.</rdfs:comment>
    </owl:Class>
    


    <!-- https://saref.etsi.org/saref4bldg/DistributionDevice -->


    <owl:Class rdf:about="https://saref.etsi.org/saref4bldg/DistributionDevice">
        <rdfs:subClassOf rdf:resource="https://saref.etsi.org/saref4bldg/BuildingDevice"/>
        <rdfs:comment>Generalization of all devices that participate in a distribution system. (Definition adapated from http://www.buildingsmart-tech.org/ifc/IFC4/Add1/html/schema/ifcproductextension/lexical/ifcdistributionelement.htm)</rdfs:comment>
    </owl:Class>
    


    <!-- https://saref.etsi.org/saref4bldg/DistributionFlowDevice -->


    <owl:Class rdf:about="https://saref.etsi.org/saref4bldg/DistributionFlowDevice">
        <rdfs:subClassOf rdf:resource="https://saref.etsi.org/saref4bldg/DistributionDevice"/>
        <rdfs:comment>Represents devices of a distribution system that facilitate the distribution of energy or matter, such as air, water or power. (Definition adapated from http://www.buildingsmart-tech.org/ifc/IFC4/Add1/html/schema/ifcsharedbldgserviceelements/lexical/ifcdistributionflowelement.htm)</rdfs:comment>
    </owl:Class>
    


    <!-- https://saref.etsi.org/saref4bldg/EnergyConversionDevice -->


    <owl:Class rdf:about="https://saref.etsi.org/saref4bldg/EnergyConversionDevice">
        <rdfs:subClassOf rdf:resource="https://saref.etsi.org/saref4bldg/DistributionFlowDevice"/>
        <rdfs:comment>The distribution flow element EnergyConversionDevice defines the occurrence of a device used to perform energy conversion or heat transfer and typically participates in a flow distribution system.</rdfs:comment>
    </owl:Class>
    


    <!-- https://saref.etsi.org/saref4bldg/FlowMovingDevice -->


    <owl:Class rdf:about="https://saref.etsi.org/saref4bldg/FlowMovingDevice">
        <rdfs:subClassOf rdf:resource="https://saref.etsi.org/saref4bldg/DistributionFlowDevice"/>
        <rdfs:comment>The distribution flow element FlowMovingDevice defines the occurrence of an apparatus used to distribute, circulate or perform conveyance of fluids, including liquids and gases (such as a pump or fan), and typically participates in a flow distribution system.</rdfs:comment>
    </owl:Class>
    


    <!-- https://saref.etsi.org/saref4bldg/FlowTerminal -->


    <owl:Class rdf:about="https://saref.etsi.org/saref4bldg/FlowTerminal">
        <rdfs:subClassOf rdf:resource="https://saref.etsi.org/saref4bldg/DistributionFlowDevice"/>
        <rdfs:comment>The distribution flow element FlowTerminal defines the occurrence of a permanently attached element that acts as a terminus or beginning of a distribution system (such as an air outlet, drain, water closet, or sink). A terminal is typically a point at which a system interfaces with an external environment.</rdfs:comment>
    </owl:Class>
    


    <!-- https://saref.etsi.org/saref4bldg/PhysicalObject -->


    <owl:Class rdf:about="https://saref.etsi.org/saref4bldg/PhysicalObject">
        <rdfs:comment>Any Object that has a proper space region. (Definition extracted from DUL ontology)</rdfs:comment>
    </owl:Class>
    


    <!-- https://saref.etsi.org/saref4bldg/ShadingDevice -->


    <owl:Class rdf:about="https://saref.etsi.org/saref4bldg/ShadingDevice">
        <rdfs:subClassOf rdf:resource="https://saref.etsi.org/saref4bldg/BuildingDevice"/>
        <rdfs:comment>Shading devices are purpose built devices to protect from the sunlight, from natural light, or screening them from view. Shading devices can form part of the facade or can be mounted inside the building, they can be fixed or operable.</rdfs:comment>
    </owl:Class>
    


    <!-- https://saref.etsi.org/saref4bldg/SolarDevice -->


    <owl:Class rdf:about="https://saref.etsi.org/saref4bldg/SolarDevice">
        <rdfs:subClassOf rdf:resource="https://saref.etsi.org/saref4bldg/EnergyConversionDevice"/>
        <rdfs:comment>A solar device converts solar radiation into other energy such as electric current or thermal energy.</rdfs:comment>
    </owl:Class>
    


    <!-- https://saref.etsi.org/saref4bldg/SpaceHeater -->


    <owl:Class rdf:about="https://saref.etsi.org/saref4bldg/SpaceHeater">
        <rdfs:subClassOf rdf:resource="https://saref.etsi.org/saref4bldg/FlowTerminal"/>
        <rdfs:comment>Space heaters utilize a combination of radiation and/or natural convection using a heating source such as electricity, steam or hot water to heat a limited space or area. Examples of space heaters include radiators, convectors, baseboard and finned-tube heaters. UnitaryEquipment should be used for packaged units supporting a combination of heating, cooling, and/or dehumidification; Coil should be used for coil-based floor heating.</rdfs:comment>
    </owl:Class>
    


    <!-- https://w3id.org/bot#Building -->


    <owl:Class rdf:about="https://w3id.org/bot#Building">
        <rdfs:subClassOf rdf:resource="https://w3id.org/bot#Zone"/>
        <owl:disjointWith rdf:resource="https://w3id.org/bot#Site"/>
        <owl:disjointWith rdf:resource="https://w3id.org/bot#Space"/>
        <owl:disjointWith rdf:resource="https://w3id.org/bot#Storey"/>
        <rdfs:comment xml:lang="en">An independent unit of the built environment with a characteristic spatial structure, intended to serve at least one function or user activity [ISO 12006-2:2013]. A bot:Building is a part of the physical world or a virtual world that is inherently both located in this world and having a 3D spatial extent, is contained in a building site, and can contain one or more storeys that are vertically connected.</rdfs:comment>
        <rdfs:comment xml:lang="nl">Een onafhankelijke entiteit met een ruimtelijke structuur die onderdeel is van de gebouwde omgeving, en bedoeld is om minimaal één functie of gebruikersactiviteit te bedienen [ISO 12006-2:2013]. Een bot:Building is deel van de fysieke wereld of een virtuele wereld dat zowel gelokaliseerd kan worden in deze wereld als een ruimtelijke omvang heeft, is deel van een gebouwsite, en kan één of meerder verdiepingen bevatten die verticaal verbonden zijn.</rdfs:comment>
        <rdfs:label xml:lang="en">Building</rdfs:label>
        <rdfs:label xml:lang="nl">Gebouw</rdfs:label>
    </owl:Class>
    


    <!-- https://w3id.org/bot#Element -->


    <owl:Class rdf:about="https://w3id.org/bot#Element">
        <owl:disjointWith rdf:resource="https://w3id.org/bot#Zone"/>
        <rdfs:comment xml:lang="nl">Bestanddeel van een gebouwde entiteit met een karakteristieke technische functie, vorm of positie [ISO 12006-2:2015, 3.4.7]</rdfs:comment>
        <rdfs:comment xml:lang="en">Constituent of a construction entity with a characteristic technical function, form or position [ISO 12006-2:2015, 3.4.7]</rdfs:comment>
        <rdfs:label xml:lang="en">Building element</rdfs:label>
        <rdfs:label xml:lang="nl">Gebouwelement</rdfs:label>
    </owl:Class>
    


    <!-- https://w3id.org/bot#Site -->


    <owl:Class rdf:about="https://w3id.org/bot#Site">
        <rdfs:subClassOf rdf:resource="https://w3id.org/bot#Zone"/>
        <owl:disjointWith rdf:resource="https://w3id.org/bot#Space"/>
        <owl:disjointWith rdf:resource="https://w3id.org/bot#Storey"/>
        <rdfs:comment xml:lang="en">A part of the physical world or a virtual world that is inherently both located in this world and having a 3D spatial extent. It is intended to contain or contains one or more buildings.</rdfs:comment>
        <rdfs:comment xml:lang="nl">Een deel van de fysieke wereld of een virtuele wereld dat zowel gelokaliseerd kan worden in deze wereld als een ruimtelijke omvang heeft. Het is bedoeld om één of meerdere gebouwen te bevatten of bevat al één of meerdere gebouwen.</rdfs:comment>
        <rdfs:label xml:lang="en">Site</rdfs:label>
        <rdfs:label xml:lang="nl">Terrein</rdfs:label>
    </owl:Class>
    


    <!-- https://w3id.org/bot#Space -->


    <owl:Class rdf:about="https://w3id.org/bot#Space">
        <rdfs:subClassOf rdf:resource="https://w3id.org/bot#Zone"/>
        <owl:disjointWith rdf:resource="https://w3id.org/bot#Storey"/>
        <rdfs:comment xml:lang="en">A part of the physical world or a virtual world whose 3D spatial extent is bounded actually or theoretically, and provides for certain functions within the zone it is contained in.</rdfs:comment>
        <rdfs:comment xml:lang="nl">Een deel van de fysieke wereld of een virtuele wereld waarvan de driedimensionale omvang feitelijk of virtueel begrensd is, en dat bepaalde activiteiten faciliteert in de zone die de ruimte bevat.</rdfs:comment>
        <rdfs:label xml:lang="nl">Ruimte</rdfs:label>
        <rdfs:label xml:lang="en">Space</rdfs:label>
    </owl:Class>
    


    <!-- https://w3id.org/bot#Storey -->


    <owl:Class rdf:about="https://w3id.org/bot#Storey">
        <rdfs:subClassOf rdf:resource="https://w3id.org/bot#Zone"/>
        <rdfs:comment xml:lang="en">A part of the physical world or a virtual world that is inherently both located in this world and having a 3D spatial extent. A bot:Storey is contained in one or more buildings, and is intended to contain one or more spaces that are horizontally connected. Storeys of a building are connected by means of vertical connections such as elevators and stairs. A bot:Storey encompasses both zones above and below ground, for example, a building with 21 floors above ground, one ground floor and 3 basements is equal to the sentence: A building has 25 instances of bot:Storey.</rdfs:comment>
        <rdfs:comment xml:lang="nl">Een deel van de fysieke wereld of een virtuele wereld dat zowel gelokaliseerd kan worden in deze wereld als een ruimtelijke omvang heeft. Een bot:Storey is deel van één of meerdere gebouwen, en is bedoeld om één of meerdere ruimtes te bevatten die horizontaal geconnecteerd zijn. De verdiepingen van een gebouw zijn verbonden door middel van verticale connecties zoals liften en trappen. Een bot:Storey omvat zowel zones boven als onder de grond, bijvoorbeeld een gebouw met 21 verdiepingen boven de grond, één gelijkvloers en 3 kelderverdiepingen is evenwaardig aan de zin: Een gebouw heeft 25 instanties van bot:Storey.</rdfs:comment>
        <rdfs:label xml:lang="en">Storey</rdfs:label>
        <rdfs:label xml:lang="nl">Verdieping</rdfs:label>
    </owl:Class>
    


    <!-- https://w3id.org/bot#Zone -->


    <owl:Class rdf:about="https://w3id.org/bot#Zone">
        <rdfs:comment xml:lang="en">A part of the physical world or a virtual world that is inherently both located in this world and has a 3D spatial extent; Sub-classes of bot:Zone include bot:Site, bot:Building, bot:Storey, or bot:Space.  An instance of bot:Zone can contain other bot:Zone instances, making it possible to group or subdivide zones. An instance of bot:Zone can be adjacent to or intersecting other bot:Zone instances. Finally, a bot:Zone can instantiate three relations to bot:Element, which are either contained in (bot:containsElement), adjacent to it (bot:adjacentElement) or intersecting (bot:intersectingElement).</rdfs:comment>
        <rdfs:comment xml:lang="nl">Een deel van de fysieke wereld of een virtuele wereld dat zowel gelokaliseerd kan worden in deze wereld als een ruimtelijke omvang heeft; subklasses van bot:Zone zijn bot:Site, bot:Building, bot:Storey of bot:Space. Een instantie van bot:Zone kan een ander bot:Zone instantie bevatten, wat gebruikt kan worden om zones te groeperen of op te delen. Een instantie van bot:Zone kan aangrenzend zijn aan of snijdend met een andere bot:Zone instantie. Ten slotte kan een bot:Zone instantie drie relaties hebben met een bot:Element instantie dat het ofwel bevat (bot:containsElement), waar het aangrenzend aan is (bot:adjacentElement) of waarmee het snijdt (bot:intersectingElement).</rdfs:comment>
        <rdfs:label xml:lang="en">Zone</rdfs:label>
        <rdfs:label xml:lang="nl">Zone</rdfs:label>
    </owl:Class>
    


    <!-- https://w3id.org/reno#AALabel -->


    <owl:Class rdf:about="https://w3id.org/reno#AALabel">
        <owl:equivalentClass>
            <owl:Class>
                <owl:intersectionOf rdf:parseType="Collection">
                    <rdf:Description rdf:about="https://w3id.org/reno#EnergyPerformanceCertificate"/>
                    <owl:Restriction>
                        <owl:onProperty rdf:resource="https://w3id.org/reno#hasEnergyScore"/>
                        <owl:someValuesFrom>
                            <rdfs:Datatype>
                                <owl:onDatatype rdf:resource="http://www.w3.org/2001/XMLSchema#decimal"/>
                                <owl:withRestrictions rdf:parseType="Collection">
                                    <rdf:Description>
                                        <xsd:maxExclusive rdf:datatype="http://www.w3.org/2001/XMLSchema#integer">0</xsd:maxExclusive>
                                    </rdf:Description>
                                </owl:withRestrictions>
                            </rdfs:Datatype>
                        </owl:someValuesFrom>
                    </owl:Restriction>
                </owl:intersectionOf>
            </owl:Class>
        </owl:equivalentClass>
        <rdfs:comment xml:lang="nl">Het A+ label geeft energieprestatiecertificaten aan met een energiescore lager dan 100 kWh/m²year.</rdfs:comment>
        <rdfs:comment xml:lang="en">The A+ label indicates energy performance certificates which have an energy score of less than 100 kWh/m²year.</rdfs:comment>
        <rdfs:label xml:lang="en">A+ label</rdfs:label>
        <rdfs:label xml:lang="nl">A+ label</rdfs:label>
    </owl:Class>
    


    <!-- https://w3id.org/reno#ALabel -->


    <owl:Class rdf:about="https://w3id.org/reno#ALabel">
        <owl:equivalentClass>
            <owl:Class>
                <owl:intersectionOf rdf:parseType="Collection">
                    <rdf:Description rdf:about="https://w3id.org/reno#EnergyPerformanceCertificate"/>
                    <owl:Restriction>
                        <owl:onProperty rdf:resource="https://w3id.org/reno#hasEnergyScore"/>
                        <owl:someValuesFrom>
                            <rdfs:Datatype>
                                <owl:onDatatype rdf:resource="http://www.w3.org/2001/XMLSchema#decimal"/>
                                <owl:withRestrictions rdf:parseType="Collection">
                                    <rdf:Description>
                                        <xsd:minInclusive rdf:datatype="http://www.w3.org/2001/XMLSchema#integer">0</xsd:minInclusive>
                                    </rdf:Description>
                                    <rdf:Description>
                                        <xsd:maxExclusive rdf:datatype="http://www.w3.org/2001/XMLSchema#integer">100</xsd:maxExclusive>
                                    </rdf:Description>
                                </owl:withRestrictions>
                            </rdfs:Datatype>
                        </owl:someValuesFrom>
                    </owl:Restriction>
                </owl:intersectionOf>
            </owl:Class>
        </owl:equivalentClass>
        <rdfs:comment xml:lang="nl">Het A label geeft energieprestatiecertificaten aan met een energiescore tussen 0 en 100 kWh/m²year.</rdfs:comment>
        <rdfs:comment xml:lang="en">The A label indicates energy performance certificates which have an energy score between 0 and 100 kWh/m²year.</rdfs:comment>
        <rdfs:label xml:lang="en">A label</rdfs:label>
        <rdfs:label xml:lang="nl">A label</rdfs:label>
    </owl:Class>
    


    <!-- https://w3id.org/reno#Address -->


    <owl:Class rdf:about="https://w3id.org/reno#Address">
        <rdfs:subClassOf>
            <owl:Restriction>
                <owl:onProperty rdf:resource="https://w3id.org/reno#hasCity"/>
                <owl:someValuesFrom rdf:resource="http://www.w3.org/2001/XMLSchema#string"/>
            </owl:Restriction>
        </rdfs:subClassOf>
        <rdfs:subClassOf>
            <owl:Restriction>
                <owl:onProperty rdf:resource="https://w3id.org/reno#hasCountry"/>
                <owl:someValuesFrom rdf:resource="http://www.w3.org/2001/XMLSchema#string"/>
            </owl:Restriction>
        </rdfs:subClassOf>
        <rdfs:subClassOf>
            <owl:Restriction>
                <owl:onProperty rdf:resource="https://w3id.org/reno#hasHouseNumber"/>
                <owl:someValuesFrom rdf:resource="http://www.w3.org/2001/XMLSchema#string"/>
            </owl:Restriction>
        </rdfs:subClassOf>
        <rdfs:subClassOf>
            <owl:Restriction>
                <owl:onProperty rdf:resource="https://w3id.org/reno#hasPostalCode"/>
                <owl:someValuesFrom rdf:resource="http://www.w3.org/2001/XMLSchema#string"/>
            </owl:Restriction>
        </rdfs:subClassOf>
        <rdfs:subClassOf>
            <owl:Restriction>
                <owl:onProperty rdf:resource="https://w3id.org/reno#hasStreet"/>
                <owl:someValuesFrom rdf:resource="http://www.w3.org/2001/XMLSchema#string"/>
            </owl:Restriction>
        </rdfs:subClassOf>
        <rdfs:comment xml:lang="en">An address is an indication of a location, in this ontology more specifically of a building.</rdfs:comment>
        <rdfs:comment xml:lang="nl">Een adres is een aanduiding van een locatie, in deze ontologie meer bepaald van een gebouw.</rdfs:comment>
        <rdfs:label xml:lang="en">address</rdfs:label>
        <rdfs:label xml:lang="nl">adres</rdfs:label>
        <rdfs:seeAlso xml:lang="en">https://en.wikipedia.org/wiki/Address</rdfs:seeAlso>
        <rdfs:seeAlso xml:lang="nl">https://nl.wikipedia.org/wiki/Adres_(woonplaats)</rdfs:seeAlso>
    </owl:Class>
    


    <!-- https://w3id.org/reno#AirHeating -->


    <owl:Class rdf:about="https://w3id.org/reno#AirHeating">
        <rdfs:subClassOf rdf:resource="https://saref.etsi.org/saref4bldg/SpaceHeater"/>
        <rdfs:comment xml:lang="en">Air heating is a system that heats air directly and distributes it through ducts and vents to heat up spaces.</rdfs:comment>
        <rdfs:comment xml:lang="nl">Luchtverwarming is een systeem dat lucht rechtstreeks opwarmt en verdeelt via kanalen en roosters om ruimtes te verwarmen.</rdfs:comment>
        <rdfs:label xml:lang="en">air heating</rdfs:label>
        <rdfs:label xml:lang="nl">luchtverwarming</rdfs:label>
        <rdfs:seeAlso xml:lang="nl">https://nl.wikipedia.org/wiki/Luchtverwarming</rdfs:seeAlso>
    </owl:Class>
    


    <!-- https://w3id.org/reno#Aluminium -->


    <owl:Class rdf:about="https://w3id.org/reno#Aluminium">
        <rdfs:subClassOf rdf:resource="https://w3id.org/reno#WindowFrameMaterial"/>
        <rdfs:comment xml:lang="en">Aluminium is a chemical element which has a density lower than that of other common metals, about one-third that of steel.</rdfs:comment>
        <rdfs:comment xml:lang="nl">Aluminium is een chemisch element met een dichtheid die lager is dan die van andere gewone metalen, ongeveer een derde van die van staal.</rdfs:comment>
        <rdfs:label xml:lang="en">aluminium</rdfs:label>
        <rdfs:label xml:lang="nl">aluminium</rdfs:label>
        <rdfs:seeAlso xml:lang="en">https://en.wikipedia.org/wiki/Aluminium</rdfs:seeAlso>
        <rdfs:seeAlso xml:lang="nl">https://nl.wikipedia.org/wiki/Aluminium</rdfs:seeAlso>
    </owl:Class>
    


    <!-- https://w3id.org/reno#AsbestosContaining -->


    <owl:Class rdf:about="https://w3id.org/reno#AsbestosContaining">
        <owl:equivalentClass>
            <owl:Class>
                <owl:intersectionOf rdf:parseType="Collection">
                    <rdf:Description rdf:about="http://bimerr.iot.linkeddata.es/def/material-properties#MaterialLayerSet"/>
                    <owl:Restriction>
                        <owl:onProperty rdf:resource="http://bimerr.iot.linkeddata.es/def/material-properties#hasMaterialLayer"/>
                        <owl:someValuesFrom>
                            <owl:Restriction>
                                <owl:onProperty rdf:resource="http://bimerr.iot.linkeddata.es/def/material-properties#hasMaterial"/>
                                <owl:someValuesFrom>
                                    <owl:Restriction>
                                        <owl:onProperty rdf:resource="https://w3id.org/reno#containsAsbestos"/>
                                        <owl:hasValue rdf:datatype="http://www.w3.org/2001/XMLSchema#boolean">true</owl:hasValue>
                                    </owl:Restriction>
                                </owl:someValuesFrom>
                            </owl:Restriction>
                        </owl:someValuesFrom>
                    </owl:Restriction>
                </owl:intersectionOf>
            </owl:Class>
        </owl:equivalentClass>
        <rdfs:comment xml:lang="en">An asbestos containing element is an element where at least one of the materials contains asbestos.</rdfs:comment>
        <rdfs:comment xml:lang="nl">Een asbesthoudend element is een element waarvan minstens één van de materialen asbest bevat.</rdfs:comment>
        <rdfs:label xml:lang="nl">asbesthoudend</rdfs:label>
        <rdfs:label xml:lang="en">asbestos containing</rdfs:label>
    </owl:Class>
    


    <!-- https://w3id.org/reno#AttachedBuilding -->


    <owl:Class rdf:about="https://w3id.org/reno#AttachedBuilding">
        <rdfs:subClassOf rdf:resource="https://w3id.org/bot#Building"/>
        <owl:disjointWith rdf:resource="https://w3id.org/reno#DetachedBuilding"/>
        <owl:disjointWith rdf:resource="https://w3id.org/reno#SemiDetachedBuilding"/>
        <rdfs:comment xml:lang="en">An attached building is a building that shares a wall with other houses on either side.</rdfs:comment>
        <rdfs:comment xml:lang="nl">Een gesloten bebouwing is een gebouw dat aan weerszijde een muur deelt met andere woningen.</rdfs:comment>
        <rdfs:label xml:lang="en">attached building</rdfs:label>
        <rdfs:label xml:lang="nl">gesloten bebouwing</rdfs:label>
    </owl:Class>
    


    <!-- https://w3id.org/reno#BLabel -->


    <owl:Class rdf:about="https://w3id.org/reno#BLabel">
        <owl:equivalentClass>
            <owl:Class>
                <owl:intersectionOf rdf:parseType="Collection">
                    <rdf:Description rdf:about="https://w3id.org/reno#EnergyPerformanceCertificate"/>
                    <owl:Restriction>
                        <owl:onProperty rdf:resource="https://w3id.org/reno#hasEnergyScore"/>
                        <owl:someValuesFrom>
                            <rdfs:Datatype>
                                <owl:onDatatype rdf:resource="http://www.w3.org/2001/XMLSchema#decimal"/>
                                <owl:withRestrictions rdf:parseType="Collection">
                                    <rdf:Description>
                                        <xsd:minInclusive rdf:datatype="http://www.w3.org/2001/XMLSchema#integer">100</xsd:minInclusive>
                                    </rdf:Description>
                                    <rdf:Description>
                                        <xsd:maxExclusive rdf:datatype="http://www.w3.org/2001/XMLSchema#integer">200</xsd:maxExclusive>
                                    </rdf:Description>
                                </owl:withRestrictions>
                            </rdfs:Datatype>
                        </owl:someValuesFrom>
                    </owl:Restriction>
                </owl:intersectionOf>
            </owl:Class>
        </owl:equivalentClass>
        <rdfs:comment xml:lang="nl">Het B label geeft energieprestatiecertificaten aan met een energiescore tussen 100 en 200 kWh/m²year.</rdfs:comment>
        <rdfs:comment xml:lang="en">The B label indicates energy performance certificates which have an energy score between 100 and 200 kWh/m²year.</rdfs:comment>
        <rdfs:label xml:lang="en">B label</rdfs:label>
        <rdfs:label xml:lang="nl">B label</rdfs:label>
    </owl:Class>
    


    <!-- https://w3id.org/reno#Biomass -->


    <owl:Class rdf:about="https://w3id.org/reno#Biomass">
        <rdfs:subClassOf rdf:resource="https://saref.etsi.org/core/EnergyCommodity"/>
        <rdfs:comment xml:lang="en">Biomass is a term used in several contexts: in the context of ecology it means living organisms, and in the context of bioenergy it means matter from recently living (but now dead) organisms.</rdfs:comment>
        <rdfs:comment xml:lang="nl">Biomassa is een term die in verschillende contexten wordt gebruikt: in de context van ecologie betekent het levende organismen, en in de context van bio-energie betekent het materie van recent levende (maar nu dode) organismen.</rdfs:comment>
        <rdfs:label xml:lang="en">biomass</rdfs:label>
        <rdfs:label xml:lang="nl">biomassa</rdfs:label>
        <rdfs:seeAlso xml:lang="en">https://en.wikipedia.org/wiki/Biomass</rdfs:seeAlso>
        <rdfs:seeAlso xml:lang="nl">https://nl.wikipedia.org/wiki/Biomassa</rdfs:seeAlso>
    </owl:Class>
    


    <!-- https://w3id.org/reno#CLabel -->


    <owl:Class rdf:about="https://w3id.org/reno#CLabel">
        <owl:equivalentClass>
            <owl:Class>
                <owl:intersectionOf rdf:parseType="Collection">
                    <rdf:Description rdf:about="https://w3id.org/reno#EnergyPerformanceCertificate"/>
                    <owl:Restriction>
                        <owl:onProperty rdf:resource="https://w3id.org/reno#hasEnergyScore"/>
                        <owl:someValuesFrom>
                            <rdfs:Datatype>
                                <owl:onDatatype rdf:resource="http://www.w3.org/2001/XMLSchema#decimal"/>
                                <owl:withRestrictions rdf:parseType="Collection">
                                    <rdf:Description>
                                        <xsd:minInclusive rdf:datatype="http://www.w3.org/2001/XMLSchema#integer">200</xsd:minInclusive>
                                    </rdf:Description>
                                    <rdf:Description>
                                        <xsd:maxExclusive rdf:datatype="http://www.w3.org/2001/XMLSchema#integer">300</xsd:maxExclusive>
                                    </rdf:Description>
                                </owl:withRestrictions>
                            </rdfs:Datatype>
                        </owl:someValuesFrom>
                    </owl:Restriction>
                </owl:intersectionOf>
            </owl:Class>
        </owl:equivalentClass>
        <rdfs:comment xml:lang="nl">Het C label geeft energieprestatiecertificaten aan met een energiescore tussen 200 en 300 kWh/m²year.</rdfs:comment>
        <rdfs:comment xml:lang="en">The C label indicates energy performance certificates which have an energy score between 200 and 300 kWh/m²year.</rdfs:comment>
        <rdfs:label xml:lang="en">C label</rdfs:label>
        <rdfs:label xml:lang="nl">C label</rdfs:label>
    </owl:Class>
    


    <!-- https://w3id.org/reno#DLabel -->


    <owl:Class rdf:about="https://w3id.org/reno#DLabel">
        <owl:equivalentClass>
            <owl:Class>
                <owl:intersectionOf rdf:parseType="Collection">
                    <rdf:Description rdf:about="https://w3id.org/reno#EnergyPerformanceCertificate"/>
                    <owl:Restriction>
                        <owl:onProperty rdf:resource="https://w3id.org/reno#hasEnergyScore"/>
                        <owl:someValuesFrom>
                            <rdfs:Datatype>
                                <owl:onDatatype rdf:resource="http://www.w3.org/2001/XMLSchema#decimal"/>
                                <owl:withRestrictions rdf:parseType="Collection">
                                    <rdf:Description>
                                        <xsd:minInclusive rdf:datatype="http://www.w3.org/2001/XMLSchema#integer">300</xsd:minInclusive>
                                    </rdf:Description>
                                    <rdf:Description>
                                        <xsd:maxExclusive rdf:datatype="http://www.w3.org/2001/XMLSchema#integer">400</xsd:maxExclusive>
                                    </rdf:Description>
                                </owl:withRestrictions>
                            </rdfs:Datatype>
                        </owl:someValuesFrom>
                    </owl:Restriction>
                </owl:intersectionOf>
            </owl:Class>
        </owl:equivalentClass>
        <rdfs:comment xml:lang="nl">Het D label geeft energieprestatiecertificaten aan met een energiescore tussen 300 en 400 kWh/m²year.</rdfs:comment>
        <rdfs:comment xml:lang="en">The D label indicates energy performance certificates which have an energy score between 300 and 400 kWh/m²year.</rdfs:comment>
        <rdfs:label xml:lang="en">D label</rdfs:label>
        <rdfs:label xml:lang="nl">D label</rdfs:label>
    </owl:Class>
    


    <!-- https://w3id.org/reno#DetachedBuilding -->


    <owl:Class rdf:about="https://w3id.org/reno#DetachedBuilding">
        <rdfs:subClassOf rdf:resource="https://w3id.org/bot#Building"/>
        <owl:disjointWith rdf:resource="https://w3id.org/reno#SemiDetachedBuilding"/>
        <rdfs:comment xml:lang="en">A detached building is a building that is not connected to any other house, on any side.</rdfs:comment>
        <rdfs:comment xml:lang="nl">Een open bebouwing is een gebouw dat aan geen enkele zijde verbonden is met een andere woning.</rdfs:comment>
        <rdfs:label xml:lang="en">detached building</rdfs:label>
        <rdfs:label xml:lang="nl">open bebouwing</rdfs:label>
        <rdfs:seeAlso xml:lang="en">https://en.wikipedia.org/wiki/Single-family_detached_home</rdfs:seeAlso>
        <rdfs:seeAlso xml:lang="nl">https://nl.wikipedia.org/wiki/Vrijstaand_huis</rdfs:seeAlso>
    </owl:Class>
    


    <!-- https://w3id.org/reno#DoubleGlazing -->


    <owl:Class rdf:about="https://w3id.org/reno#DoubleGlazing">
        <rdfs:subClassOf rdf:resource="https://w3id.org/reno#WindowGlazingType"/>
        <rdfs:comment xml:lang="en">Double glazing consists of two glass window panes seperated by a space. It has a better insulating value than single glazing.</rdfs:comment>
        <rdfs:comment xml:lang="nl">Dubbele beglazing bestaat uit twee glazen ruiten die van elkaar gescheiden zijn door een ruimte. Het heeft een betere isolatiewaarde dan enkel glas.</rdfs:comment>
        <rdfs:label xml:lang="en">double glazing</rdfs:label>
        <rdfs:label xml:lang="nl">dubbel glas</rdfs:label>
        <rdfs:seeAlso xml:lang="en">https://en.wikipedia.org/wiki/Insulated_glazing</rdfs:seeAlso>
        <rdfs:seeAlso xml:lang="nl">https://nl.wikipedia.org/wiki/Dubbelglas</rdfs:seeAlso>
    </owl:Class>
    


    <!-- https://w3id.org/reno#ELabel -->


    <owl:Class rdf:about="https://w3id.org/reno#ELabel">
        <owl:equivalentClass>
            <owl:Class>
                <owl:intersectionOf rdf:parseType="Collection">
                    <rdf:Description rdf:about="https://w3id.org/reno#EnergyPerformanceCertificate"/>
                    <owl:Restriction>
                        <owl:onProperty rdf:resource="https://w3id.org/reno#hasEnergyScore"/>
                        <owl:someValuesFrom>
                            <rdfs:Datatype>
                                <owl:onDatatype rdf:resource="http://www.w3.org/2001/XMLSchema#decimal"/>
                                <owl:withRestrictions rdf:parseType="Collection">
                                    <rdf:Description>
                                        <xsd:minInclusive rdf:datatype="http://www.w3.org/2001/XMLSchema#integer">400</xsd:minInclusive>
                                    </rdf:Description>
                                    <rdf:Description>
                                        <xsd:maxExclusive rdf:datatype="http://www.w3.org/2001/XMLSchema#integer">500</xsd:maxExclusive>
                                    </rdf:Description>
                                </owl:withRestrictions>
                            </rdfs:Datatype>
                        </owl:someValuesFrom>
                    </owl:Restriction>
                </owl:intersectionOf>
            </owl:Class>
        </owl:equivalentClass>
        <rdfs:comment xml:lang="nl">Het E label geeft energieprestatiecertificaten aan met een energiescore tussen 400 en 500 kWh/m²year.</rdfs:comment>
        <rdfs:comment xml:lang="en">The E label indicates energy performance certificates which have an energy score between 400 and 500 kWh/m²year.</rdfs:comment>
        <rdfs:label xml:lang="en">E label</rdfs:label>
        <rdfs:label xml:lang="nl">E label</rdfs:label>
    </owl:Class>
    


    <!-- https://w3id.org/reno#East -->


    <owl:Class rdf:about="https://w3id.org/reno#East">
        <rdfs:subClassOf rdf:resource="https://w3id.org/reno#Orientation"/>
        <rdfs:comment xml:lang="nl">Een van de vier kardinale richtingen, meestal aangeduid als O.</rdfs:comment>
        <rdfs:comment xml:lang="en">One of the four cardinal directions, commonly denoted as E.</rdfs:comment>
        <rdfs:label xml:lang="en">east</rdfs:label>
        <rdfs:label xml:lang="nl">oosten</rdfs:label>
    </owl:Class>
    


    <!-- https://w3id.org/reno#ElectricBoiler -->


    <owl:Class rdf:about="https://w3id.org/reno#ElectricBoiler">
        <rdfs:subClassOf rdf:resource="https://saref.etsi.org/saref4bldg/Boiler"/>
        <rdfs:comment xml:lang="en">An electric boiler is a subtype of a boiler, that uses electricity.</rdfs:comment>
        <rdfs:comment xml:lang="nl">Een elektrische boiler is een subtype van een boiler die gebruikmaakt van elektriciteit.</rdfs:comment>
        <rdfs:label xml:lang="en">electric boiler</rdfs:label>
        <rdfs:label xml:lang="nl">elektrische boiler</rdfs:label>
    </owl:Class>
    


    <!-- https://w3id.org/reno#ElectricConvector -->


    <owl:Class rdf:about="https://w3id.org/reno#ElectricConvector">
        <rdfs:subClassOf rdf:resource="https://saref.etsi.org/saref4bldg/SpaceHeater"/>
        <rdfs:comment xml:lang="en">An electric convector is a heating device that uses electric resistance to warm air, which then circulates through natural convection.</rdfs:comment>
        <rdfs:comment xml:lang="nl">Een elektrische convector is een verwarmingstoestel dat elektrische weerstand gebruikt om lucht op te warmen, die vervolgens door natuurlijke convectie circuleert.</rdfs:comment>
        <rdfs:label xml:lang="en">electric convector</rdfs:label>
        <rdfs:label xml:lang="nl">elektrische convector</rdfs:label>
        <rdfs:seeAlso xml:lang="en">https://en.wikipedia.org/wiki/Convection_heater</rdfs:seeAlso>
        <rdfs:seeAlso xml:lang="nl">https://nl.wikipedia.org/wiki/Convectorkachel</rdfs:seeAlso>
    </owl:Class>
    


    <!-- https://w3id.org/reno#Electricity -->


    <owl:Class rdf:about="https://w3id.org/reno#Electricity">
        <rdfs:subClassOf rdf:resource="https://saref.etsi.org/core/EnergyCommodity"/>
        <rdfs:comment xml:lang="en">Electricity is the set of physical phenomena associated with the presence and motion of matter possessing an electric charge.</rdfs:comment>
        <rdfs:comment xml:lang="nl">Elektriciteit is het geheel van fysische verschijnselen die verband houden met de aanwezigheid en beweging van materie met een elektrische lading.</rdfs:comment>
        <rdfs:label xml:lang="en">electricity</rdfs:label>
        <rdfs:label xml:lang="nl">elektriciteit</rdfs:label>
        <rdfs:seeAlso xml:lang="en">https://en.wikipedia.org/wiki/Electricity</rdfs:seeAlso>
        <rdfs:seeAlso xml:lang="nl">https://nl.wikipedia.org/wiki/Elektriciteit</rdfs:seeAlso>
    </owl:Class>
    


    <!-- https://w3id.org/reno#EnergyExpert -->


    <owl:Class rdf:about="https://w3id.org/reno#EnergyExpert">
        <rdfs:subClassOf rdf:resource="http://xmlns.com/foaf/spec/Person"/>
        <rdfs:subClassOf>
            <owl:Restriction>
                <owl:onProperty rdf:resource="https://w3id.org/reno#isCreatorOf"/>
                <owl:someValuesFrom rdf:resource="https://w3id.org/reno#EnergyPerformanceCertificate"/>
            </owl:Restriction>
        </rdfs:subClassOf>
        <rdfs:comment xml:lang="en">An energy expert is a person who is authorised to create an energy performance certificate</rdfs:comment>
        <rdfs:comment xml:lang="nl">Een energiedeskundige is een persoon die gemachtigd is om een energieprestatiecertificaat op te stellen.</rdfs:comment>
        <rdfs:label xml:lang="nl">energiedeskundige</rdfs:label>
        <rdfs:label xml:lang="en">energy expert</rdfs:label>
        <rdfs:seeAlso xml:lang="nl">https://www.vlaanderen.be/energieprestatiecertificaten-epcs/erkende-energiedeskundigen-voor-epc</rdfs:seeAlso>
    </owl:Class>
    


    <!-- https://w3id.org/reno#EnergyPerformanceCertificate -->


    <owl:Class rdf:about="https://w3id.org/reno#EnergyPerformanceCertificate">
        <rdfs:subClassOf>
            <owl:Restriction>
                <owl:onProperty rdf:resource="https://w3id.org/reno#hasCreator"/>
                <owl:someValuesFrom rdf:resource="https://w3id.org/reno#EnergyExpert"/>
            </owl:Restriction>
        </rdfs:subClassOf>
        <rdfs:subClassOf>
            <owl:Restriction>
                <owl:onProperty rdf:resource="https://w3id.org/reno#hasCertificateNumber"/>
                <owl:someValuesFrom rdf:resource="http://www.w3.org/2001/XMLSchema#string"/>
            </owl:Restriction>
        </rdfs:subClassOf>
        <rdfs:subClassOf>
            <owl:Restriction>
                <owl:onProperty rdf:resource="https://w3id.org/reno#hasCreationDate"/>
                <owl:someValuesFrom rdf:resource="http://www.w3.org/2001/XMLSchema#date"/>
            </owl:Restriction>
        </rdfs:subClassOf>
        <rdfs:subClassOf>
            <owl:Restriction>
                <owl:onProperty rdf:resource="https://w3id.org/reno#hasEnergyScore"/>
                <owl:someValuesFrom rdf:resource="http://www.w3.org/2001/XMLSchema#decimal"/>
            </owl:Restriction>
        </rdfs:subClassOf>
        <rdfs:subClassOf>
            <owl:Restriction>
                <owl:onProperty rdf:resource="https://w3id.org/reno#isValidUntil"/>
                <owl:someValuesFrom rdf:resource="http://www.w3.org/2001/XMLSchema#date"/>
            </owl:Restriction>
        </rdfs:subClassOf>
        <rdfs:comment xml:lang="en">A energy performance certificate (EPC) is a document that summarises the energy efficiency of buildings or building units.</rdfs:comment>
        <rdfs:comment xml:lang="nl">Een energieprestatiecertificaat (EPC) is een document dat weergeeft hoe energiezuinig een gebouw of gebouweenheid is.</rdfs:comment>
        <rdfs:label xml:lang="nl">energieprestatiecertificaat</rdfs:label>
        <rdfs:label xml:lang="en">energy performance certificate</rdfs:label>
        <rdfs:seeAlso xml:lang="en">https://en.wikipedia.org/wiki/Energy_performance_certificate</rdfs:seeAlso>
        <rdfs:seeAlso xml:lang="nl">https://nl.wikipedia.org/wiki/Energieprestatiecertificaat</rdfs:seeAlso>
    </owl:Class>
    


    <!-- https://w3id.org/reno#EnergyReductionMotivation -->


    <owl:Class rdf:about="https://w3id.org/reno#EnergyReductionMotivation">
        <rdfs:subClassOf rdf:resource="https://w3id.org/reno#Motivation"/>
        <rdfs:comment xml:lang="nl">The energie vermindering motivatie van een persoon is de motivatie waarom een persoon zijn energieverbruik wil verlagen.</rdfs:comment>
        <rdfs:comment xml:lang="en">The energy reduction motivation of a person is the motivation why a person wants to reduce their energy consumption.</rdfs:comment>
        <rdfs:label xml:lang="nl">energie vermindering motivatie</rdfs:label>
        <rdfs:label xml:lang="en">energy reduction motivation</rdfs:label>
    </owl:Class>
    


    <!-- https://w3id.org/reno#FLabel -->


    <owl:Class rdf:about="https://w3id.org/reno#FLabel">
        <owl:equivalentClass>
            <owl:Class>
                <owl:intersectionOf rdf:parseType="Collection">
                    <rdf:Description rdf:about="https://w3id.org/reno#EnergyPerformanceCertificate"/>
                    <owl:Restriction>
                        <owl:onProperty rdf:resource="https://w3id.org/reno#hasEnergyScore"/>
                        <owl:someValuesFrom>
                            <rdfs:Datatype>
                                <owl:onDatatype rdf:resource="http://www.w3.org/2001/XMLSchema#decimal"/>
                                <owl:withRestrictions rdf:parseType="Collection">
                                    <rdf:Description>
                                        <xsd:minInclusive rdf:datatype="http://www.w3.org/2001/XMLSchema#integer">500</xsd:minInclusive>
                                    </rdf:Description>
                                </owl:withRestrictions>
                            </rdfs:Datatype>
                        </owl:someValuesFrom>
                    </owl:Restriction>
                </owl:intersectionOf>
            </owl:Class>
        </owl:equivalentClass>
        <rdfs:comment xml:lang="nl">Het F label geeft energieprestatiecertificaten aan met een energiescore hoger dan 500 kWh/m²year.</rdfs:comment>
        <rdfs:comment xml:lang="en">The F label indicates energy performance certificates which have an energy score of more than 500 kWh/m²year.</rdfs:comment>
        <rdfs:label xml:lang="en">F label</rdfs:label>
        <rdfs:label xml:lang="nl">F label</rdfs:label>
    </owl:Class>
    


    <!-- https://w3id.org/reno#FirePlace -->


    <owl:Class rdf:about="https://w3id.org/reno#FirePlace">
        <rdfs:subClassOf rdf:resource="https://saref.etsi.org/saref4bldg/SpaceHeater"/>
        <rdfs:comment xml:lang="en">A fireplace is a structure designed to contain a fire. Fireplaces are used for the relaxing ambiance they create and for heating a room.</rdfs:comment>
        <rdfs:comment xml:lang="nl">Een open haard is een structuur die ontworpen is om vuur te bevatten. Open haarden worden gebruikt voor de ontspannen sfeer die ze creëren en om een kamer te verwarmen.</rdfs:comment>
        <rdfs:label xml:lang="en">fireplace</rdfs:label>
        <rdfs:label xml:lang="nl">open haard</rdfs:label>
        <rdfs:seeAlso xml:lang="en">https://en.wikipedia.org/wiki/Fireplace</rdfs:seeAlso>
        <rdfs:seeAlso xml:lang="nl">https://nl.wikipedia.org/wiki/Open_haard</rdfs:seeAlso>
    </owl:Class>
    


    <!-- https://w3id.org/reno#FloorHeating -->


    <owl:Class rdf:about="https://w3id.org/reno#FloorHeating">
        <rdfs:subClassOf rdf:resource="https://saref.etsi.org/saref4bldg/SpaceHeater"/>
        <rdfs:comment xml:lang="en">Floor heating is a heating system that uses pipes embedded under the floor to evenly distribute heat across the floor surface.</rdfs:comment>
        <rdfs:comment xml:lang="nl">Vloerverwarming is een verwarmingssysteem dat gebruik maakt van buizen onder de vloer om de warmte gelijkmatig over het vloeroppervlak te verdelen.</rdfs:comment>
        <rdfs:label xml:lang="en">floor heating</rdfs:label>
        <rdfs:label xml:lang="nl">vloerverwarming</rdfs:label>
        <rdfs:seeAlso xml:lang="en">https://en.wikipedia.org/wiki/Underfloor_heating</rdfs:seeAlso>
        <rdfs:seeAlso xml:lang="nl">https://nl.wikipedia.org/wiki/Vloerverwarming</rdfs:seeAlso>
    </owl:Class>
    


    <!-- https://w3id.org/reno#FuelOil -->


    <owl:Class rdf:about="https://w3id.org/reno#FuelOil">
        <rdfs:subClassOf rdf:resource="https://saref.etsi.org/core/EnergyCommodity"/>
        <rdfs:comment xml:lang="en">Fuel oil is any of various fractions obtained from the distillation of petroleum (crude oil).</rdfs:comment>
        <rdfs:comment xml:lang="nl">Stookolie is een van de verschillende fracties die worden verkregen uit de destillatie van aardolie (ruwe olie).</rdfs:comment>
        <rdfs:label xml:lang="en">fuel oil</rdfs:label>
        <rdfs:label xml:lang="nl">stookolie</rdfs:label>
        <rdfs:seeAlso xml:lang="en">https://en.wikipedia.org/wiki/Fuel_oil</rdfs:seeAlso>
        <rdfs:seeAlso xml:lang="nl">https://nl.wikipedia.org/wiki/Stookolie</rdfs:seeAlso>
    </owl:Class>
    


    <!-- https://w3id.org/reno#Gas -->


    <owl:Class rdf:about="https://w3id.org/reno#Gas">
        <rdfs:subClassOf rdf:resource="https://saref.etsi.org/core/EnergyCommodity"/>
        <rdfs:subClassOf rdf:resource="https://saref.etsi.org/core/NaturalResourceCommodity"/>
        <rdfs:comment xml:lang="nl">Aardgas is een fossiele brandstof die wordt gevormd wanneer lagen organisch materiaal onder zuurstofloze omstandigheden thermisch worden ontbonden, onderhevig aan intense hitte en druk onder de grond gedurende miljoenen jaren. De energie die de vergane organismen oorspronkelijk via fotosynthese van de zon kregen, wordt als chemische energie in de moleculen opgeslagen. Aardgas kan worden verbrand voor verwarming, koken en het opwekken van elektriciteit.</rdfs:comment>
        <rdfs:comment xml:lang="en">Natural gas is a fossil fuel that is formed when layers of organic matter are thermally decomposed under oxygen-free conditions, subjected to intense heat and pressure underground over millions of years. The energy that the decayed organisms originally obtained from the sun via photosynthesis is stored as chemical energy within the molecules. Natural gas can be burned for heating, cooking, and electricity generation.</rdfs:comment>
        <rdfs:label xml:lang="en">gas</rdfs:label>
        <rdfs:label xml:lang="nl">gas</rdfs:label>
        <rdfs:seeAlso xml:lang="en">https://en.wikipedia.org/wiki/Natural_gas</rdfs:seeAlso>
        <rdfs:seeAlso xml:lang="nl">https://nl.wikipedia.org/wiki/Aardgas</rdfs:seeAlso>
    </owl:Class>
    


    <!-- https://w3id.org/reno#HeatGrid -->


    <owl:Class rdf:about="https://w3id.org/reno#HeatGrid">
        <rdfs:subClassOf rdf:resource="https://saref.etsi.org/saref4bldg/EnergyConversionDevice"/>
        <rdfs:comment xml:lang="en">A heat grid functions as a large-scale central heating system. It brings heat from heat sources to heat consumers.</rdfs:comment>
        <rdfs:comment xml:lang="nl">Een warmtenet functioneert als een grootschalige centrale verwarming. Het brengt warmte van warmtebronnen naar de warmteverbruikers.</rdfs:comment>
        <rdfs:label xml:lang="en">heat grid</rdfs:label>
        <rdfs:label xml:lang="nl">warmtenet</rdfs:label>
        <rdfs:seeAlso xml:lang="nl">https://www.vlaanderen.be/bouwen-wonen-en-energie/groene-energie/warmtenet</rdfs:seeAlso>
    </owl:Class>
    


    <!-- https://w3id.org/reno#HeatPump -->


    <owl:Class rdf:about="https://w3id.org/reno#HeatPump">
        <rdfs:subClassOf rdf:resource="https://saref.etsi.org/saref4bldg/EnergyConversionDevice"/>
        <rdfs:comment xml:lang="en">A heat pump is a device that uses electricity to transfer heat from a colder place to a warmer place. Specifically, the heat pump transfers thermal energy using a heat pump and refrigeration cycle, cooling the cool space and warming the warm space.</rdfs:comment>
        <rdfs:comment xml:lang="nl">Een warmtepomp is een apparaat dat elektriciteit gebruikt om warmte over te brengen van een koudere naar een warmere ruimte. De warmtepomp brengt thermische energie over met behulp van een warmtepomp- en koelcyclus, waarbij de koele ruimte wordt gekoeld en de warme ruimte wordt opgewarmd.</rdfs:comment>
        <rdfs:label xml:lang="en">heat pump</rdfs:label>
        <rdfs:label xml:lang="nl">warmtepomp</rdfs:label>
        <rdfs:seeAlso xml:lang="en">https://en.wikipedia.org/wiki/Heat_pump</rdfs:seeAlso>
        <rdfs:seeAlso xml:lang="nl">https://nl.wikipedia.org/wiki/Warmtepomp</rdfs:seeAlso>
    </owl:Class>
    


    <!-- https://w3id.org/reno#HeatPumpBoiler -->


    <owl:Class rdf:about="https://w3id.org/reno#HeatPumpBoiler">
        <rdfs:subClassOf rdf:resource="https://saref.etsi.org/saref4bldg/Boiler"/>
        <rdfs:comment xml:lang="en">A heat pump boiler is a heat pump that heats domestic water with heat from the air.</rdfs:comment>
        <rdfs:comment xml:lang="nl">Een warmtepompboiler is een warmtepomp die sanitair water verwarmt met warmte uit de lucht.</rdfs:comment>
        <rdfs:label xml:lang="en">heat pump boiler</rdfs:label>
        <rdfs:label xml:lang="nl">warmtepompboiler</rdfs:label>
    </owl:Class>
    


    <!-- https://w3id.org/reno#HeatingPeriod -->


    <owl:Class rdf:about="https://w3id.org/reno#HeatingPeriod">
        <rdfs:subClassOf>
            <owl:Restriction>
                <owl:onProperty rdf:resource="https://w3id.org/reno#hasEndTime"/>
                <owl:someValuesFrom rdf:resource="http://www.w3.org/2001/XMLSchema#time"/>
            </owl:Restriction>
        </rdfs:subClassOf>
        <rdfs:subClassOf>
            <owl:Restriction>
                <owl:onProperty rdf:resource="https://w3id.org/reno#hasStartTime"/>
                <owl:someValuesFrom rdf:resource="http://www.w3.org/2001/XMLSchema#time"/>
            </owl:Restriction>
        </rdfs:subClassOf>
        <rdfs:subClassOf>
            <owl:Restriction>
                <owl:onProperty rdf:resource="https://w3id.org/reno#hasTemperatureSetPoint"/>
                <owl:someValuesFrom rdf:resource="http://www.w3.org/2001/XMLSchema#decimal"/>
            </owl:Restriction>
        </rdfs:subClassOf>
        <rdfs:comment xml:lang="nl">De verwarmingsperiode van een ruimte is de periode waarin een ruimte verwarmd wordt, op een bepaalde temperatuur. De verwarmingsperiode kan opgevolgd worden door een andere verwarmingsperiode op een andere temperatuur.</rdfs:comment>
        <rdfs:comment xml:lang="en">The heating period of a room is the period during which a room is heated, at a certain temperature. The heating period can be succeeded by another heating period at a different temperature.</rdfs:comment>
        <rdfs:label xml:lang="en">heating period</rdfs:label>
        <rdfs:label xml:lang="nl">verwarmingsperiode</rdfs:label>
    </owl:Class>
    


    <!-- https://w3id.org/reno#InsulationGrade -->


    <owl:Class rdf:about="https://w3id.org/reno#InsulationGrade">
        <rdfs:comment xml:lang="nl">De isolatiegraad van een element bepaalt hoe goed het element geïsoleerd is. De drempelwaarde kan variëren voor elk type bouwelement en kan in de loop van de tijd veranderen.</rdfs:comment>
        <rdfs:comment xml:lang="en">The insulation grade of an element defines how well the element is insulated. The threshold can vary for each type of building element, and can change over time.</rdfs:comment>
        <rdfs:label xml:lang="en">insulation grade</rdfs:label>
        <rdfs:label xml:lang="nl">isolatiegraad</rdfs:label>
    </owl:Class>
    


    <!-- https://w3id.org/reno#ModeratelyInsulated -->


    <owl:Class rdf:about="https://w3id.org/reno#ModeratelyInsulated">
        <rdfs:subClassOf rdf:resource="https://w3id.org/reno#InsulationGrade"/>
        <rdfs:comment xml:lang="nl">Dit geeft aan dat het gebouwelement matig geïsoleerd is.</rdfs:comment>
        <rdfs:comment xml:lang="en">This indicates that the building element is moderately insulated.</rdfs:comment>
        <rdfs:label xml:lang="nl">matig geïsoleerd</rdfs:label>
        <rdfs:label xml:lang="en">moderately insulated</rdfs:label>
    </owl:Class>
    


    <!-- https://w3id.org/reno#Motivation -->


    <owl:Class rdf:about="https://w3id.org/reno#Motivation">
        <rdfs:comment xml:lang="nl">Motivatie is datgene wat een individu tot bepaald gedrag drijft.</rdfs:comment>
        <rdfs:comment xml:lang="en">Motivation is an internal state that propels individuals to engage in goal-directed behavior.</rdfs:comment>
        <rdfs:label xml:lang="nl">motivatie</rdfs:label>
        <rdfs:label xml:lang="en">motivation</rdfs:label>
        <rdfs:seeAlso xml:lang="en">https://en.wikipedia.org/wiki/Motivation</rdfs:seeAlso>
        <rdfs:seeAlso xml:lang="nl">https://nl.wikipedia.org/wiki/Motivatie</rdfs:seeAlso>
    </owl:Class>
    


    <!-- https://w3id.org/reno#MultiPhase -->


    <owl:Class rdf:about="https://w3id.org/reno#MultiPhase">
        <rdfs:subClassOf rdf:resource="https://w3id.org/reno#PowerConnection"/>
        <rdfs:comment xml:lang="en">A multiphase connection is a type of electricity connection. This type may be required in a residential context when using appliances with high power demand.</rdfs:comment>
        <rdfs:comment xml:lang="nl">Een meerfasige aansluiting is een type elektriciteitsaansluiting. Dit type kan vereist zijn in een residentiële context bij het gebruik van apparaten met een hoge stroomvraag.</rdfs:comment>
        <rdfs:label xml:lang="nl">meerfasig</rdfs:label>
        <rdfs:label xml:lang="en">multi-phase</rdfs:label>
    </owl:Class>
    


    <!-- https://w3id.org/reno#North -->


    <owl:Class rdf:about="https://w3id.org/reno#North">
        <rdfs:subClassOf rdf:resource="https://w3id.org/reno#Orientation"/>
        <rdfs:comment xml:lang="nl">Een van de vier kardinale richtingen, meestal aangeduid als N.</rdfs:comment>
        <rdfs:comment xml:lang="en">One of the four cardinal directions, commonly denoted as N.</rdfs:comment>
        <rdfs:label xml:lang="nl">noorden</rdfs:label>
        <rdfs:label xml:lang="en">north</rdfs:label>
    </owl:Class>
    


    <!-- https://w3id.org/reno#NotInsulated -->


    <owl:Class rdf:about="https://w3id.org/reno#NotInsulated">
        <rdfs:subClassOf rdf:resource="https://w3id.org/reno#InsulationGrade"/>
        <rdfs:comment xml:lang="nl">Dit geeft aan dat het gebouwelement niet geïsoleerd is.</rdfs:comment>
        <rdfs:comment xml:lang="en">This indicates that the building element is not insulated.</rdfs:comment>
        <rdfs:label xml:lang="nl">niet geïsoleerd</rdfs:label>
        <rdfs:label xml:lang="en">not insulated</rdfs:label>
    </owl:Class>
    


    <!-- https://w3id.org/reno#Orientation -->


    <owl:Class rdf:about="https://w3id.org/reno#Orientation">
        <rdfs:comment xml:lang="nl">De vier kardinale richtingen, of kardinale punten, zijn de vier belangrijkste kompasrichtingen: noord, zuid, oost en west.</rdfs:comment>
        <rdfs:comment xml:lang="en">The four cardinal directions, or cardinal points, are the four main compass directions: north, south, east, and west.</rdfs:comment>
        <rdfs:label xml:lang="en">orientation</rdfs:label>
        <rdfs:label xml:lang="nl">oriëntatie</rdfs:label>
        <rdfs:seeAlso xml:lang="en">https://en.wikipedia.org/wiki/Cardinal_direction</rdfs:seeAlso>
        <rdfs:seeAlso xml:lang="nl">https://nl.wikipedia.org/wiki/Windstreek</rdfs:seeAlso>
    </owl:Class>
    


    <!-- https://w3id.org/reno#Owner -->


    <owl:Class rdf:about="https://w3id.org/reno#Owner">
        <rdfs:subClassOf rdf:resource="http://xmlns.com/foaf/spec/Person"/>
        <rdfs:subClassOf>
            <owl:Restriction>
                <owl:onProperty rdf:resource="https://w3id.org/reno#isOwnerOf"/>
                <owl:someValuesFrom rdf:resource="https://w3id.org/bot#Building"/>
            </owl:Restriction>
        </rdfs:subClassOf>
        <rdfs:subClassOf>
            <owl:Restriction>
                <owl:onProperty rdf:resource="https://w3id.org/reno#hasDesiredEPCLabel"/>
                <owl:someValuesFrom rdf:resource="http://www.w3.org/2001/XMLSchema#string"/>
            </owl:Restriction>
        </rdfs:subClassOf>
        <rdfs:subClassOf>
            <owl:Restriction>
                <owl:onProperty rdf:resource="https://w3id.org/reno#hasNuisanceScore"/>
                <owl:someValuesFrom rdf:resource="http://www.w3.org/2001/XMLSchema#integer"/>
            </owl:Restriction>
        </rdfs:subClassOf>
        <rdfs:subClassOf>
            <owl:Restriction>
                <owl:onProperty rdf:resource="https://w3id.org/reno#hasRenovationBudget"/>
                <owl:someValuesFrom rdf:resource="http://www.w3.org/2001/XMLSchema#decimal"/>
            </owl:Restriction>
        </rdfs:subClassOf>
        <rdfs:subClassOf>
            <owl:Restriction>
                <owl:onProperty rdf:resource="https://w3id.org/reno#inFavourOfPVInGarden"/>
                <owl:someValuesFrom rdf:resource="http://www.w3.org/2001/XMLSchema#boolean"/>
            </owl:Restriction>
        </rdfs:subClassOf>
        <rdfs:subClassOf>
            <owl:Restriction>
                <owl:onProperty rdf:resource="https://w3id.org/reno#ownerSince"/>
                <owl:someValuesFrom rdf:resource="http://www.w3.org/2001/XMLSchema#gYear"/>
            </owl:Restriction>
        </rdfs:subClassOf>
        <rdfs:subClassOf>
            <owl:Restriction>
                <owl:onProperty rdf:resource="https://w3id.org/reno#ownerUntil"/>
                <owl:someValuesFrom rdf:resource="http://www.w3.org/2001/XMLSchema#gYear"/>
            </owl:Restriction>
        </rdfs:subClassOf>
        <rdfs:subClassOf>
            <owl:Restriction>
                <owl:onProperty rdf:resource="https://w3id.org/reno#satisfiedWithRevenuePV"/>
                <owl:someValuesFrom rdf:resource="http://www.w3.org/2001/XMLSchema#boolean"/>
            </owl:Restriction>
        </rdfs:subClassOf>
        <rdfs:comment xml:lang="en">An owner is someone who obtained ownership over a property, in this context a building.</rdfs:comment>
        <rdfs:comment xml:lang="nl">Een eigenaar is iemand die een eigendom heeft verkregen, in deze context van een gebouw.</rdfs:comment>
        <rdfs:label xml:lang="nl">eigenaar</rdfs:label>
        <rdfs:label xml:lang="en">owner</rdfs:label>
        <rdfs:seeAlso xml:lang="en">https://en.wikipedia.org/wiki/Ownership</rdfs:seeAlso>
        <rdfs:seeAlso xml:lang="nl">https://nl.wikipedia.org/wiki/Eigendom</rdfs:seeAlso>
    </owl:Class>
    


    <!-- https://w3id.org/reno#PVC -->


    <owl:Class rdf:about="https://w3id.org/reno#PVC">
        <rdfs:subClassOf rdf:resource="https://w3id.org/reno#WindowFrameMaterial"/>
        <rdfs:comment xml:lang="en">Polyvinyl chloride (PVC) is the world&apos;s third-most widely produced synthetic polymer of plastic.</rdfs:comment>
        <rdfs:comment xml:lang="nl">Polyvinylchloride (PVC) is wereldwijd het op twee na meest geproduceerde synthetische polymeer van kunststof.</rdfs:comment>
        <rdfs:label xml:lang="en">PVC</rdfs:label>
        <rdfs:label xml:lang="nl">PVC</rdfs:label>
        <rdfs:seeAlso xml:lang="en">https://en.wikipedia.org/wiki/Polyvinyl_chloride</rdfs:seeAlso>
        <rdfs:seeAlso xml:lang="nl">https://nl.wikipedia.org/wiki/Polyvinylchloride</rdfs:seeAlso>
    </owl:Class>
    


    <!-- https://w3id.org/reno#PowerConnection -->


    <owl:Class rdf:about="https://w3id.org/reno#PowerConnection">
        <rdfs:comment xml:lang="en">A power connection connects the power grid to a meter box, providing power in the home.</rdfs:comment>
        <rdfs:comment xml:lang="nl">Een elektriciteitsaansluiting verbindt het energienet met een meterkast, waardoor er stroom is in de woning.</rdfs:comment>
        <rdfs:label xml:lang="nl">elektriciteitsaansluiting</rdfs:label>
        <rdfs:label xml:lang="en">power connection</rdfs:label>
    </owl:Class>
    


    <!-- https://w3id.org/reno#PriorState -->


    <owl:Class rdf:about="https://w3id.org/reno#PriorState">
        <owl:equivalentClass>
            <owl:Class>
                <owl:unionOf rdf:parseType="Collection">
                    <owl:Class>
                        <owl:intersectionOf rdf:parseType="Collection">
                            <rdf:Description rdf:about="http://bimerr.iot.linkeddata.es/def/material-properties#MaterialLayerSet"/>
                            <owl:Restriction>
                                <owl:onProperty rdf:resource="https://w3id.org/reno#changedInto"/>
                                <owl:someValuesFrom rdf:resource="http://bimerr.iot.linkeddata.es/def/material-properties#MaterialLayerSet"/>
                            </owl:Restriction>
                        </owl:intersectionOf>
                    </owl:Class>
                    <owl:Class>
                        <owl:intersectionOf rdf:parseType="Collection">
                            <rdf:Description rdf:about="https://w3id.org/reno#WindowFrame"/>
                            <owl:Restriction>
                                <owl:onProperty rdf:resource="https://w3id.org/reno#changedInto"/>
                                <owl:someValuesFrom rdf:resource="https://w3id.org/reno#WindowFrame"/>
                            </owl:Restriction>
                        </owl:intersectionOf>
                    </owl:Class>
                    <owl:Class>
                        <owl:intersectionOf rdf:parseType="Collection">
                            <rdf:Description rdf:about="https://w3id.org/reno#WindowGlazing"/>
                            <owl:Restriction>
                                <owl:onProperty rdf:resource="https://w3id.org/reno#changedInto"/>
                                <owl:someValuesFrom rdf:resource="https://w3id.org/reno#WindowGlazing"/>
                            </owl:Restriction>
                        </owl:intersectionOf>
                    </owl:Class>
                </owl:unionOf>
            </owl:Class>
        </owl:equivalentClass>
        <rdfs:comment xml:lang="nl">De eerdere toestand duidt alle toestanden dat een gebouwelement had voor een renovatie aan.</rdfs:comment>
        <rdfs:comment xml:lang="en">The prior state denotes all states that a building element had before a renovation.</rdfs:comment>
        <rdfs:label xml:lang="nl">eerdere toestand</rdfs:label>
        <rdfs:label xml:lang="en">prior state</rdfs:label>
    </owl:Class>
    


    <!-- https://w3id.org/reno#Radiator -->


    <owl:Class rdf:about="https://w3id.org/reno#Radiator">
        <rdfs:subClassOf rdf:resource="https://saref.etsi.org/saref4bldg/SpaceHeater"/>
        <rdfs:comment xml:lang="en">A radiator is a heat exchange device that transfers heat from hot water to the surrounding air through both convection and radiation.</rdfs:comment>
        <rdfs:comment xml:lang="nl">Een radiator is een warmtewisselaar die warmte van warm water overdraagt aan de omringende lucht door zowel convectie als straling.</rdfs:comment>
        <rdfs:label xml:lang="en">radiator</rdfs:label>
        <rdfs:label xml:lang="nl">radiator</rdfs:label>
        <rdfs:seeAlso xml:lang="en">https://en.wikipedia.org/wiki/Radiator</rdfs:seeAlso>
        <rdfs:seeAlso xml:lang="nl">https://nl.wikipedia.org/wiki/Radiateur</rdfs:seeAlso>
    </owl:Class>
    


    <!-- https://w3id.org/reno#RenovatedElement -->


    <owl:Class rdf:about="https://w3id.org/reno#RenovatedElement">
        <owl:equivalentClass>
            <owl:Class>
                <owl:intersectionOf rdf:parseType="Collection">
                    <rdf:Description rdf:about="https://pi.pauwel.be/voc/buildingelement#BuildingElement"/>
                    <owl:Class>
                        <owl:unionOf rdf:parseType="Collection">
                            <owl:Restriction>
                                <owl:onProperty rdf:resource="http://bimerr.iot.linkeddata.es/def/material-properties#hasMaterialLayerSet"/>
                                <owl:minQualifiedCardinality rdf:datatype="http://www.w3.org/2001/XMLSchema#nonNegativeInteger">2</owl:minQualifiedCardinality>
                                <owl:onClass rdf:resource="http://bimerr.iot.linkeddata.es/def/material-properties#MaterialLayerSet"/>
                            </owl:Restriction>
                            <owl:Restriction>
                                <owl:onProperty rdf:resource="https://w3id.org/reno#hasFrame"/>
                                <owl:minQualifiedCardinality rdf:datatype="http://www.w3.org/2001/XMLSchema#nonNegativeInteger">2</owl:minQualifiedCardinality>
                                <owl:onClass rdf:resource="https://w3id.org/reno#WindowFrame"/>
                            </owl:Restriction>
                            <owl:Restriction>
                                <owl:onProperty rdf:resource="https://w3id.org/reno#hasGlazing"/>
                                <owl:minQualifiedCardinality rdf:datatype="http://www.w3.org/2001/XMLSchema#nonNegativeInteger">2</owl:minQualifiedCardinality>
                                <owl:onClass rdf:resource="https://w3id.org/reno#WindowGlazing"/>
                            </owl:Restriction>
                        </owl:unionOf>
                    </owl:Class>
                </owl:intersectionOf>
            </owl:Class>
        </owl:equivalentClass>
        <rdfs:comment xml:lang="en">A renovated element is a building element which has undergone modifications during a renovation (intervention).</rdfs:comment>
        <rdfs:comment xml:lang="nl">Een gerenoveerd element is een gebouwelement dat wijzigingen heeft ondergaan tijdens een renovatie (interventie).</rdfs:comment>
        <rdfs:label xml:lang="nl">gerenoveerd element</rdfs:label>
        <rdfs:label xml:lang="en">renovated element</rdfs:label>
    </owl:Class>
    


    <!-- https://w3id.org/reno#Renovation -->


    <owl:Class rdf:about="https://w3id.org/reno#Renovation">
        <rdfs:subClassOf>
            <owl:Restriction>
                <owl:onProperty rdf:resource="https://w3id.org/reno#hasRenovationIntervention"/>
                <owl:someValuesFrom rdf:resource="https://w3id.org/reno#RenovationIntervention"/>
            </owl:Restriction>
        </rdfs:subClassOf>
        <rdfs:subClassOf>
            <owl:Restriction>
                <owl:onProperty rdf:resource="https://w3id.org/reno#hasEndDate"/>
                <owl:someValuesFrom rdf:resource="http://www.w3.org/2001/XMLSchema#date"/>
            </owl:Restriction>
        </rdfs:subClassOf>
        <rdfs:subClassOf>
            <owl:Restriction>
                <owl:onProperty rdf:resource="https://w3id.org/reno#hasRenovationCost"/>
                <owl:someValuesFrom rdf:resource="http://www.w3.org/2001/XMLSchema#decimal"/>
            </owl:Restriction>
        </rdfs:subClassOf>
        <rdfs:subClassOf>
            <owl:Restriction>
                <owl:onProperty rdf:resource="https://w3id.org/reno#hasStartDate"/>
                <owl:someValuesFrom rdf:resource="http://www.w3.org/2001/XMLSchema#date"/>
            </owl:Restriction>
        </rdfs:subClassOf>
        <rdfs:comment xml:lang="en">A renovation indicates the process of improving broken, damaged, or outdated structures. A renovation often consists of multiple renovation interventions.</rdfs:comment>
        <rdfs:comment xml:lang="nl">Een renovatie duidt het proces van het verbeteren van kapotte, beschadigde of verouderde structuren aan. Een renovatie bestaat vaak uit meerdere renovatie interventies.</rdfs:comment>
        <rdfs:label xml:lang="nl">renovatie</rdfs:label>
        <rdfs:label xml:lang="en">renovation</rdfs:label>
        <rdfs:seeAlso xml:lang="en">https://en.wikipedia.org/wiki/Renovation</rdfs:seeAlso>
        <rdfs:seeAlso xml:lang="nl">https://nl.wikipedia.org/wiki/Renovatie</rdfs:seeAlso>
    </owl:Class>
    


    <!-- https://w3id.org/reno#RenovationIntervention -->


    <owl:Class rdf:about="https://w3id.org/reno#RenovationIntervention">
        <rdfs:subClassOf>
            <owl:Restriction>
                <owl:onProperty rdf:resource="https://w3id.org/reno#isRenovationInterventionOf"/>
                <owl:someValuesFrom rdf:resource="https://w3id.org/reno#Renovation"/>
            </owl:Restriction>
        </rdfs:subClassOf>
        <rdfs:comment xml:lang="en">A renovation consists often of multiple renovation interventions. The division of interventions is considered per building element.</rdfs:comment>
        <rdfs:comment xml:lang="nl">Een renovatie bestaat vaak uit meerdere renovatie interventies. De opsplitsting van interventies wordt gezien per bouwelement.</rdfs:comment>
        <rdfs:label xml:lang="nl">renovatie interventie</rdfs:label>
        <rdfs:label xml:lang="en">renovation intervention</rdfs:label>
    </owl:Class>
    


    <!-- https://w3id.org/reno#RenovationMotivation -->


    <owl:Class rdf:about="https://w3id.org/reno#RenovationMotivation">
        <rdfs:subClassOf rdf:resource="https://w3id.org/reno#Motivation"/>
        <rdfs:comment xml:lang="nl">De renovatie motivatie van een persoon is de motivatie waarom een persoon wil renoveren.</rdfs:comment>
        <rdfs:comment xml:lang="en">The renovation motivation of a person is the motivation why a person wants to renovate.</rdfs:comment>
        <rdfs:label xml:lang="nl">renovatie motivatie</rdfs:label>
        <rdfs:label xml:lang="en">renovation motivation</rdfs:label>
    </owl:Class>
    


    <!-- https://w3id.org/reno#Resident -->


    <owl:Class rdf:about="https://w3id.org/reno#Resident">
        <rdfs:subClassOf rdf:resource="http://xmlns.com/foaf/spec/Person"/>
        <rdfs:subClassOf>
            <owl:Restriction>
                <owl:onProperty rdf:resource="https://w3id.org/reno#hasAddress"/>
                <owl:someValuesFrom rdf:resource="https://w3id.org/reno#Address"/>
            </owl:Restriction>
        </rdfs:subClassOf>
        <rdfs:subClassOf>
            <owl:Restriction>
                <owl:onProperty rdf:resource="https://w3id.org/reno#isResidentOf"/>
                <owl:someValuesFrom rdf:resource="https://w3id.org/bot#Building"/>
            </owl:Restriction>
        </rdfs:subClassOf>
        <rdfs:subClassOf>
            <owl:Restriction>
                <owl:onProperty rdf:resource="https://w3id.org/reno#residentSince"/>
                <owl:someValuesFrom rdf:resource="http://www.w3.org/2001/XMLSchema#gYear"/>
            </owl:Restriction>
        </rdfs:subClassOf>
        <rdfs:subClassOf>
            <owl:Restriction>
                <owl:onProperty rdf:resource="https://w3id.org/reno#residentUntil"/>
                <owl:someValuesFrom rdf:resource="http://www.w3.org/2001/XMLSchema#gYear"/>
            </owl:Restriction>
        </rdfs:subClassOf>
        <rdfs:comment xml:lang="nl">A resident is someone who lives in a building. A person&apos;s domicile is often look at to determine which building is resided bu them.</rdfs:comment>
        <rdfs:comment xml:lang="nl">Een bewoner is iemand die in een gebouw woont. Vaak wordt er gekeken naar de domicilie van een persoon, om te bepalen welk gebouw door hen wordt bewoond.</rdfs:comment>
        <rdfs:label xml:lang="nl">bewoner</rdfs:label>
        <rdfs:label xml:lang="en">resident</rdfs:label>
        <rdfs:seeAlso xml:lang="en">https://en.wikipedia.org/wiki/Domicile_(law)</rdfs:seeAlso>
        <rdfs:seeAlso xml:lang="nl">https://nl.wikipedia.org/wiki/Domicilie</rdfs:seeAlso>
    </owl:Class>
    


    <!-- https://w3id.org/reno#SemiDetachedBuilding -->


    <owl:Class rdf:about="https://w3id.org/reno#SemiDetachedBuilding">
        <rdfs:subClassOf rdf:resource="https://w3id.org/bot#Building"/>
        <rdfs:comment xml:lang="en">A semi-detached building is a building that shares a wall with another house on one side.</rdfs:comment>
        <rdfs:comment xml:lang="nl">Een halfopen bebouwing is een gebouw dat aan een zijde een muur deelt met een andere woning.</rdfs:comment>
        <rdfs:label xml:lang="nl">halfopen bebouwing</rdfs:label>
        <rdfs:label xml:lang="en">semi-detached building</rdfs:label>
        <rdfs:seeAlso xml:lang="en">https://en.wikipedia.org/wiki/Semi-detached</rdfs:seeAlso>
        <rdfs:seeAlso xml:lang="nl">https://nl.wikipedia.org/wiki/Twee-onder-een-kapwoning</rdfs:seeAlso>
    </owl:Class>
    


    <!-- https://w3id.org/reno#SingleGlazing -->


    <owl:Class rdf:about="https://w3id.org/reno#SingleGlazing">
        <rdfs:subClassOf rdf:resource="https://w3id.org/reno#WindowGlazingType"/>
        <rdfs:comment xml:lang="nl">Enkele beglazing bestaat uit slechts één glazen paneel. Dit type beglazing heeft slechte thermische en akoestische eigenschappen.</rdfs:comment>
        <rdfs:comment xml:lang="en">Single-glazing consists of only one glass panel. This type of glazing has poor thermal and acoustic properties.</rdfs:comment>
        <rdfs:label xml:lang="nl">enkel glas</rdfs:label>
        <rdfs:label xml:lang="en">single glazing</rdfs:label>
    </owl:Class>
    


    <!-- https://w3id.org/reno#SinglePhase -->


    <owl:Class rdf:about="https://w3id.org/reno#SinglePhase">
        <rdfs:subClassOf rdf:resource="https://w3id.org/reno#PowerConnection"/>
        <rdfs:comment xml:lang="en">A single-phase connection is a type of electricity connection. This provides enough electricity for domestic use.</rdfs:comment>
        <rdfs:comment xml:lang="nl">Een monofasige aansluiting is een type elektriciteitsaansluiting. Dit biedt genoeg elektriciteit voor huishoudelijk gebruik.</rdfs:comment>
        <rdfs:label xml:lang="nl">monofasig</rdfs:label>
        <rdfs:label xml:lang="en">single-phase</rdfs:label>
    </owl:Class>
    


    <!-- https://w3id.org/reno#SolarBoiler -->


    <owl:Class rdf:about="https://w3id.org/reno#SolarBoiler">
        <rdfs:subClassOf rdf:resource="https://saref.etsi.org/saref4bldg/Boiler"/>
        <rdfs:comment xml:lang="en">A solar water heater heats up water with energy obtained from the sun.</rdfs:comment>
        <rdfs:comment xml:lang="nl">Een zonneboiler verwarmt water met energie van de zon.</rdfs:comment>
        <rdfs:label xml:lang="en">solar boiler</rdfs:label>
        <rdfs:label xml:lang="nl">zonneboiler</rdfs:label>
    </owl:Class>
    


    <!-- https://w3id.org/reno#SoundLevel -->


    <owl:Class rdf:about="https://w3id.org/reno#SoundLevel">
        <rdfs:comment xml:lang="nl">Het geluidsniveau van een ruimte geeft weer welk geluid toegestaan is of voorkomt in deze ruimte. Vaak hangt dit samen met de functie van de ruimte.</rdfs:comment>
        <rdfs:comment xml:lang="en">The sound level of a room reflects what sound is allowed or occurs in this room. This is often related to the function of the room.</rdfs:comment>
        <rdfs:label xml:lang="nl">geluidsniveau</rdfs:label>
        <rdfs:label xml:lang="en">sound level</rdfs:label>
    </owl:Class>
    


    <!-- https://w3id.org/reno#South -->


    <owl:Class rdf:about="https://w3id.org/reno#South">
        <rdfs:subClassOf rdf:resource="https://w3id.org/reno#Orientation"/>
        <rdfs:comment xml:lang="nl">Een van de vier kardinale richtingen, meestal aangeduid als Z.</rdfs:comment>
        <rdfs:comment xml:lang="en">One of the four cardinal directions, commonly denoted as S.</rdfs:comment>
        <rdfs:label xml:lang="en">south</rdfs:label>
        <rdfs:label xml:lang="nl">zuiden</rdfs:label>
    </owl:Class>
    


    <!-- https://w3id.org/reno#SpaceUsage -->


    <owl:Class rdf:about="https://w3id.org/reno#SpaceUsage">
        <rdfs:comment xml:lang="nl">Het ruimtegebruik geeft aan waarvoor een bepaalde ruimte wordt gebruikt.</rdfs:comment>
        <rdfs:comment xml:lang="en">The space usage indicates for what purpose a certain room is used.</rdfs:comment>
        <rdfs:label xml:lang="nl">ruimtegebruik</rdfs:label>
        <rdfs:label xml:lang="en">space usage</rdfs:label>
    </owl:Class>
    


    <!-- https://w3id.org/reno#State -->


    <owl:Class rdf:about="https://w3id.org/reno#State">
        <rdfs:subClassOf>
            <owl:Restriction>
                <owl:onProperty rdf:resource="https://w3id.org/reno#hasStateDate"/>
                <owl:someValuesFrom rdf:resource="http://www.w3.org/2001/XMLSchema#date"/>
            </owl:Restriction>
        </rdfs:subClassOf>
        <rdfs:subClassOf>
            <owl:Restriction>
                <owl:onProperty rdf:resource="https://w3id.org/reno#hasStateValue"/>
                <owl:someValuesFrom rdf:resource="http://www.w3.org/2001/XMLSchema#integer"/>
            </owl:Restriction>
        </rdfs:subClassOf>
        <rdfs:comment xml:lang="nl">De staat van iets geeft de toestand aan met betrekking tot het uiterlijk, de kwaliteit of de efficiëntie ervan.</rdfs:comment>
        <rdfs:comment xml:lang="en">The state of something indicates the state with regard to its appearance, quality or efficiency.</rdfs:comment>
        <rdfs:label xml:lang="nl">staat</rdfs:label>
        <rdfs:label xml:lang="en">state</rdfs:label>
    </owl:Class>
    


    <!-- https://w3id.org/reno#Steel -->


    <owl:Class rdf:about="https://w3id.org/reno#Steel">
        <rdfs:subClassOf rdf:resource="https://w3id.org/reno#WindowFrameMaterial"/>
        <rdfs:comment xml:lang="nl">Staal is een legering van ijzer en koolstof met een verbeterde sterkte en breukvastheid in vergelijking met andere vormen van ijzer. Vanwege de hoge treksterkte en lage kosten is staal een van de meest geproduceerde materialen ter wereld.</rdfs:comment>
        <rdfs:comment xml:lang="en">Steel is an alloy of iron and carbon with improved strength and fracture resistance compared to other forms of iron. Because of its high tensile strength and low cost, steel is one of the most commonly manufactured materials in the world.</rdfs:comment>
        <rdfs:label xml:lang="nl">staal</rdfs:label>
        <rdfs:label xml:lang="en">steel</rdfs:label>
        <rdfs:seeAlso xml:lang="en">https://en.wikipedia.org/wiki/Steel</rdfs:seeAlso>
        <rdfs:seeAlso xml:lang="nl">https://nl.wikipedia.org/wiki/Staal_(legering)</rdfs:seeAlso>
    </owl:Class>
    


    <!-- https://w3id.org/reno#Stove -->


    <owl:Class rdf:about="https://w3id.org/reno#Stove">
        <rdfs:subClassOf rdf:resource="https://saref.etsi.org/saref4bldg/SpaceHeater"/>
        <rdfs:comment xml:lang="en">A stove is a heating device in which heat is generated by burning fuel.</rdfs:comment>
        <rdfs:comment xml:lang="nl">Een kachel is een verwarmingsapparaat waarin er warmte door middel van verbranding van brandstof wordt opgewekt.</rdfs:comment>
        <rdfs:label xml:lang="nl">kachel</rdfs:label>
        <rdfs:label xml:lang="en">stove</rdfs:label>
        <rdfs:seeAlso xml:lang="en">https://en.wikipedia.org/wiki/Stove</rdfs:seeAlso>
        <rdfs:seeAlso xml:lang="nl">https://nl.wikipedia.org/wiki/Kachel</rdfs:seeAlso>
    </owl:Class>
    


    <!-- https://w3id.org/reno#Tender -->


    <owl:Class rdf:about="https://w3id.org/reno#Tender">
        <rdfs:subClassOf>
            <owl:Restriction>
                <owl:onProperty rdf:resource="https://w3id.org/reno#hasAffectedElement"/>
                <owl:someValuesFrom rdf:resource="https://w3id.org/bot#Element"/>
            </owl:Restriction>
        </rdfs:subClassOf>
        <rdfs:subClassOf>
            <owl:Restriction>
                <owl:onProperty rdf:resource="https://w3id.org/reno#isSignedBy"/>
                <owl:someValuesFrom rdf:resource="http://xmlns.com/foaf/spec/Person"/>
            </owl:Restriction>
        </rdfs:subClassOf>
        <rdfs:subClassOf>
            <owl:Restriction>
                <owl:onProperty rdf:resource="https://w3id.org/reno#hasSignatureDate"/>
                <owl:someValuesFrom rdf:resource="http://www.w3.org/2001/XMLSchema#date"/>
            </owl:Restriction>
        </rdfs:subClassOf>
        <rdfs:comment xml:lang="en">A tender is a formal offer to conclude a contract, made at the request of a company&apos;s potential customer.</rdfs:comment>
        <rdfs:comment xml:lang="nl">Een offerte is een formeel aanbod tot het sluiten van een overeenkomst, opgesteld op verzoek van een potentiële klant van een bedrijf.</rdfs:comment>
        <rdfs:label xml:lang="nl">offerte</rdfs:label>
        <rdfs:label xml:lang="en">tender</rdfs:label>
        <rdfs:seeAlso xml:lang="en">https://en.wikipedia.org/wiki/Bidding</rdfs:seeAlso>
        <rdfs:seeAlso xml:lang="nl">https://nl.wikipedia.org/wiki/Offerte</rdfs:seeAlso>
    </owl:Class>
    


    <!-- https://w3id.org/reno#TripleGlazing -->


    <owl:Class rdf:about="https://w3id.org/reno#TripleGlazing">
        <rdfs:subClassOf rdf:resource="https://w3id.org/reno#WindowGlazingType"/>
        <rdfs:comment xml:lang="nl">Driedubbel glas bestaat uit drie glazen ruiten die van elkaar gescheiden zijn door spaties. Het heeft een betere isolatiewaarde dan dubbele beglazing.</rdfs:comment>
        <rdfs:comment xml:lang="en">Triple glazing consists of three glass window panes seperated by spaces. It has a better insulating value than double glazing.</rdfs:comment>
        <rdfs:label xml:lang="nl">driedubbel glas</rdfs:label>
        <rdfs:label xml:lang="en">triple glazing</rdfs:label>
        <rdfs:seeAlso xml:lang="en">https://en.wikipedia.org/wiki/Insulated_glazing</rdfs:seeAlso>
    </owl:Class>
    


    <!-- https://w3id.org/reno#VentilationSystem -->


    <owl:Class rdf:about="https://w3id.org/reno#VentilationSystem">
        <rdfs:subClassOf rdf:resource="https://saref.etsi.org/saref4bldg/FlowMovingDevice"/>
        <rdfs:comment xml:lang="nl">Ventilatiesystemen worden gebruikt om buitenlucht in de geklimatiseerde ruimte te brengen om de kwaliteit van de binnenlucht te regelen en het thermisch comfort te behouden.</rdfs:comment>
        <rdfs:comment xml:lang="en">Ventilation systems are used to introduce outdoor air into the air-conditioned space for the purposes of controlling the quality of indoor air and maintaining thermal comfort.</rdfs:comment>
        <rdfs:label xml:lang="nl">ventilatiesysteem</rdfs:label>
        <rdfs:label xml:lang="en">ventilation system</rdfs:label>
    </owl:Class>
    


    <!-- https://w3id.org/reno#VentilationSystemA -->


    <owl:Class rdf:about="https://w3id.org/reno#VentilationSystemA">
        <rdfs:subClassOf rdf:resource="https://w3id.org/reno#VentilationSystem"/>
        <rdfs:comment xml:lang="nl">Het ventilatiesysteem A werkt op basis van een natuurlijke luchttoevoer en luchtafvoer.</rdfs:comment>
        <rdfs:comment xml:lang="en">Ventilation system A works on the basis of natural air supply and air exhaust.</rdfs:comment>
        <rdfs:label xml:lang="nl">ventilatiesysteem A</rdfs:label>
        <rdfs:label xml:lang="en">ventilation system A</rdfs:label>
        <rdfs:seeAlso xml:lang="nl">https://www.vlaanderen.be/bouwen-wonen-en-energie/veilig-gezond-en-kwaliteitsvol-wonen/verluchting-en-ventilatie/ventilatiesystemen</rdfs:seeAlso>
    </owl:Class>
    


    <!-- https://w3id.org/reno#VentilationSystemB -->


    <owl:Class rdf:about="https://w3id.org/reno#VentilationSystemB">
        <rdfs:subClassOf rdf:resource="https://w3id.org/reno#VentilationSystem"/>
        <rdfs:comment xml:lang="nl">Het ventilatiesysteem A werkt op basis van een mechanische luchttoevoer en een natuurlijke luchtafvoer.</rdfs:comment>
        <rdfs:comment xml:lang="en">Ventilation system A works on the basis of mechanical air supply and natural air exhaust.</rdfs:comment>
        <rdfs:label xml:lang="nl">ventilatiesysteem B</rdfs:label>
        <rdfs:label xml:lang="en">ventilation system B</rdfs:label>
        <rdfs:seeAlso xml:lang="nl">https://www.vlaanderen.be/bouwen-wonen-en-energie/veilig-gezond-en-kwaliteitsvol-wonen/verluchting-en-ventilatie/ventilatiesystemen</rdfs:seeAlso>
    </owl:Class>
    


    <!-- https://w3id.org/reno#VentilationSystemC -->


    <owl:Class rdf:about="https://w3id.org/reno#VentilationSystemC">
        <rdfs:subClassOf rdf:resource="https://w3id.org/reno#VentilationSystem"/>
        <rdfs:comment xml:lang="nl">Het ventilatiesysteem A werkt op basis van een natuurlijke luchttoevoer en een mechanische luchtafvoer.</rdfs:comment>
        <rdfs:comment xml:lang="en">Ventilation system A works on the basis of natural air supply and mechanical air exhaust.</rdfs:comment>
        <rdfs:label xml:lang="nl">ventilatiesysteem C</rdfs:label>
        <rdfs:label xml:lang="en">ventilation system C</rdfs:label>
        <rdfs:seeAlso xml:lang="nl">https://www.vlaanderen.be/bouwen-wonen-en-energie/veilig-gezond-en-kwaliteitsvol-wonen/verluchting-en-ventilatie/ventilatiesystemen</rdfs:seeAlso>
    </owl:Class>
    


    <!-- https://w3id.org/reno#VentilationSystemD -->


    <owl:Class rdf:about="https://w3id.org/reno#VentilationSystemD">
        <rdfs:subClassOf rdf:resource="https://w3id.org/reno#VentilationSystem"/>
        <rdfs:comment xml:lang="nl">Het ventilatiesysteem A werkt op basis van een natuurlijke luchttoevoer en luchtafvoer.</rdfs:comment>
        <rdfs:comment xml:lang="en">Ventilation system A works on the basis of mechanical air supply and air exhaust.</rdfs:comment>
        <rdfs:label xml:lang="nl">ventilatiesysteem D</rdfs:label>
        <rdfs:label xml:lang="en">ventilation system D</rdfs:label>
        <rdfs:seeAlso xml:lang="nl">https://www.vlaanderen.be/bouwen-wonen-en-energie/veilig-gezond-en-kwaliteitsvol-wonen/verluchting-en-ventilatie/ventilatiesystemen</rdfs:seeAlso>
    </owl:Class>
    


    <!-- https://w3id.org/reno#Water -->


    <owl:Class rdf:about="https://w3id.org/reno#Water">
        <rdfs:subClassOf rdf:resource="https://saref.etsi.org/core/NaturalResourceCommodity"/>
        <rdfs:comment xml:lang="en">Water is an inorganic compound. It is a transparent, tasteless, odorless, and nearly colorless chemical substance.</rdfs:comment>
        <rdfs:comment xml:lang="nl">Water is een anorganische verbinding. Het is een transparante, smaakloze, geurloze en bijna kleurloze chemische stof.</rdfs:comment>
        <rdfs:label xml:lang="en">water</rdfs:label>
        <rdfs:label xml:lang="nl">water</rdfs:label>
        <rdfs:seeAlso xml:lang="en">https://en.wikipedia.org/wiki/Water</rdfs:seeAlso>
        <rdfs:seeAlso xml:lang="nl">https://nl.wikipedia.org/wiki/Water</rdfs:seeAlso>
    </owl:Class>
    


    <!-- https://w3id.org/reno#WellInsulated -->


    <owl:Class rdf:about="https://w3id.org/reno#WellInsulated">
        <rdfs:subClassOf rdf:resource="https://w3id.org/reno#InsulationGrade"/>
        <rdfs:comment xml:lang="nl">Dit geeft aan dat het gebouwelement goed geïsoleerd is.</rdfs:comment>
        <rdfs:comment xml:lang="en">This indicates that the building element is well insulated.</rdfs:comment>
        <rdfs:label xml:lang="nl">goed geïsoleerd</rdfs:label>
        <rdfs:label xml:lang="en">well insulated</rdfs:label>
    </owl:Class>
    


    <!-- https://w3id.org/reno#West -->


    <owl:Class rdf:about="https://w3id.org/reno#West">
        <rdfs:subClassOf rdf:resource="https://w3id.org/reno#Orientation"/>
        <rdfs:comment xml:lang="nl">Een van de vier kardinale richtingen, meestal aangeduid als W.</rdfs:comment>
        <rdfs:comment xml:lang="en">One of the four cardinal directions, commonly denoted as W.</rdfs:comment>
        <rdfs:label xml:lang="en">west</rdfs:label>
        <rdfs:label xml:lang="nl">westen</rdfs:label>
    </owl:Class>
    


    <!-- https://w3id.org/reno#WindowFrame -->


    <owl:Class rdf:about="https://w3id.org/reno#WindowFrame">
        <rdfs:subClassOf>
            <owl:Restriction>
                <owl:onProperty rdf:resource="https://w3id.org/reno#hasFrameMaterial"/>
                <owl:someValuesFrom rdf:resource="https://w3id.org/reno#WindowFrameMaterial"/>
            </owl:Restriction>
        </rdfs:subClassOf>
        <rdfs:subClassOf>
            <owl:Restriction>
                <owl:onProperty rdf:resource="https://w3id.org/reno#isFrameOf"/>
                <owl:someValuesFrom rdf:resource="https://pi.pauwel.be/voc/buildingelement#Window"/>
            </owl:Restriction>
        </rdfs:subClassOf>
        <rdfs:subClassOf>
            <owl:Restriction>
                <owl:onProperty rdf:resource="https://w3id.org/reno#hasFrameThickness"/>
                <owl:someValuesFrom rdf:resource="http://www.w3.org/2001/XMLSchema#decimal"/>
            </owl:Restriction>
        </rdfs:subClassOf>
        <rdfs:subClassOf>
            <owl:Restriction>
                <owl:onProperty rdf:resource="https://w3id.org/reno#hasThermalBreak"/>
                <owl:someValuesFrom rdf:resource="http://www.w3.org/2001/XMLSchema#boolean"/>
            </owl:Restriction>
        </rdfs:subClassOf>
        <rdfs:comment xml:lang="en">A window frame is a rectangular frame, edging or framework in which windows or movable sash sheets are placed. It is a component of a window.</rdfs:comment>
        <rdfs:comment xml:lang="nl">Een raamkader is een rechthoekig frame, randwerk of raamwerk waarin ruiten of beweegbare raambladen worden geplaatst. Het is een onderdeel van een raam.</rdfs:comment>
        <rdfs:label xml:lang="nl">raamkader</rdfs:label>
        <rdfs:label xml:lang="en">window frame</rdfs:label>
        <rdfs:seeAlso xml:lang="nl">https://nl.wikipedia.org/wiki/Raamkozijn</rdfs:seeAlso>
    </owl:Class>
    


    <!-- https://w3id.org/reno#WindowFrameMaterial -->


    <owl:Class rdf:about="https://w3id.org/reno#WindowFrameMaterial">
        <rdfs:comment xml:lang="nl">Het materiaal waaruit het raamkader vervaardigd is.</rdfs:comment>
        <rdfs:comment xml:lang="en">The material from which the window frame is made.</rdfs:comment>
        <rdfs:label xml:lang="nl">raamkader materiaal</rdfs:label>
        <rdfs:label xml:lang="en">window frame material</rdfs:label>
    </owl:Class>
    


    <!-- https://w3id.org/reno#WindowGlazing -->


    <owl:Class rdf:about="https://w3id.org/reno#WindowGlazing">
        <rdfs:subClassOf>
            <owl:Restriction>
                <owl:onProperty rdf:resource="https://w3id.org/reno#hasGlazingType"/>
                <owl:someValuesFrom rdf:resource="https://w3id.org/reno#WindowGlazingType"/>
            </owl:Restriction>
        </rdfs:subClassOf>
        <rdfs:subClassOf>
            <owl:Restriction>
                <owl:onProperty rdf:resource="https://w3id.org/reno#isGlazingOf"/>
                <owl:someValuesFrom rdf:resource="https://pi.pauwel.be/voc/buildingelement#Window"/>
            </owl:Restriction>
        </rdfs:subClassOf>
        <rdfs:comment xml:lang="nl">De beglazing is het (vaak transparante) deel van een raam dat vervat zit in het raamkader.</rdfs:comment>
        <rdfs:comment xml:lang="en">The glazing is the (often transparent) part of a window contained within the window frame.</rdfs:comment>
        <rdfs:label xml:lang="nl">raam beglazing</rdfs:label>
        <rdfs:label xml:lang="en">window glazing</rdfs:label>
    </owl:Class>
    


    <!-- https://w3id.org/reno#WindowGlazingType -->


    <owl:Class rdf:about="https://w3id.org/reno#WindowGlazingType">
        <rdfs:comment xml:lang="nl">Het type beglazing heeft veel invloed op de thermische en akoestische performantie van het raam.</rdfs:comment>
        <rdfs:comment xml:lang="en">The type of glazing has a lot of influence on the thermal and acoustic performance of the window.</rdfs:comment>
        <rdfs:label xml:lang="nl">raambeglazingstype</rdfs:label>
        <rdfs:label xml:lang="en">window glazing type</rdfs:label>
    </owl:Class>
    


    <!-- https://w3id.org/reno#Wood -->


    <owl:Class rdf:about="https://w3id.org/reno#Wood">
        <rdfs:subClassOf rdf:resource="https://saref.etsi.org/core/EnergyCommodity"/>
        <rdfs:subClassOf rdf:resource="https://saref.etsi.org/core/NaturalResourceCommodity"/>
        <rdfs:subClassOf rdf:resource="https://w3id.org/reno#WindowFrameMaterial"/>
        <rdfs:comment xml:lang="nl">Hout is een structureel weefsel of materiaal dat gevonden wordt in de stammen en wortels van bomen en andere houtachtige planten.</rdfs:comment>
        <rdfs:comment xml:lang="en">Wood is a structural tissue or material found in the stems and roots of trees and other woody plants.</rdfs:comment>
        <rdfs:label xml:lang="nl">hout</rdfs:label>
        <rdfs:label xml:lang="en">wood</rdfs:label>
        <rdfs:seeAlso xml:lang="en">https://en.wikipedia.org/wiki/Wood</rdfs:seeAlso>
        <rdfs:seeAlso xml:lang="nl">https://nl.wikipedia.org/wiki/Hout</rdfs:seeAlso>
    </owl:Class>
    


    <!-- 
    ///////////////////////////////////////////////////////////////////////////////////////
    //
    // Individuals
    //
    ///////////////////////////////////////////////////////////////////////////////////////
     -->


    


    <!-- https://example.com/AsRoom -->


    <owl:NamedIndividual rdf:about="https://example.com/AsRoom">
        <rdf:type rdf:resource="https://w3id.org/reno#SpaceUsage"/>
    </owl:NamedIndividual>
    


    <!-- https://example.com/AsbestosFreeRoof -->


    <owl:NamedIndividual rdf:about="https://example.com/AsbestosFreeRoof"/>
    


    <!-- https://example.com/Bathing -->


    <owl:NamedIndividual rdf:about="https://example.com/Bathing">
        <rdf:type rdf:resource="https://saref.etsi.org/core/Task"/>
    </owl:NamedIndividual>
    


    <!-- https://example.com/ConnectToHeatGrid -->


    <owl:NamedIndividual rdf:about="https://example.com/ConnectToHeatGrid">
        <rdf:type rdf:resource="http://www.daml.org/services/owl-s/1.1/Process.owl#AtomicProcess"/>
    </owl:NamedIndividual>
    


    <!-- https://example.com/Cooking -->


    <owl:NamedIndividual rdf:about="https://example.com/Cooking">
        <rdf:type rdf:resource="https://saref.etsi.org/core/Task"/>
    </owl:NamedIndividual>
    


    <!-- https://example.com/EnvironmentalConsideration -->


    <owl:NamedIndividual rdf:about="https://example.com/EnvironmentalConsideration">
        <rdf:type rdf:resource="https://w3id.org/reno#EnergyReductionMotivation"/>
    </owl:NamedIndividual>
    


    <!-- https://example.com/FillingPool -->


    <owl:NamedIndividual rdf:about="https://example.com/FillingPool">
        <rdf:type rdf:resource="https://saref.etsi.org/core/Task"/>
    </owl:NamedIndividual>
    


    <!-- https://example.com/FinancialConsideration -->


    <owl:NamedIndividual rdf:about="https://example.com/FinancialConsideration">
        <rdf:type rdf:resource="https://w3id.org/reno#EnergyReductionMotivation"/>
    </owl:NamedIndividual>
    


    <!-- https://example.com/ForStorage -->


    <owl:NamedIndividual rdf:about="https://example.com/ForStorage">
        <rdf:type rdf:resource="https://w3id.org/reno#SpaceUsage"/>
    </owl:NamedIndividual>
    


    <!-- https://example.com/ForTechnicalInstallations -->


    <owl:NamedIndividual rdf:about="https://example.com/ForTechnicalInstallations">
        <rdf:type rdf:resource="https://w3id.org/reno#SpaceUsage"/>
    </owl:NamedIndividual>
    


    <!-- https://example.com/HighNuisance -->


    <owl:NamedIndividual rdf:about="https://example.com/HighNuisance">
        <hasNuisanceScore rdf:datatype="http://www.w3.org/2001/XMLSchema#integer">8</hasNuisanceScore>
    </owl:NamedIndividual>
    


    <!-- https://example.com/InsulateAtticFloor -->


    <owl:NamedIndividual rdf:about="https://example.com/InsulateAtticFloor">
        <rdf:type rdf:resource="http://www.daml.org/services/owl-s/1.1/Process.owl#AtomicProcess"/>
    </owl:NamedIndividual>
    


    <!-- https://example.com/InsulateFlatRoof -->


    <owl:NamedIndividual rdf:about="https://example.com/InsulateFlatRoof">
        <rdf:type rdf:resource="http://www.daml.org/services/owl-s/1.1/Process.owl#AtomicProcess"/>
    </owl:NamedIndividual>
    


    <!-- https://example.com/InsulateFloorAboveBasement -->


    <owl:NamedIndividual rdf:about="https://example.com/InsulateFloorAboveBasement">
        <rdf:type rdf:resource="http://www.daml.org/services/owl-s/1.1/Process.owl#AtomicProcess"/>
    </owl:NamedIndividual>
    


    <!-- https://example.com/InsulateGableRoof -->


    <owl:NamedIndividual rdf:about="https://example.com/InsulateGableRoof">
        <rdf:type rdf:resource="http://www.daml.org/services/owl-s/1.1/Process.owl#AtomicProcess"/>
    </owl:NamedIndividual>
    


    <!-- https://example.com/InsulateWallCavity -->


    <owl:NamedIndividual rdf:about="https://example.com/InsulateWallCavity">
        <rdf:type rdf:resource="http://www.daml.org/services/owl-s/1.1/Process.owl#AtomicProcess"/>
    </owl:NamedIndividual>
    


    <!-- https://example.com/InsulateWallExterior -->


    <owl:NamedIndividual rdf:about="https://example.com/InsulateWallExterior">
        <rdf:type rdf:resource="http://www.daml.org/services/owl-s/1.1/Process.owl#AtomicProcess"/>
    </owl:NamedIndividual>
    


    <!-- https://example.com/InsulateWallInterior -->


    <owl:NamedIndividual rdf:about="https://example.com/InsulateWallInterior">
        <rdf:type rdf:resource="http://www.daml.org/services/owl-s/1.1/Process.owl#AtomicProcess"/>
    </owl:NamedIndividual>
    


    <!-- https://example.com/InsulatedFloor -->


    <owl:NamedIndividual rdf:about="https://example.com/InsulatedFloor"/>
    


    <!-- https://example.com/LowNuisance -->


    <owl:NamedIndividual rdf:about="https://example.com/LowNuisance">
        <hasNuisanceScore rdf:datatype="http://www.w3.org/2001/XMLSchema#integer">2</hasNuisanceScore>
    </owl:NamedIndividual>
    


    <!-- https://example.com/ModerateNuisance -->


    <owl:NamedIndividual rdf:about="https://example.com/ModerateNuisance">
        <hasNuisanceScore rdf:datatype="http://www.w3.org/2001/XMLSchema#integer">5</hasNuisanceScore>
    </owl:NamedIndividual>
    


    <!-- https://example.com/NoMotivation -->


    <owl:NamedIndividual rdf:about="https://example.com/NoMotivation">
        <rdf:type rdf:resource="https://w3id.org/reno#RenovationMotivation"/>
    </owl:NamedIndividual>
    


    <!-- https://example.com/Normal -->


    <owl:NamedIndividual rdf:about="https://example.com/Normal">
        <rdf:type rdf:resource="https://w3id.org/reno#SoundLevel"/>
    </owl:NamedIndividual>
    


    <!-- https://example.com/NotInUse -->


    <owl:NamedIndividual rdf:about="https://example.com/NotInUse">
        <rdf:type rdf:resource="https://w3id.org/reno#SpaceUsage"/>
    </owl:NamedIndividual>
    


    <!-- https://example.com/NotMatterNuisance -->


    <owl:NamedIndividual rdf:about="https://example.com/NotMatterNuisance">
        <hasNuisanceScore rdf:datatype="http://www.w3.org/2001/XMLSchema#integer">10</hasNuisanceScore>
    </owl:NamedIndividual>
    


    <!-- https://example.com/OtherMotivation -->


    <owl:NamedIndividual rdf:about="https://example.com/OtherMotivation">
        <rdf:type rdf:resource="https://w3id.org/reno#RenovationMotivation"/>
    </owl:NamedIndividual>
    


    <!-- https://example.com/PlaceAirAirHeatpump -->


    <owl:NamedIndividual rdf:about="https://example.com/PlaceAirAirHeatpump">
        <rdf:type rdf:resource="http://www.daml.org/services/owl-s/1.1/Process.owl#AtomicProcess"/>
    </owl:NamedIndividual>
    


    <!-- https://example.com/PlaceAirWaterHeatpump -->


    <owl:NamedIndividual rdf:about="https://example.com/PlaceAirWaterHeatpump">
        <rdf:type rdf:resource="http://www.daml.org/services/owl-s/1.1/Process.owl#AtomicProcess"/>
    </owl:NamedIndividual>
    


    <!-- https://example.com/PlaceAirWaterHeatpumpWithCooling -->


    <owl:NamedIndividual rdf:about="https://example.com/PlaceAirWaterHeatpumpWithCooling">
        <rdf:type rdf:resource="http://www.daml.org/services/owl-s/1.1/Process.owl#AtomicProcess"/>
    </owl:NamedIndividual>
    


    <!-- https://example.com/PlaceAirconditioning -->


    <owl:NamedIndividual rdf:about="https://example.com/PlaceAirconditioning">
        <rdf:type rdf:resource="http://www.daml.org/services/owl-s/1.1/Process.owl#AtomicProcess"/>
    </owl:NamedIndividual>
    


    <!-- https://example.com/PlaceFloorHeating -->


    <owl:NamedIndividual rdf:about="https://example.com/PlaceFloorHeating">
        <rdf:type rdf:resource="http://www.daml.org/services/owl-s/1.1/Process.owl#AtomicProcess"/>
        <Process:hasPrecondition rdf:resource="https://example.com/InsulatedFloor"/>
    </owl:NamedIndividual>
    


    <!-- https://example.com/PlaceGeothermalHeatpumpHorizontal -->


    <owl:NamedIndividual rdf:about="https://example.com/PlaceGeothermalHeatpumpHorizontal">
        <rdf:type rdf:resource="http://www.daml.org/services/owl-s/1.1/Process.owl#AtomicProcess"/>
    </owl:NamedIndividual>
    


    <!-- https://example.com/PlaceGeothermalHeatpumpVertical -->


    <owl:NamedIndividual rdf:about="https://example.com/PlaceGeothermalHeatpumpVertical">
        <rdf:type rdf:resource="http://www.daml.org/services/owl-s/1.1/Process.owl#AtomicProcess"/>
    </owl:NamedIndividual>
    


    <!-- https://example.com/PlaceHeatPumpBoiler -->


    <owl:NamedIndividual rdf:about="https://example.com/PlaceHeatPumpBoiler">
        <rdf:type rdf:resource="http://www.daml.org/services/owl-s/1.1/Process.owl#AtomicProcess"/>
    </owl:NamedIndividual>
    


    <!-- https://example.com/PlaceLowTemperatureEmission -->


    <owl:NamedIndividual rdf:about="https://example.com/PlaceLowTemperatureEmission">
        <rdf:type rdf:resource="http://www.daml.org/services/owl-s/1.1/Process.owl#AtomicProcess"/>
    </owl:NamedIndividual>
    


    <!-- https://example.com/PlacePVPanelsInGarden -->


    <owl:NamedIndividual rdf:about="https://example.com/PlacePVPanelsInGarden">
        <rdf:type rdf:resource="http://www.daml.org/services/owl-s/1.1/Process.owl#AtomicProcess"/>
    </owl:NamedIndividual>
    


    <!-- https://example.com/PlacePVPanelsOnRoof -->


    <owl:NamedIndividual rdf:about="https://example.com/PlacePVPanelsOnRoof">
        <rdf:type rdf:resource="http://www.daml.org/services/owl-s/1.1/Process.owl#AtomicProcess"/>
        <Process:hasPrecondition rdf:resource="https://example.com/AsbestosFreeRoof"/>
    </owl:NamedIndividual>
    


    <!-- https://example.com/PlaceRoofUnderlayment -->


    <owl:NamedIndividual rdf:about="https://example.com/PlaceRoofUnderlayment">
        <rdf:type rdf:resource="http://www.daml.org/services/owl-s/1.1/Process.owl#AtomicProcess"/>
    </owl:NamedIndividual>
    


    <!-- https://example.com/PlaceSunShade -->


    <owl:NamedIndividual rdf:about="https://example.com/PlaceSunShade">
        <rdf:type rdf:resource="http://www.daml.org/services/owl-s/1.1/Process.owl#AtomicProcess"/>
    </owl:NamedIndividual>
    


    <!-- https://example.com/Quiet -->


    <owl:NamedIndividual rdf:about="https://example.com/Quiet">
        <rdf:type rdf:resource="https://w3id.org/reno#SoundLevel"/>
    </owl:NamedIndividual>
    


    <!-- https://example.com/RemoveAsbestosFlatRoof -->


    <owl:NamedIndividual rdf:about="https://example.com/RemoveAsbestosFlatRoof">
        <rdf:type rdf:resource="http://www.daml.org/services/owl-s/1.1/Process.owl#AtomicProcess"/>
    </owl:NamedIndividual>
    


    <!-- https://example.com/RemoveAsbestosGableRoof -->


    <owl:NamedIndividual rdf:about="https://example.com/RemoveAsbestosGableRoof">
        <rdf:type rdf:resource="http://www.daml.org/services/owl-s/1.1/Process.owl#AtomicProcess"/>
    </owl:NamedIndividual>
    


    <!-- https://example.com/ReplaceFlatRoof -->


    <owl:NamedIndividual rdf:about="https://example.com/ReplaceFlatRoof">
        <rdf:type rdf:resource="http://www.daml.org/services/owl-s/1.1/Process.owl#AtomicProcess"/>
    </owl:NamedIndividual>
    


    <!-- https://example.com/ReplaceGableRoof -->


    <owl:NamedIndividual rdf:about="https://example.com/ReplaceGableRoof">
        <rdf:type rdf:resource="http://www.daml.org/services/owl-s/1.1/Process.owl#AtomicProcess"/>
    </owl:NamedIndividual>
    


    <!-- https://example.com/ReplaceGlazing -->


    <owl:NamedIndividual rdf:about="https://example.com/ReplaceGlazing">
        <rdf:type rdf:resource="http://www.daml.org/services/owl-s/1.1/Process.owl#AtomicProcess"/>
    </owl:NamedIndividual>
    


    <!-- https://example.com/ReplaceVentilationSystem -->


    <owl:NamedIndividual rdf:about="https://example.com/ReplaceVentilationSystem">
        <rdf:type rdf:resource="http://www.daml.org/services/owl-s/1.1/Process.owl#AtomicProcess"/>
    </owl:NamedIndividual>
    


    <!-- https://example.com/ReplaceWindows -->


    <owl:NamedIndividual rdf:about="https://example.com/ReplaceWindows">
        <rdf:type rdf:resource="http://www.daml.org/services/owl-s/1.1/Process.owl#AtomicProcess"/>
    </owl:NamedIndividual>
    


    <!-- https://example.com/Showering -->


    <owl:NamedIndividual rdf:about="https://example.com/Showering">
        <rdf:type rdf:resource="https://saref.etsi.org/core/Task"/>
    </owl:NamedIndividual>
    


    <!-- https://example.com/SpaceCooling -->


    <owl:NamedIndividual rdf:about="https://example.com/SpaceCooling">
        <rdf:type rdf:resource="https://saref.etsi.org/core/Task"/>
    </owl:NamedIndividual>
    


    <!-- https://example.com/SpaceHeating -->


    <owl:NamedIndividual rdf:about="https://example.com/SpaceHeating">
        <rdf:type rdf:resource="https://saref.etsi.org/core/Task"/>
    </owl:NamedIndividual>
    


    <!-- https://example.com/TakingASauna -->


    <owl:NamedIndividual rdf:about="https://example.com/TakingASauna">
        <rdf:type rdf:resource="https://saref.etsi.org/core/Task"/>
    </owl:NamedIndividual>
    


    <!-- https://example.com/ToImproveEPC -->


    <owl:NamedIndividual rdf:about="https://example.com/ToImproveEPC">
        <rdf:type rdf:resource="https://w3id.org/reno#EnergyReductionMotivation"/>
        <rdf:type rdf:resource="https://w3id.org/reno#RenovationMotivation"/>
    </owl:NamedIndividual>
    


    <!-- https://example.com/ToImproveSustainability -->


    <owl:NamedIndividual rdf:about="https://example.com/ToImproveSustainability">
        <rdf:type rdf:resource="https://w3id.org/reno#RenovationMotivation"/>
    </owl:NamedIndividual>
    


    <!-- https://example.com/ToIncreaseMarketValue -->


    <owl:NamedIndividual rdf:about="https://example.com/ToIncreaseMarketValue">
        <rdf:type rdf:resource="https://w3id.org/reno#RenovationMotivation"/>
    </owl:NamedIndividual>
    


    <!-- https://example.com/ToIncreaseThermalComfort -->


    <owl:NamedIndividual rdf:about="https://example.com/ToIncreaseThermalComfort">
        <rdf:type rdf:resource="https://w3id.org/reno#RenovationMotivation"/>
    </owl:NamedIndividual>
    


    <!-- https://example.com/ToLowerEnergyConsumption -->


    <owl:NamedIndividual rdf:about="https://example.com/ToLowerEnergyConsumption">
        <rdf:type rdf:resource="https://w3id.org/reno#RenovationMotivation"/>
    </owl:NamedIndividual>
    


    <!-- https://example.com/ToLowerEnergyCost -->


    <owl:NamedIndividual rdf:about="https://example.com/ToLowerEnergyCost">
        <rdf:type rdf:resource="https://w3id.org/reno#RenovationMotivation"/>
    </owl:NamedIndividual>
    


    <!-- https://example.com/VeryQuiet -->


    <owl:NamedIndividual rdf:about="https://example.com/VeryQuiet">
        <rdf:type rdf:resource="https://w3id.org/reno#SoundLevel"/>
    </owl:NamedIndividual>
    


    <!-- https://example.com/WaterHeating -->


    <owl:NamedIndividual rdf:about="https://example.com/WaterHeating">
        <rdf:type rdf:resource="https://saref.etsi.org/core/Task"/>
    </owl:NamedIndividual>
</rdf:RDF>



<!-- Generated by the OWL API (version 5.1.18) https://github.com/owlcs/owlapi/ -->


